PREFIX :          <https://w3id.org/idsa/core#>
PREFIX core:      <https://w3id.org/idsa/core/>
PREFIX dcam:      <http://purl.org/dc/dcam/>
PREFIX dqv:       <http://www.w3.org/ns/dqv#>
PREFIX foaf:      <http://xmlns.com/foaf/0.1/>
PREFIX ns:        <http://creativecommons.org/ns#>
PREFIX odrl:      <http://www.w3.org/ns/odrl/2/>
PREFIX org:       <http://www.w3.org/ns/org#>
PREFIX owl:       <http://www.w3.org/2002/07/owl#>
PREFIX rdf:       <http://www.w3.org/1999/02/22-rdf-syntax-ns#>
PREFIX rdfs:      <http://www.w3.org/2000/01/rdf-schema#>
PREFIX skos:      <http://www.w3.org/2004/02/skos/core#>
PREFIX terms:     <http://purl.org/dc/terms/>
PREFIX vann:      <http://purl.org/vocab/vann/>
PREFIX void:      <http://rdfs.org/ns/void#>
PREFIX wgs84_pos: <http://www.w3.org/2003/01/geo/wgs84_pos#>
PREFIX xml:       <http://www.w3.org/XML/1998/namespace>
PREFIX xsd:       <http://www.w3.org/2001/XMLSchema#>

<https://w3id.org/idsa/code/AA>
        rdf:type    core:Language , owl:NamedIndividual;
        rdfs:label  "Afar"@en .

<https://w3id.org/idsa/code/AB>
        rdf:type    core:Language , owl:NamedIndividual;
        rdfs:label  "Abkhaz"@en .

<https://w3id.org/idsa/code/ABSOLUTE_SPATIAL_POSITION>
        rdf:type      odrl:LeftOperand , owl:NamedIndividual;
        rdfs:comment  "The current geospatial position of the *consuming connector*. In case the connector only appears as a virtual entity, the physical location of the hosting server is referenced. Allowed operators are idsc:in. No other spatial operators (close to, north of, etc.) are currently allowed."@en;
        rdfs:label    "Absolute geo-spatial position"@en;
        skos:broader  odrl:absoluteSpatialPosition .

<https://w3id.org/idsa/code/ADD>
        rdf:type      odrl:Action , owl:NamedIndividual;
        rdfs:comment  "This action modifies a number by adding a given value to it."@en;
        rdfs:label    "add"@en;
        skos:note     "This action modifies a number by adding a given value to it. The field to be modified and the given value are specified in the policy as idsc:JSONPATH/idsc:XPATH and idsc:OPERAND, respectively."@en .

<https://w3id.org/idsa/code/AE>
        rdf:type    core:Language , owl:NamedIndividual;
        rdfs:label  "Avestan"@en .

<https://w3id.org/idsa/code/AF>
        rdf:type    core:Language , owl:NamedIndividual;
        rdfs:label  "Afrikaans"@en .

<https://w3id.org/idsa/code/AFTER>
        rdf:type      core:BinaryOperator , owl:NamedIndividual;
        rdfs:comment  "If a temporal entity T1 is after another temporal entity T2, then the beginning of T1 is after the end of T2 and the beginning of T1 is different to the ending of T2. Temporal entities can either be a xsd:dateTimeStamp or a time:TemporalEntity."@en;
        rdfs:label    "after"@en;
        rdfs:seeAlso  <http://www.w3.org/2006/time#after> .

<https://w3id.org/idsa/code/AGGREGATE_BY_CONSUMER>
        rdf:type         odrl:Action , owl:NamedIndividual;
        rdfs:comment     "Data will be part of another piece of data so that it is not distinguishable anymore."@en;
        rdfs:label       "aggregate by consumer"@en;
        skos:broader     odrl:aggregate;
        skos:note        "This action is always evaluated at the consumer side."@en;
        odrl:includedIn  <https://w3id.org/idsa/code/USE> .

<https://w3id.org/idsa/code/AGGREGATE_BY_PROVIDER>
        rdf:type         odrl:Action , owl:NamedIndividual;
        rdfs:comment     "Data will be part of another piece of data so that it is not distinguishable anymore."@en;
        rdfs:label       "aggregate by provider"@en;
        skos:broader     odrl:aggregate;
        skos:note        "This action is always evaluated at the provider side."@en;
        odrl:includedIn  <https://w3id.org/idsa/code/AGGREGATE_BY_CONSUMER> .

<https://w3id.org/idsa/code/AK>
        rdf:type    core:Language , owl:NamedIndividual;
        rdfs:label  "Akan"@en .

<https://w3id.org/idsa/code/ALLOW_DATA_USAGE>
        rdf:type      core:UsagePolicyClass , owl:NamedIndividual;
        rdfs:comment  "This policy restricts the usage of the data to a specific Data Consumer, regardless of how many connectors they have and without any further usage restriction."@en;
        rdfs:label    "Allow data usage"@en .

<https://w3id.org/idsa/code/AM>
        rdf:type    core:Language , owl:NamedIndividual;
        rdfs:label  "Amharic"@en .

<https://w3id.org/idsa/code/AN>
        rdf:type    core:Language , owl:NamedIndividual;
        rdfs:label  "Aragonese"@en .

<https://w3id.org/idsa/code/ANNUAL>
        rdf:type          core:Frequency , skos:Concept , owl:NamedIndividual;
        rdfs:comment      "The event occurs once a year."@en;
        rdfs:isDefinedBy  <http://purl.org/cld/freq/>;
        rdfs:label        "Annual"@en;
        rdfs:seeAlso      <https://www.loc.gov/marc/holdings/hd853855.html>;
        dcam:memberOf     <http://purl.org/cld/terms/Frequency>;
        skos:inScheme     <http://purl.org/cld/terms/Frequency>;
        skos:prefLabel    "Annual"@en .

<https://w3id.org/idsa/code/ANONYMIZE>
        rdf:type         odrl:Action , owl:NamedIndividual;
        rdfs:comment     "To anonymize all, parts or certain attributes of the resource."@en;
        rdfs:label       "anonymize"@en;
        skos:broader     odrl:anonymize;
        skos:note        "This action is always evaluated at the provider side."@en;
        odrl:includedIn  <https://w3id.org/idsa/code/USE> .

<https://w3id.org/idsa/code/ANONYMIZED>
        rdf:type      core:ArtifactState , owl:NamedIndividual;
        rdfs:comment  "The artifact is anonymized so the data source can not be recognized by any further user."@en;
        rdfs:label    "is anonymized"@en .

<https://w3id.org/idsa/code/ANY>
        rdf:type    core:QueryTarget , owl:NamedIndividual;
        rdfs:label  "ANY" .

<https://w3id.org/idsa/code/APPLICATION>
        rdf:type      odrl:LeftOperand , owl:NamedIndividual;
        rdfs:comment  "An application is a program or piece of software designed to fulfill a particular purpose. For example, a certified IDS App."@en;
        rdfs:label    "application" .

<https://w3id.org/idsa/code/APPLICATION_RESTRICTED_DATA_USAGE>
        rdf:type      core:UsagePolicyClass , owl:NamedIndividual;
        rdfs:comment  "This policy restricts the usage of the data to a specific system or application inside an IDS Connector."@en;
        rdfs:label    "System restricted data usage"@en .

<https://w3id.org/idsa/code/APPSTORE>
        rdf:type    core:QueryTarget , owl:NamedIndividual;
        rdfs:label  "APPSTORE" .

<https://w3id.org/idsa/code/APP_RESOURCES_LOCAL_ENFORCEMENT>
        rdf:type    core:AppExecutionResources , owl:NamedIndividual;
        rdfs:label  "App Resources Local Enforcement" .

<https://w3id.org/idsa/code/APP_RESOURCES_NONE>
        rdf:type    core:AppExecutionResources , owl:NamedIndividual;
        rdfs:label  "App Resources None" .

<https://w3id.org/idsa/code/APP_RESOURCES_REMOTE_VERIFICATION>
        rdf:type    core:AppExecutionResources , owl:NamedIndividual;
        rdfs:label  "App Resources Remote Verification" .

<https://w3id.org/idsa/code/AR>
        rdf:type    core:Language , owl:NamedIndividual;
        rdfs:label  "Arabic"@en .

<https://w3id.org/idsa/code/ARTIFACT_STATE>
        rdf:type      odrl:LeftOperand , owl:NamedIndividual;
        rdfs:comment  "Suggested values exist in the Information Model : idsc:ANONYMIZED, idsc:PSEUDONYMIZED, idsc:ENCRYPTED, idsc:COMBINED. "@en;
        rdfs:label    "artifact state"@en .

<https://w3id.org/idsa/code/AS>
        rdf:type    core:Language , owl:NamedIndividual;
        rdfs:label  "Assamese"@en .

<https://w3id.org/idsa/code/ATTACH_POLICY_FOR_THIRD_PARTY>
        rdf:type      core:UsagePolicyClass , owl:NamedIndividual;
        rdfs:comment  "This policy restricts the usage of data assets with the obligation to notify a specific party about the data usage."@en;
        rdfs:label    "Remote notification"@en .

<https://w3id.org/idsa/code/AUDIT_LOCAL_LOGGING>
        rdf:type    core:AuditGuarantee , owl:NamedIndividual;
        rdfs:label  "Audit Local Logging" .

<https://w3id.org/idsa/code/AUDIT_NONE>
        rdf:type    core:AuditGuarantee , owl:NamedIndividual;
        rdfs:label  "Audit None" .

<https://w3id.org/idsa/code/AUDIT_REMOTE_TRACING>
        rdf:type    core:AuditGuarantee , owl:NamedIndividual;
        rdfs:label  "Audit Remote Tracing" .

<https://w3id.org/idsa/code/AUTHENTICATION_MUTUAL>
        rdf:type    core:AuthenticationGuarantee , owl:NamedIndividual;
        rdfs:label  "Authentication Mutual" .

<https://w3id.org/idsa/code/AUTHENTICATION_NONE>
        rdf:type    core:AuthenticationGuarantee , owl:NamedIndividual;
        rdfs:label  "Authentication None" .

<https://w3id.org/idsa/code/AUTHENTICATION_SERVER_SIDE>
        rdf:type    core:AuthenticationGuarantee , owl:NamedIndividual;
        rdfs:label  "Authentication Serverside" .

<https://w3id.org/idsa/code/AV>
        rdf:type    core:Language , owl:NamedIndividual;
        rdfs:label  "Avaric"@en .

<https://w3id.org/idsa/code/AVAILABILITY>
        rdf:type         dqv:Dimension , owl:NamedIndividual;
        rdfs:label       "Availability";
        skos:definition  "Availability of a dataset: Is the data present, obtainable and ready for use?"@en .

<https://w3id.org/idsa/code/AY>
        rdf:type    core:Language , owl:NamedIndividual;
        rdfs:label  "Aymara"@en .

<https://w3id.org/idsa/code/AZ>
        rdf:type    core:Language , owl:NamedIndividual;
        rdfs:label  "Azerbaijani"@en .

<https://w3id.org/idsa/code/BA>
        rdf:type    core:Language , owl:NamedIndividual;
        rdfs:label  "Bashkir"@en .

<https://w3id.org/idsa/code/BAD_PARAMETERS>
        rdf:type      core:RejectionReason , owl:NamedIndividual;
        rdfs:comment  "At least one query or operation parameter is not acceptable for the sender of this rejection message.";
        rdfs:label    "BAD_PARAMETERS" .

<https://w3id.org/idsa/code/BASE_SECURITY_PROFILE>
        rdf:type                core:SecurityProfile , owl:NamedIndividual;
        rdfs:comment            "Default security profile of a certified IDS Connector."@en;
        rdfs:label              "Base security profile"@en;
        core:securityGuarantee  <https://w3id.org/idsa/code/USAGE_CONTROL_NONE> , <https://w3id.org/idsa/code/SERVICE_ISOLATION_PROCESS_GROUP> , <https://w3id.org/idsa/code/LOCAL_DATA_CONFIDENTIALITY_NONE> , <https://w3id.org/idsa/code/INTEGRITY_VERIFICATION_SCOPE_NONE> , <https://w3id.org/idsa/code/INTEGRITY_PROTECTION_NONE> , <https://w3id.org/idsa/code/AUTHENTICATION_MUTUAL> , <https://w3id.org/idsa/code/AUDIT_LOCAL_LOGGING> , <https://w3id.org/idsa/code/APP_RESOURCES_NONE> .

<https://w3id.org/idsa/code/BE>
        rdf:type    core:Language , owl:NamedIndividual;
        rdfs:label  "Belarusian"@en .

<https://w3id.org/idsa/code/BEFORE>
        rdf:type      core:BinaryOperator , owl:NamedIndividual;
        rdfs:comment  "If a temporal entity T1 is before another temporal entity T2, then the ending of T1 is before the end of T2 and the ending of T1 is different to the beginning of T2. Temporal entities can either be a xsd:dateTimeStamp or a time:TemporalEntity."@en;
        rdfs:label    "before"@en;
        rdfs:seeAlso  <http://www.w3.org/2006/time#before>;
        skos:note     "Compares an instance of time:TemporalEntity or a Literal of xsd:dateTimeStamp to an instance of time:TemporalEntity or a Literal of xsd:dateTimeStamp."@en .

<https://w3id.org/idsa/code/BG>
        rdf:type    core:Language , owl:NamedIndividual;
        rdfs:label  "Bulgarian"@en .

<https://w3id.org/idsa/code/BH>
        rdf:type    core:Language , owl:NamedIndividual;
        rdfs:label  "Bihari"@en .

<https://w3id.org/idsa/code/BI>
        rdf:type    core:Language , owl:NamedIndividual;
        rdfs:label  "Bislama"@en .

<https://w3id.org/idsa/code/BIENNIAL>
        rdf:type          core:Frequency , skos:Concept , owl:NamedIndividual;
        rdfs:comment      "The event occurs every two years."@en;
        rdfs:isDefinedBy  <http://purl.org/cld/freq/>;
        rdfs:label        "Biennial"@en;
        rdfs:seeAlso      <https://www.loc.gov/marc/holdings/hd853855.html>;
        dcam:memberOf     <http://purl.org/cld/terms/Frequency>;
        skos:inScheme     <http://purl.org/cld/terms/Frequency>;
        skos:prefLabel    "Biennial"@en .

<https://w3id.org/idsa/code/BIHOURLY>
        rdf:type      core:Frequency , skos:Concept , owl:NamedIndividual;
        rdfs:comment  "The event occurs twice an hour."@en;
        rdfs:label    "Bihourly"@en .

<https://w3id.org/idsa/code/BIMONTHLY>
        rdf:type          core:Frequency , skos:Concept , owl:NamedIndividual;
        rdfs:comment      "The event occurs every two months."@en;
        rdfs:isDefinedBy  <http://purl.org/cld/freq/>;
        rdfs:label        "Bimonthly"@en;
        rdfs:seeAlso      <https://www.loc.gov/marc/holdings/hd853855.html>;
        dcam:memberOf     <http://purl.org/cld/terms/Frequency>;
        skos:inScheme     <http://purl.org/cld/terms/Frequency>;
        skos:prefLabel    "Bimonthly"@en .

<https://w3id.org/idsa/code/BIWEEKLY>
        rdf:type          core:Frequency , skos:Concept , owl:NamedIndividual;
        rdfs:comment      "The event occurs every two weeks."@en;
        rdfs:isDefinedBy  <http://purl.org/cld/freq/>;
        rdfs:label        "Biweekly"@en;
        rdfs:seeAlso      <https://www.loc.gov/marc/holdings/hd853855.html>;
        dcam:memberOf     <http://purl.org/cld/terms/Frequency>;
        skos:inScheme     <http://purl.org/cld/terms/Frequency>;
        skos:prefLabel    "Biweekly"@en .

<https://w3id.org/idsa/code/BM>
        rdf:type    core:Language , owl:NamedIndividual;
        rdfs:label  "Bambara"@en .

<https://w3id.org/idsa/code/BN>
        rdf:type    core:Language , owl:NamedIndividual;
        rdfs:label  "Bengali, Bangla"@en .

<https://w3id.org/idsa/code/BO>
        rdf:type    core:Language , owl:NamedIndividual;
        rdfs:label  "Tibetan Standard, Tibetan, Central"@en .

<https://w3id.org/idsa/code/BR>
        rdf:type    core:Language , owl:NamedIndividual;
        rdfs:label  "Breton"@en .

<https://w3id.org/idsa/code/BROKER>
        rdf:type    core:QueryTarget , owl:NamedIndividual;
        rdfs:label  "BROKER" .

<https://w3id.org/idsa/code/BS>
        rdf:type    core:Language , owl:NamedIndividual;
        rdfs:label  "Bosnian"@en .

<https://w3id.org/idsa/code/CA>
        rdf:type    core:Language , owl:NamedIndividual;
        rdfs:label  "Catalan"@en .

<https://w3id.org/idsa/code/CE>
        rdf:type    core:Language , owl:NamedIndividual;
        rdfs:label  "Chechen"@en .

<https://w3id.org/idsa/code/CH>
        rdf:type    core:Language , owl:NamedIndividual;
        rdfs:label  "Chamorro"@en .

<https://w3id.org/idsa/code/CLEARING_HOUSE>
        rdf:type    core:QueryTarget , owl:NamedIndividual;
        rdfs:label  "CLEARING_HOUSE" .

<https://w3id.org/idsa/code/CO>
        rdf:type    core:Language , owl:NamedIndividual;
        rdfs:label  "Corsican"@en .

<https://w3id.org/idsa/code/COMBINED>
        rdf:type      core:ArtifactState , owl:NamedIndividual;
        rdfs:comment  "The artifact is a collection of smaller artifacts and can be split into parts when necessary."@en;
        rdfs:label    "is combined"@en .

<https://w3id.org/idsa/code/COMPENSATE>
        rdf:type         odrl:Action , owl:NamedIndividual;
        rdfs:comment     "To pay a certain amount of money in order to use a resource."@en;
        rdfs:label       "compensate"@en;
        skos:broader     odrl:compensate;
        skos:note        "This action must be evaluated both at the consumer and provider side. A compensation might be required before access is granted (provider-side), or each time the usage action is performed (consumer-side)."@en;
        odrl:includedIn  <https://w3id.org/idsa/code/USE> .

<https://w3id.org/idsa/code/COMPONENT_BASE_SECURITY_PROFILE_CHECKLIST_APPROACH>
        rdf:type    core:ComponentCertificationLevel , owl:NamedIndividual;
        rdfs:label  "Base Security Profile Certification of Components based on Checklist Approach"@en .

<https://w3id.org/idsa/code/COMPONENT_BASE_SECURITY_PROFILE_CONCEPT_REVIEW>
        rdf:type    core:ComponentCertificationLevel , owl:NamedIndividual;
        rdfs:label  "Base Security Profile Certification of Components based on Concept Review"@en;
        core:includedCertificationLevel
                <https://w3id.org/idsa/code/COMPONENT_BASE_SECURITY_PROFILE_CHECKLIST_APPROACH> .

<https://w3id.org/idsa/code/COMPONENT_TRUSTPLUS_SECURITY_PROFILE_CONCEPT_REVIEW>
        rdf:type    core:ComponentCertificationLevel , owl:NamedIndividual;
        rdfs:label  "Trust-Plus Security Profile Certification of Components based on Concept Review"@en;
        core:includedCertificationLevel
                <https://w3id.org/idsa/code/COMPONENT_TRUST_SECURITY_PROFILE_CONCEPT_REVIEW> .

<https://w3id.org/idsa/code/COMPONENT_TRUSTPLUS_SECURITY_PROFILE_HIGH_ASSURANCE_EVALUATION>
        rdf:type    core:ComponentCertificationLevel , owl:NamedIndividual;
        rdfs:label  "Trust-Plus Security Profile Certification of Components based on High AssuranceEvaluation"@en;
        core:includedCertificationLevel
                <https://w3id.org/idsa/code/COMPONENT_TRUSTPLUS_SECURITY_PROFILE_CONCEPT_REVIEW> .

<https://w3id.org/idsa/code/COMPONENT_TRUST_SECURITY_PROFILE_CONCEPT_REVIEW>
        rdf:type    core:ComponentCertificationLevel , owl:NamedIndividual;
        rdfs:label  "Trust Security Profile Certification of Components based on Concept Review"@en;
        core:includedCertificationLevel
                <https://w3id.org/idsa/code/COMPONENT_BASE_SECURITY_PROFILE_CONCEPT_REVIEW> .

<https://w3id.org/idsa/code/COMPONENT_TRUST_SECURITY_PROFILE_HIGH_ASSURANCE_EVALUATION>
        rdf:type    core:ComponentCertificationLevel , owl:NamedIndividual;
        rdfs:label  "Trust Security Profile Certification of Components based on High Assurance Evaluation"@en;
        core:includedCertificationLevel
                <https://w3id.org/idsa/code/COMPONENT_TRUST_SECURITY_PROFILE_CONCEPT_REVIEW> .

<https://w3id.org/idsa/code/CONFIG_ENDPOINT>
        rdf:type      core:AppEndpointType , owl:NamedIndividual;
        rdfs:comment  "Endpoint is used for runtime-related app configurations and app parameters."@en;
        rdfs:label    "Config endpoint"@en .

<https://w3id.org/idsa/code/CONNECTOR>
        rdf:type      odrl:LeftOperand , owl:NamedIndividual;
        rdfs:comment  "Accepts an IDS connector URI."@en;
        rdfs:label    "connector" .

<https://w3id.org/idsa/code/CONNECTOR_BADLY_CONFIGURED>
        rdf:type      core:ConnectorStatus , owl:NamedIndividual;
        rdfs:comment  "Indicates that a Connector is badly configured."@en;
        rdfs:label    "Connector badly configured"@en .

<https://w3id.org/idsa/code/CONNECTOR_OFFLINE>
        rdf:type      core:ConnectorStatus , owl:NamedIndividual;
        rdfs:comment  "Indicates that a Connector is offline."@en;
        rdfs:label    "Connector Offline"@en .

<https://w3id.org/idsa/code/CONNECTOR_ONLINE>
        rdf:type      core:ConnectorStatus , owl:NamedIndividual;
        rdfs:comment  "Indicates that a Connector is online."@en;
        rdfs:label    "Connector Online"@en .

<https://w3id.org/idsa/code/CONNECTOR_RESTRICTED_DATA_USAGE>
        rdf:type      core:UsagePolicyClass , owl:NamedIndividual;
        rdfs:comment  "This policy restrict the usage of the data to a specific IDS connector."@en;
        rdfs:label    "Connector restricted data usage"@en .

<https://w3id.org/idsa/code/CONTAINS>
        rdf:type      core:BinaryOperator , owl:NamedIndividual;
        rdfs:comment  "If a TemporalEntity (or xsd:dateTimeStamp) T1 contains another time:TemporalEntity T2, then the beginning of T1 is idsc:AFTER the beginning of T2 and the ending of T1 is idsc:BEFORE the ending of T2. An Instant (or xsd:dateTimeStamp) cannot contain another Instant (or xsd:dateTimeStamp), neihter contains itself."@en;
        rdfs:label    "contains"@en;
        rdfs:seeAlso  <http://www.w3.org/2006/time#intervalContains> , <http://www.w3.org/2006/time#inside>;
        skos:note     "Compares an instance of time:Instant, time:Interval or xsd:dateTimeStamp with an instance of time:Interval. Evaluates to false if compared to a non time:Interval."@en .

<https://w3id.org/idsa/code/CONTINUOUS>
        rdf:type          core:Frequency , skos:Concept , owl:NamedIndividual;
        rdfs:comment      "The event repeats without interruption."@en;
        rdfs:isDefinedBy  <http://purl.org/cld/freq/>;
        rdfs:label        "Continuous"@en;
        rdfs:seeAlso      <https://www.loc.gov/marc/holdings/hd853855.html>;
        dcam:memberOf     <http://purl.org/cld/terms/Frequency>;
        skos:inScheme     <http://purl.org/cld/terms/Frequency>;
        skos:prefLabel    "Continuous"@en .

<https://w3id.org/idsa/code/COUNT>
        rdf:type      odrl:LeftOperand , owl:NamedIndividual;
        rdfs:comment  "Numeric count of executions of the Rule. Operators can be idsc:LT, idsc:LTEQ, idsc:EQ, idsc:GT, idsc:GTEQ. Datatype is xsd:double."@en;
        rdfs:label    "count"@en;
        skos:broader  odrl:count .

<https://w3id.org/idsa/code/COVERED_BY>
        rdf:type      core:BinaryOperator , owl:NamedIndividual;
        rdfs:comment  "Spatial operator 'covered by' as defined by the Egenhofer Topological Relations family: An object A is covered_by another object B if both objects share common bounding and interior faces; if A has interior faces which are bounding faces of B; and if none of B's interior faces are part of A's boundary. (https://doi.org/10.1007/3-540-51295-0_148 Definition 7)"@en;
        rdfs:label    "covered by"@en;
        rdfs:seeAlso  <http://www.opengis.net/ont/geosparql#ehCoveredBy> .

<https://w3id.org/idsa/code/COVERS>
        rdf:type      core:BinaryOperator , owl:NamedIndividual;
        rdfs:comment  "Spatial operator 'covers' as defined by the Egenhofer Topological Relations family: An object A covers another object B if both objects share common bounding and interior faces; if B has interior faces which are bounding faces of A; and if none of A's interior faces are part of B's boundary. (https://doi.org/10.1007/3-540-51295-0_148 Definition 6)"@en;
        rdfs:label    "covers"@en;
        rdfs:seeAlso  <http://www.opengis.net/ont/geosparql#ehCovers> .

<https://w3id.org/idsa/code/CR>
        rdf:type    core:Language , owl:NamedIndividual;
        rdfs:label  "Cree"@en .

<https://w3id.org/idsa/code/CS>
        rdf:type    core:Language , owl:NamedIndividual;
        rdfs:label  "Czech"@en .

<https://w3id.org/idsa/code/CU>
        rdf:type    core:Language , owl:NamedIndividual;
        rdfs:label  "Old Church Slavonic, Church Slavonic, Old Bulgarian"@en .

<https://w3id.org/idsa/code/CV>
        rdf:type    core:Language , owl:NamedIndividual;
        rdfs:label  "Chuvash"@en .

<https://w3id.org/idsa/code/CY>
        rdf:type    core:Language , owl:NamedIndividual;
        rdfs:label  "Welsh"@en .

<https://w3id.org/idsa/code/DA>
        rdf:type    core:Language , owl:NamedIndividual;
        rdfs:label  "Danish"@en .

<https://w3id.org/idsa/code/DAILY>
        rdf:type          core:Frequency , skos:Concept , owl:NamedIndividual;
        rdfs:comment      "The event occurs once a day."@en;
        rdfs:isDefinedBy  <http://purl.org/cld/freq/>;
        rdfs:label        "Daily"@en;
        rdfs:seeAlso      <https://www.loc.gov/marc/holdings/hd853855.html>;
        dcam:memberOf     <http://purl.org/cld/terms/Frequency>;
        skos:inScheme     <http://purl.org/cld/terms/Frequency>;
        skos:prefLabel    "Daily"@en .

<https://w3id.org/idsa/code/DATA_RENTAL>
        rdf:type      core:UsagePolicyClass , owl:NamedIndividual;
        rdfs:comment  "This policy restricts transfer of data in return for a monthly fee. The ending is not specified. Nevertheless, the policy ends when a notice of termination has been made by any of the policy partners."@en;
        rdfs:label    "Data rental"@en .

<https://w3id.org/idsa/code/DATE_TIME>
        rdf:type      odrl:LeftOperand , owl:NamedIndividual;
        rdfs:comment  "The date and time of exercising the action of the Rule. Right operand value must be an xsd:dateTimeStamp."@en;
        rdfs:label    "date time"@en .

<https://w3id.org/idsa/code/DE>
        rdf:type    core:Language , owl:NamedIndividual;
        rdfs:label  "German"@en .

<https://w3id.org/idsa/code/DEBUG_LEVEL_LOGGING>
        rdf:type      core:LogLevel , owl:NamedIndividual;
        rdfs:comment  "Debug level logging."@en;
        rdfs:label    "Debug Level Logging"@en .

<https://w3id.org/idsa/code/DEFINES_AS>
        rdf:type      core:BinaryOperator , owl:NamedIndividual;
        rdfs:comment  "Allows assignments similar to 'var x := {RightOperand}'."@en;
        rdfs:label    "defines as"@en;
        skos:note     "Different to the other ids:BinaryOperator, idsc:DEFINES_AS does *not* compare a feature but tells the interpreter where to *find* one. Therefore, the constraint is not evaluated in the same way as with other operators."@en .

<https://w3id.org/idsa/code/DELAY>
        rdf:type      odrl:LeftOperand , owl:NamedIndividual;
        rdfs:comment  "Delay the action. Use idsc:DURATION_EQ, idsc:LONGER, idsc:LONGER_EQ, idsc:SHORTER_EQ, or idsc:SHORTER with datatype xsd:duration."@en;
        rdfs:label    "delay"@en .

<https://w3id.org/idsa/code/DELETE>
        rdf:type         odrl:Action , owl:NamedIndividual;
        rdfs:comment     "To remove a resource or inhibit any further access with reasonable measures."@en;
        rdfs:label       "delete"@en;
        skos:broader     odrl:delete;
        skos:note        "This action is evaluated at the consumer side if used in a duty clause. A provider cannot be forced to delete its data resources. If used in a permission clause, it is effecting the data provider as it allows the consumer to delete the provider's resource remotely."@en;
        odrl:includedIn  <https://w3id.org/idsa/code/WRITE> .

<https://w3id.org/idsa/code/DISJOINT>
        rdf:type      core:BinaryOperator , owl:NamedIndividual;
        rdfs:comment  "Spatial operator 'disjoint' as defined by the Egenhofer Topological Relations family: If all four intersections among all object parts are empty, then the two objects are disjoint. (https://doi.org/10.1007/3-540-51295-0_148 Definition 1)"@en;
        rdfs:label    "disjoint"@en;
        rdfs:seeAlso  <http://www.opengis.net/ont/geosparql#ehDisjoint> .

<https://w3id.org/idsa/code/DISTRIBUTE>
        rdf:type         odrl:Action , owl:NamedIndividual;
        rdfs:comment     "To forward or supply a resource to a third-party."@en;
        rdfs:label       "distribute"@en;
        skos:broader     odrl:distribute;
        skos:note        "This action is always evaluated at the consumer side and allows it to become a data provider of this resource."@en;
        odrl:includedIn  <https://w3id.org/idsa/code/USE> .

<https://w3id.org/idsa/code/DISTRIBUTE_ONLY_IF_ENCRYPTED>
        rdf:type      core:UsagePolicyClass , owl:NamedIndividual;
        rdfs:comment  "This policy restricts the usage of data assets with the obligation to encrypt the data asset before distribution."@en;
        rdfs:label    "Distribute only if encrypted"@en .

<https://w3id.org/idsa/code/DIVIDE>
        rdf:type      odrl:Action , owl:NamedIndividual;
        rdfs:comment  "This action modifies dividing something by something else."@en;
        rdfs:label    "divide"@en;
        skos:note     "This action modifies dividing something by something else. The field to be modified and the given value are specified in the policy as idsc:JSONPATH/idsc:XPATH and idsc:OPERAND, respectively."@en .

<https://w3id.org/idsa/code/DOWNLOAD_URL_AVAILABILITY_METRIC>
        rdf:type              dqv:Metric , owl:NamedIndividual;
        skos:definition       "Checks if all ResourceEndpoints for given resource are available and dereferenceable."@en;
        dqv:expectedDataType  xsd:boolean;
        dqv:inDimension       <https://w3id.org/idsa/code/AVAILABILITY> .

<https://w3id.org/idsa/code/DSA>
        rdf:type    core:KeyType , owl:NamedIndividual;
        rdfs:label  "DSA"@en .

<https://w3id.org/idsa/code/DURATION_EQ>
        rdf:type      core:BinaryOperator , owl:NamedIndividual;
        rdfs:comment  "If a temporal entity T1 has the same duration as another temporal entity T2, then their length or their duration is equal. Instants and xsd:dateTimeStamp Literals have always the duration 'P0Y0M0DT0H0M0S'^^xsd:duration and therefore have always the same duration."@en;
        rdfs:label    "has same duration"@en;
        rdfs:seeAlso  <http://www.w3.org/2006/time#hasTemporalDuration>;
        skos:note     "Compares an instance of time:TemporalEntity with an instance of time:TemporalEntity."@en .

<https://w3id.org/idsa/code/DURATION_RESTRICTED_DATA_USAGE>
        rdf:type      core:UsagePolicyClass , owl:NamedIndividual;
        rdfs:comment  "This policy restricts the usage of the data to a specific duration."@en;
        rdfs:label    "Duration restricted data usage"@en .

<https://w3id.org/idsa/code/DURING>
        rdf:type      core:BinaryOperator , owl:NamedIndividual;
        rdfs:comment  "If a TemporalEntity T1 is during another TemporalEntity T2, then the beginning of T1 is after the beginning of T2, and the end of T1 is before the end of T2."@en;
        rdfs:label    "during"@en;
        rdfs:seeAlso  <http://www.w3.org/2006/time#intervalDuring>;
        skos:note     "Compares an instance of time:Instant, time:Interval or xsd:dateTimeStamp with an instance of time:Interval. Evaluates to false if compared to a non time:Interval."@en .

<https://w3id.org/idsa/code/DV>
        rdf:type    core:Language , owl:NamedIndividual;
        rdfs:label  "Divehi, Dhivehi, Maldivian"@en .

<https://w3id.org/idsa/code/DZ>
        rdf:type    core:Language , owl:NamedIndividual;
        rdfs:label  "Dzongkha"@en .

<https://w3id.org/idsa/code/ECDSA>
        rdf:type    core:KeyType , owl:NamedIndividual;
        rdfs:label  "ECDSA"@en .

<https://w3id.org/idsa/code/ED25519>
        rdf:type    core:KeyType , owl:NamedIndividual;
        rdfs:label  "ED25519"@en .

<https://w3id.org/idsa/code/EE>
        rdf:type    core:Language , owl:NamedIndividual;
        rdfs:label  "Ewe"@en .

<https://w3id.org/idsa/code/EL>
        rdf:type    core:Language , owl:NamedIndividual;
        rdfs:label  "Greek (modern)"@en .

<https://w3id.org/idsa/code/ELAPSED_TIME>
        rdf:type      odrl:LeftOperand , owl:NamedIndividual;
        rdfs:comment  "A continuous elapsed time period which may be used for exercising of the action of the Rule. Allowed operators are idsc:SHORTER, idsc:SHORTER_EQ, idsc:LONGER, idsc:LONGER_EQ, and idsc:DURATION_EQ with datatype xsd:duration."@en;
        rdfs:label    "elapsed time"@en;
        skos:broader  odrl:elapsedTime .

<https://w3id.org/idsa/code/EN>
        rdf:type    core:Language , owl:NamedIndividual;
        rdfs:label  "English"@en .

<https://w3id.org/idsa/code/ENCRYPT>
        rdf:type         odrl:Action , owl:NamedIndividual;
        rdfs:comment     "The data artifact or parts of it are encrypted and can not be read by neither the ids:DataConsumer nor any other third party. The encryption algorithm might be specified by a constraint."@en;
        rdfs:label       "encrypt"@en;
        skos:note        "This action is always evaluated at the provider side."@en;
        odrl:includedIn  <https://w3id.org/idsa/code/USE> .

<https://w3id.org/idsa/code/ENCRYPTED>
        rdf:type      core:ArtifactState , owl:NamedIndividual;
        rdfs:comment  "The artifact is encrypted so the data itself cannot be read by any user without having the corresponding key."@en;
        rdfs:label    "is encrypted"@en .

<https://w3id.org/idsa/code/ENDPOINT>
        rdf:type      odrl:LeftOperand , owl:NamedIndividual;
        rdfs:comment  "Remote target for an action or information provider (PIP). Must be used together with idsc:IS or idsc:IN operators. RightOperand must be a xsd:anyURI or an URL which should point to an actually deployed endpoint. An example is a refinement of idsc:NOTIFY where idsc:REMOTE points to a Clearing House."@en;
        rdfs:label    "endpoint" .

<https://w3id.org/idsa/code/EO>
        rdf:type    core:Language , owl:NamedIndividual;
        rdfs:label  "Esperanto"@en .

<https://w3id.org/idsa/code/EQ>
        rdf:type      core:BinaryOperator , owl:NamedIndividual;
        rdfs:comment  "Arithmetic equals operator (5 = 5)."@en;
        rdfs:label    "equals"@en;
        skos:broader  odrl:eq .

<https://w3id.org/idsa/code/EQUALS>
        rdf:type      core:BinaryOperator , owl:NamedIndividual;
        rdfs:comment  "Logical equals operator (true = true)."@en;
        rdfs:label    "equals"@en;
        skos:broader  odrl:eq .

<https://w3id.org/idsa/code/ES>
        rdf:type    core:Language , owl:NamedIndividual;
        rdfs:label  "Spanish"@en .

<https://w3id.org/idsa/code/ET>
        rdf:type    core:Language , owl:NamedIndividual;
        rdfs:label  "Estonian"@en .

<https://w3id.org/idsa/code/EU>
        rdf:type    core:Language , owl:NamedIndividual;
        rdfs:label  "Basque"@en .

<https://w3id.org/idsa/code/EVENT>
        rdf:type      odrl:LeftOperand , owl:NamedIndividual;
        rdfs:comment  "The feature dimension regarding whether current events are happening. Does NOT refer 'events' as in real-time data, sensor observations, or Complex Event Processing but rather as 'World Cup 2018' or 'Hannover Trade Fair'."@en;
        rdfs:label    "current event"@en .

<https://w3id.org/idsa/code/EVENT_RESTRICTED_DATA_USAGE>
        rdf:type      core:UsagePolicyClass , owl:NamedIndividual;
        rdfs:comment  "This policy restricts the usage of data assets limited to specific events.\n\t\t\t\t\tThe ODRL language defines an identified event as a context for exercising the action of the Rule. \n\t\t\t\t\tEvents are temporal periods of time. A Data Provider may want to restrict the usage of the data to a specific event when the exact time and date of the event is not clear in advance. \n\t\t\t\t\tTherefore, the event condition can be specified in a policy."@en;
        rdfs:label    "Event restricted data usage"@en .

<https://w3id.org/idsa/code/EVERY_10_MINUTES>
        rdf:type      core:Frequency , skos:Concept , owl:NamedIndividual;
        rdfs:comment  "The event occurs every 10 minutes."@en;
        rdfs:label    "Every 10 minutes"@en .

<https://w3id.org/idsa/code/EVERY_15_MINUTES>
        rdf:type      core:Frequency , skos:Concept , owl:NamedIndividual;
        rdfs:comment  "The event occurs every 15 minutes."@en;
        rdfs:label    "Every 15 minutes"@en .

<https://w3id.org/idsa/code/EVERY_1_MINUTE>
        rdf:type      core:Frequency , skos:Concept , owl:NamedIndividual;
        rdfs:comment  "The event occurs every 1 minute."@en;
        rdfs:label    "Every 1 minutes"@en .

<https://w3id.org/idsa/code/EVERY_30_MINUTES>
        rdf:type      core:Frequency , skos:Concept , owl:NamedIndividual;
        rdfs:comment  "The event occurs every 30 minutes."@en;
        rdfs:label    "Every 30 minutes"@en .

<https://w3id.org/idsa/code/EVERY_5_MINUTES>
        rdf:type      core:Frequency , skos:Concept , owl:NamedIndividual;
        rdfs:comment  "The event occurs every 5 minutes."@en;
        rdfs:label    "Every 5 minutes"@en .

<https://w3id.org/idsa/code/EVERY_THREE_HOURS>
        rdf:type      core:Frequency , skos:Concept , owl:NamedIndividual;
        rdfs:comment  "The event occurs every three hours."@en;
        rdfs:label    "Every three hours"@en .

<https://w3id.org/idsa/code/FA>
        rdf:type    core:Language , owl:NamedIndividual;
        rdfs:label  "Persian (Farsi)"@en .

<https://w3id.org/idsa/code/FF>
        rdf:type    core:Language , owl:NamedIndividual;
        rdfs:label  "Fula, Fulah, Pulaar, Pular"@en .

<https://w3id.org/idsa/code/FI>
        rdf:type    core:Language , owl:NamedIndividual;
        rdfs:label  "Finnish"@en .

<https://w3id.org/idsa/code/FINISHED_BY>
        rdf:type      core:BinaryOperator , owl:NamedIndividual;
        rdfs:comment  "If an interval T1 is finished by another interval T2, then the beginning of T1 is before the beginning of T2, and the end of T1 is coincident with the end of T2."@en;
        rdfs:label    "finished by"@en;
        rdfs:seeAlso  <http://www.w3.org/2006/time#intervalFinishedBy>;
        skos:note     "Compares an instance of time:Interval to another instance of time:Interval. Evaluates to false if compared to a non time:Interval or one interval is empty."@en .

<https://w3id.org/idsa/code/FINISHES>
        rdf:type      core:BinaryOperator , owl:NamedIndividual;
        rdfs:comment  "If an Interval T1 finishes another interval T2, then the beginning of T1 is after the beginning of T2, and the end of T1 is coincident with the end of T2."@en;
        rdfs:label    "finishes"@en;
        rdfs:seeAlso  core:intervalIn , <http://www.w3.org/2006/time#intervalFinishes>;
        skos:note     "Compares an instance of time:Interval to another instance of time:Interval. Evaluates to false if compared to a non time:Interval or one interval is empty."@en .

<https://w3id.org/idsa/code/FIXED_PRICE>
        rdf:type      core:PaymentModality , owl:NamedIndividual;
        rdfs:comment  "To express that the exchange of resource is with a fixed price"@en;
        rdfs:label    "fixed price"@en .

<https://w3id.org/idsa/code/FJ>
        rdf:type    core:Language , owl:NamedIndividual;
        rdfs:label  "Fijian"@en .

<https://w3id.org/idsa/code/FO>
        rdf:type    core:Language , owl:NamedIndividual;
        rdfs:label  "Faroese"@en .

<https://w3id.org/idsa/code/FR>
        rdf:type    core:Language , owl:NamedIndividual;
        rdfs:label  "French"@en .

<https://w3id.org/idsa/code/FREE>
        rdf:type      core:PaymentModality , owl:NamedIndividual;
        rdfs:comment  "To express that the exchange of resource is free"@en;
        rdfs:label    "free"@en .

<https://w3id.org/idsa/code/FY>
        rdf:type    core:Language , owl:NamedIndividual;
        rdfs:label  "Western Frisian"@en .

<https://w3id.org/idsa/code/GA>
        rdf:type    core:Language , owl:NamedIndividual;
        rdfs:label  "Irish"@en .

<https://w3id.org/idsa/code/GD>
        rdf:type    core:Language , owl:NamedIndividual;
        rdfs:label  "Scottish Gaelic, Gaelic"@en .

<https://w3id.org/idsa/code/GL>
        rdf:type    core:Language , owl:NamedIndividual;
        rdfs:label  "Galician"@en .

<https://w3id.org/idsa/code/GN>
        rdf:type    core:Language , owl:NamedIndividual;
        rdfs:label  "Guaraní"@en .

<https://w3id.org/idsa/code/GRANT_USE>
        rdf:type         odrl:Action , owl:NamedIndividual;
        rdfs:comment     "To grant use of a resource to another party. Does *not* imply any other usage rights."@en;
        rdfs:label       "grant use"@en;
        skos:broader     odrl:grantUse;
        skos:note        "This action is always evaluated at the consumer side, at the moment a third party intends to access the resource as received by the original consumer."@en;
        odrl:includedIn  <https://w3id.org/idsa/code/USE> .

<https://w3id.org/idsa/code/GT>
        rdf:type      core:BinaryOperator , owl:NamedIndividual;
        rdfs:comment  "Greater-than operator. Can be used for numeric (5 idsc:GT 2) comparisons."@en;
        rdfs:label    "greater than"@en;
        skos:broader  odrl:gt .

<https://w3id.org/idsa/code/GTEQ>
        rdf:type      core:BinaryOperator , owl:NamedIndividual;
        rdfs:comment  "Greater-than-or-equals operator. Can be used for numeric (5 idsc:GTEQ 2) comparisons."@en;
        rdfs:label    "greater than or equals"@en;
        skos:broader  odrl:gteq .

<https://w3id.org/idsa/code/GU>
        rdf:type    core:Language , owl:NamedIndividual;
        rdfs:label  "Gujarati"@en .

<https://w3id.org/idsa/code/GV>
        rdf:type    core:Language , owl:NamedIndividual;
        rdfs:label  "Manx"@en .

<https://w3id.org/idsa/code/HA>
        rdf:type    core:Language , owl:NamedIndividual;
        rdfs:label  "Hausa"@en .

<https://w3id.org/idsa/code/HASH>
        rdf:type      odrl:Action , owl:NamedIndividual;
        rdfs:comment  "This action modifies a value by replacing it with a hash of the value."@en;
        rdfs:label    "hash"@en;
        skos:note     "This action modifies a value by replacing it with a hash of the value. The field to be modified and the hash algorithm are specified in the policy as idsc:JSONPATH/idsc:XPATH and idsc:HASH_ALGORITHM (eg. SHA256), respectively."@en .

<https://w3id.org/idsa/code/HASH_ALGORITHM>
        rdf:type      odrl:LeftOperand , owl:NamedIndividual;
        rdfs:comment  "Indicate the hash value to be used, eg.SHA256."@en;
        rdfs:label    "hash algorithm"@en .

<https://w3id.org/idsa/code/HAS_MEMBERSHIP>
        rdf:type      core:BinaryOperator , owl:NamedIndividual;
        rdfs:comment  "If a user has a specific membership required for accessing a resource. A membership includes always a role and a related organisation (see also org:). Should be used together with a RightOperand pointing to an accessible endpoint providing this information."@en;
        rdfs:label    "has Member"@en;
        rdfs:seeAlso  org:hasMember .

<https://w3id.org/idsa/code/HAS_SITE>
        rdf:type      core:BinaryOperator , owl:NamedIndividual;
        rdfs:comment  "If a user needs to be located at a certain site required for accessing a resource. A 'HAS_SITE' relation includes always a membership (role and related organisation) corresponding to the site. Should be used together with a RightOperand pointing to an accessible endpoint providing this information."@en;
        rdfs:label    "has site"@en;
        rdfs:seeAlso  org:basedAt .

<https://w3id.org/idsa/code/HAS_STATE>
        rdf:type      core:BinaryOperator , owl:NamedIndividual;
        rdfs:comment  "Operator examining if the target resource has a certain state at the moment, for instance is anonymized (idsc:ANONYMIZED)."@en;
        rdfs:label    "has state"@en .

<https://w3id.org/idsa/code/HE>
        rdf:type    core:Language , owl:NamedIndividual;
        rdfs:label  "Hebrew (modern)"@en .

<https://w3id.org/idsa/code/HI>
        rdf:type    core:Language , owl:NamedIndividual;
        rdfs:label  "Hindi"@en .

<https://w3id.org/idsa/code/HO>
        rdf:type    core:Language , owl:NamedIndividual;
        rdfs:label  "Hiri Motu"@en .

<https://w3id.org/idsa/code/HOURLY>
        rdf:type      core:Frequency , skos:Concept , owl:NamedIndividual;
        rdfs:comment  "The event occurs every hour."@en;
        rdfs:label    "Hourly"@en .

<https://w3id.org/idsa/code/HR>
        rdf:type    core:Language , owl:NamedIndividual;
        rdfs:label  "Croatian"@en .

<https://w3id.org/idsa/code/HT>
        rdf:type    core:Language , owl:NamedIndividual;
        rdfs:label  "Haitian, Haitian Creole"@en .

<https://w3id.org/idsa/code/HU>
        rdf:type    core:Language , owl:NamedIndividual;
        rdfs:label  "Hungarian"@en .

<https://w3id.org/idsa/code/HY>
        rdf:type    core:Language , owl:NamedIndividual;
        rdfs:label  "Armenian"@en .

<https://w3id.org/idsa/code/HZ>
        rdf:type    core:Language , owl:NamedIndividual;
        rdfs:label  "Herero"@en .

<https://w3id.org/idsa/code/IA>
        rdf:type    core:Language , owl:NamedIndividual;
        rdfs:label  "Interlingua"@en .

<https://w3id.org/idsa/code/ID>
        rdf:type    core:Language , owl:NamedIndividual;
        rdfs:label  "Indonesian"@en .

<https://w3id.org/idsa/code/IDS-CP>
        rdf:type      core:IdsProtocolSpecification , owl:NamedIndividual;
        rdfs:comment  "The IDS-CP specification of the IDS interactions."@en;
        rdfs:label    "IDS-CP";
        rdfs:seeAlso  <https://github.com/International-Data-Spaces-Association/path/to/idscp/spec/> .

<https://w3id.org/idsa/code/IDS-REST>
        rdf:type      core:IdsProtocolSpecification , owl:NamedIndividual;
        rdfs:comment  "The REST specification of the IDS interactions."@en;
        rdfs:label    "IDS REST";
        rdfs:seeAlso  <https://github.com/International-Data-Spaces-Association/path/to/ids/rest/spec/> .

<https://w3id.org/idsa/code/IDS_CONNECTOR_ATTRIBUTES_ALL>
        rdf:type      core:Audience , owl:NamedIndividual;
        rdfs:comment  "Every IDS Connector is in the intended audience for the DAT with this 'scope' property."@en;
        rdfs:label    "all IDS Connectors" .

<https://w3id.org/idsa/code/IE>
        rdf:type    core:Language , owl:NamedIndividual;
        rdfs:label  "Interlingue"@en .

<https://w3id.org/idsa/code/IG>
        rdf:type    core:Language , owl:NamedIndividual;
        rdfs:label  "Igbo"@en .

<https://w3id.org/idsa/code/II>
        rdf:type    core:Language , owl:NamedIndividual;
        rdfs:label  "Nuosu"@en .

<https://w3id.org/idsa/code/IK>
        rdf:type    core:Language , owl:NamedIndividual;
        rdfs:label  "Inupiaq"@en .

<https://w3id.org/idsa/code/IN>
        rdf:type      core:BinaryOperator , owl:NamedIndividual;
        rdfs:comment  "Element-of operator. Allowed RightOperands are RDF collections('(A B C)')."@en;
        rdfs:label    "in"@en;
        skos:broader  <https://postgis.net/docs/ST_Within.html> , odrl:isAnyOf .

<https://w3id.org/idsa/code/INCREMENT_COUNTER>
        rdf:type      odrl:Action , owl:NamedIndividual;
        rdfs:comment  "An action to be used in the count usage policy where the idsc:COUNT left operand is used."@en;
        rdfs:label    "increment counter"@en .

<https://w3id.org/idsa/code/INPUT_ENDPOINT>
        rdf:type      core:AppEndpointType , owl:NamedIndividual;
        rdfs:comment  "Endpoint is used for data input."@en;
        rdfs:label    "Input endpoint"@en .

<https://w3id.org/idsa/code/INSIDE>
        rdf:type      core:BinaryOperator , owl:NamedIndividual;
        rdfs:comment  "Spatial operator 'inside' as defined by the Egenhofer Topological Relations family: An object A is inside of another object B if (1) A and B share interior, but not bounding faces, (2) if A has bounding faces which are interior faces of B, and (3) none of B's bounding faces coincides with any of A's interior faces. (https://doi.org/10.1007/3-540-51295-0_148 Definition 4)"@en;
        rdfs:label    "inside"@en;
        rdfs:seeAlso  <http://www.opengis.net/ont/geosparql#ehInside>;
        skos:note     "In addition, a point is inside a polygom iff the point is in the polygom's interior (the point itself has no interior)."@en .

<https://w3id.org/idsa/code/INSIDE_NETWORK>
        rdf:type      core:BinaryOperator , owl:NamedIndividual;
        rdfs:comment  "Is satisfied if a system is inside a specified target network or network range."@en;
        rdfs:label    "inside network"@en .

<https://w3id.org/idsa/code/INTEGRITY_PROTECTION_LOCAL>
        rdf:type    core:IntegrityGuarantee , owl:NamedIndividual;
        rdfs:label  "Integrity Protection Local" .

<https://w3id.org/idsa/code/INTEGRITY_PROTECTION_NONE>
        rdf:type    core:IntegrityGuarantee , owl:NamedIndividual;
        rdfs:label  "Integrity Protection None" .

<https://w3id.org/idsa/code/INTEGRITY_VERIFICATION_REMOTE>
        rdf:type    core:IntegrityGuarantee , owl:NamedIndividual;
        rdfs:label  "Integrity Protection Remote" .

<https://w3id.org/idsa/code/INTEGRITY_VERIFICATION_SCOPE_KERNEL_CORE_CONTAINER>
        rdf:type    core:IntegrityVerificationScopeGuarantee , owl:NamedIndividual;
        rdfs:label  "Integrity Verification Scope Kernel Core Container" .

<https://w3id.org/idsa/code/INTEGRITY_VERIFICATION_SCOPE_KERNEL_CORE_CONTAINER_APPLICATION>
        rdf:type    core:IntegrityVerificationScopeGuarantee , owl:NamedIndividual;
        rdfs:label  "Integrity Verification Scope Kernel Core Container Application" .

<https://w3id.org/idsa/code/INTEGRITY_VERIFICATION_SCOPE_NONE>
        rdf:type    core:IntegrityVerificationScopeGuarantee , owl:NamedIndividual;
        rdfs:label  "Integrity Verification Scope None" .

<https://w3id.org/idsa/code/INTERFACE_DEFINITION>
        rdf:type      terms:DCMIType , owl:NamedIndividual;
        rdfs:comment  "Formal, machine-interpretable definition of a protocol-specific API, e.g., OpenAPI, GraphQL, API Blueprint, WSDL."@en;
        rdfs:label    "Interface definition" .

<https://w3id.org/idsa/code/INTERNAL_RECIPIENT_ERROR>
        rdf:type      core:RejectionReason , owl:NamedIndividual;
        rdfs:comment  "The message recipient encountered an internal error while processing the message (e.g., storage capacity exceeded).";
        rdfs:label    "INTERNAL_RECIPIENT_ERROR" .

<https://w3id.org/idsa/code/INTERVAL_RESTRICTED_DATA_USAGE>
        rdf:type      core:UsagePolicyClass , owl:NamedIndividual;
        rdfs:comment  "This policy restricts the usage of the data to a specific (time) interval."@en;
        rdfs:label    "Interval restricted data usage"@en .

<https://w3id.org/idsa/code/IO>
        rdf:type    core:Language , owl:NamedIndividual;
        rdfs:label  "Ido"@en .

<https://w3id.org/idsa/code/IRREGULAR>
        rdf:type          core:Frequency , skos:Concept , owl:NamedIndividual;
        rdfs:comment      "The event occurs at uneven intervals."@en;
        rdfs:isDefinedBy  <http://purl.org/cld/freq/>;
        rdfs:label        "Irregular"@en;
        rdfs:seeAlso      <https://www.loc.gov/marc/holdings/hd853855.html>;
        dcam:memberOf     <http://purl.org/cld/terms/Frequency>;
        skos:inScheme     <http://purl.org/cld/terms/Frequency>;
        skos:prefLabel    "Irregular"@en .

<https://w3id.org/idsa/code/IS>
        rdf:type    core:Language , owl:NamedIndividual;
        rdfs:label  "Icelandic"@en .

<https://w3id.org/idsa/code/IT>
        rdf:type    core:Language , owl:NamedIndividual;
        rdfs:label  "Italian"@en .

<https://w3id.org/idsa/code/IU>
        rdf:type    core:Language , owl:NamedIndividual;
        rdfs:label  "Inuktitut"@en .

<https://w3id.org/idsa/code/JA>
        rdf:type    core:Language , owl:NamedIndividual;
        rdfs:label  "Japanese"@en .

<https://w3id.org/idsa/code/JSON_PATH>
        rdf:type      odrl:LeftOperand , owl:NamedIndividual;
        rdfs:comment  "An expression that refers to a part of a JSON structured data."@en;
        rdfs:label    "json path"@en .

<https://w3id.org/idsa/code/JV>
        rdf:type    core:Language , owl:NamedIndividual;
        rdfs:label  "Javanese"@en .

<https://w3id.org/idsa/code/JWT>
        rdf:type    core:TokenFormat , owl:NamedIndividual;
        rdfs:label  "Json Web Token" .

<https://w3id.org/idsa/code/KA>
        rdf:type    core:Language , owl:NamedIndividual;
        rdfs:label  "Georgian"@en .

<https://w3id.org/idsa/code/KG>
        rdf:type    core:Language , owl:NamedIndividual;
        rdfs:label  "Kongo"@en .

<https://w3id.org/idsa/code/KI>
        rdf:type    core:Language , owl:NamedIndividual;
        rdfs:label  "Kikuyu, Gikuyu"@en .

<https://w3id.org/idsa/code/KJ>
        rdf:type    core:Language , owl:NamedIndividual;
        rdfs:label  "Kwanyama, Kuanyama"@en .

<https://w3id.org/idsa/code/KK>
        rdf:type    core:Language , owl:NamedIndividual;
        rdfs:label  "Kazakh"@en .

<https://w3id.org/idsa/code/KL>
        rdf:type    core:Language , owl:NamedIndividual;
        rdfs:label  "Kalaallisut, Greenlandic"@en .

<https://w3id.org/idsa/code/KM>
        rdf:type    core:Language , owl:NamedIndividual;
        rdfs:label  "Khmer"@en .

<https://w3id.org/idsa/code/KN>
        rdf:type    core:Language , owl:NamedIndividual;
        rdfs:label  "Kannada"@en .

<https://w3id.org/idsa/code/KO>
        rdf:type    core:Language , owl:NamedIndividual;
        rdfs:label  "Korean"@en .

<https://w3id.org/idsa/code/KR>
        rdf:type    core:Language , owl:NamedIndividual;
        rdfs:label  "Kanuri"@en .

<https://w3id.org/idsa/code/KS>
        rdf:type    core:Language , owl:NamedIndividual;
        rdfs:label  "Kashmiri"@en .

<https://w3id.org/idsa/code/KU>
        rdf:type    core:Language , owl:NamedIndividual;
        rdfs:label  "Kurdish"@en .

<https://w3id.org/idsa/code/KV>
        rdf:type    core:Language , owl:NamedIndividual;
        rdfs:label  "Komi"@en .

<https://w3id.org/idsa/code/KW>
        rdf:type    core:Language , owl:NamedIndividual;
        rdfs:label  "Cornish"@en .

<https://w3id.org/idsa/code/KY>
        rdf:type    core:Language , owl:NamedIndividual;
        rdfs:label  "Kyrgyz"@en .

<https://w3id.org/idsa/code/LA>
        rdf:type    core:Language , owl:NamedIndividual;
        rdfs:label  "Latin"@en .

<https://w3id.org/idsa/code/LB>
        rdf:type    core:Language , owl:NamedIndividual;
        rdfs:label  "Luxembourgish, Letzeburgesch"@en .

<https://w3id.org/idsa/code/LG>
        rdf:type    core:Language , owl:NamedIndividual;
        rdfs:label  "Ganda"@en .

<https://w3id.org/idsa/code/LI>
        rdf:type    core:Language , owl:NamedIndividual;
        rdfs:label  "Limburgish, Limburgan, Limburger"@en .

<https://w3id.org/idsa/code/LN>
        rdf:type    core:Language , owl:NamedIndividual;
        rdfs:label  "Lingala"@en .

<https://w3id.org/idsa/code/LO>
        rdf:type    core:Language , owl:NamedIndividual;
        rdfs:label  "Lao"@en .

<https://w3id.org/idsa/code/LOCAL_DATA_CONFIDENTIALITY_FULL_ENCRYPTION>
        rdf:type    core:LocalDataConfidentialityGuarantee , owl:NamedIndividual;
        rdfs:label  "Local Data Confidentiality Full Encryption" .

<https://w3id.org/idsa/code/LOCAL_DATA_CONFIDENTIALITY_NONE>
        rdf:type    core:LocalDataConfidentialityGuarantee , owl:NamedIndividual;
        rdfs:label  "Local Data Confidentiality None" .

<https://w3id.org/idsa/code/LOCAL_DATA_CONFIDENTIALITY_SECURE_ERASURE>
        rdf:type    core:LocalDataConfidentialityGuarantee , owl:NamedIndividual;
        rdfs:label  "Local Data Confidentiality Secure Erasure" .

<https://w3id.org/idsa/code/LOCAL_LOGGING>
        rdf:type      core:UsagePolicyClass , owl:NamedIndividual;
        rdfs:comment  "This policy restricts the usage of data assets with the obligation to log prior specified processes, such as the data access."@en;
        rdfs:label    "Local logging"@en .

<https://w3id.org/idsa/code/LOCATION_RESTRICTED_DATA_USAGE>
        rdf:type      core:UsagePolicyClass , owl:NamedIndividual;
        rdfs:comment  "This policy restricts the usage of the data to a specific location, e.g., expressed via location areas, geographic points or geographic bounding polygons."@en;
        rdfs:label    "Location restricted data usage"@en .

<https://w3id.org/idsa/code/LOG>
        rdf:type         odrl:Action , owl:NamedIndividual;
        rdfs:comment     "To log information or store information about incidents in a local file or database. Is not necessarily available to external parties but can be used to create transparency on happened events."@en;
        rdfs:label       "log"@en;
        skos:note        "This action is always evaluated at the consumer side."@en;
        odrl:includedIn  <https://w3id.org/idsa/code/USE> .

<https://w3id.org/idsa/code/LOG_LEVEL>
        rdf:type      odrl:LeftOperand , owl:NamedIndividual;
        rdfs:comment  "Accepted values: ON_DENY, ON_ALLOW, ON_DUTY_EXERCISED, ON_ACTION_OPERATED."@en;
        rdfs:label    "log level" .

<https://w3id.org/idsa/code/LONGER>
        rdf:type      core:BinaryOperator , owl:NamedIndividual;
        rdfs:comment  "If a temporal entity T1 is longer than another temporal entity T2, then the length or duration of T1 is bigger. Instants and xsd:dateTimeStamp Literals have always the duration 'P0Y0M0DT0H0M0S'^^xsd:duration and therefore have always the same duration."@en;
        rdfs:label    "longer"@en;
        skos:note     "Compares an instance of time:TemporalEntity with an instance of xsd:duration."@en .

<https://w3id.org/idsa/code/LONGER_EQ>
        rdf:type      core:BinaryOperator , owl:NamedIndividual;
        rdfs:comment  "If temporal entity T1 is longer or equals than another temporal entity T2, then the length or duration of T1 is bigger or their length or their duration is equal. Instants and xsd:dateTimeStamp Literals have always the duration 'P0Y0M0DT0H0M0S'^^xsd:duration and therefore have always the same duration."@en;
        rdfs:label    "longer or equals"@en;
        skos:note     "Compares an instance of time:TemporalEntity with an instance of xsd:duration."@en .

<https://w3id.org/idsa/code/LT>
        rdf:type      core:Language , core:BinaryOperator , owl:NamedIndividual;
        rdfs:comment  "Less-than operator. Can be used for numeric (2 idsc:LT 5) comparisons."@en;
        rdfs:label    "less than"@en , "Lithuanian"@en;
        skos:broader  odrl:lt;
        skos:note     "Do not confuse with idsc:LT (which is a language)."@en .

<https://w3id.org/idsa/code/LTEQ>
        rdf:type      core:BinaryOperator , owl:NamedIndividual;
        rdfs:comment  "Less-than-or-equals operator. Can be used for numeric (2 idsc:LTEQ 5) comparisons."@en;
        rdfs:label    "less than or equals"@en;
        skos:broader  odrl:lteq .

<https://w3id.org/idsa/code/LU>
        rdf:type    core:Language , owl:NamedIndividual;
        rdfs:label  "Luba-Katanga"@en .

<https://w3id.org/idsa/code/LV>
        rdf:type    core:Language , owl:NamedIndividual;
        rdfs:label  "Latvian"@en .

<https://w3id.org/idsa/code/MALFORMED_MESSAGE>
        rdf:type      core:RejectionReason , owl:NamedIndividual;
        rdfs:comment  "The originating message is malformed or missing information.";
        rdfs:label    "MALFORMED_MESSAGE" .

<https://w3id.org/idsa/code/MATCHES>
        rdf:type      core:BinaryOperator , owl:NamedIndividual;
        rdfs:comment  "Regex operator for strings. Evaluates to true iff the regex pattern of the RightOperand matches the LeftOperand."@en;
        rdfs:label    "matches"@en .

<https://w3id.org/idsa/code/MEETS>
        rdf:type      core:BinaryOperator , owl:NamedIndividual;
        rdfs:comment  "If a TemporalEntity or (xsd:dateTimeStamp Literal) T1 meets another TemporalEntity (or xsd:dateTimeStamp Literal) T2, then the end of T1 is coincident with the beginning of T2."@en;
        rdfs:label    "meets"@en;
        rdfs:seeAlso  <http://www.w3.org/2006/time#intervalMeets>;
        skos:note     "Compares an instance of TemporalEntity or xsd:dateTimeStamp Literal to another instance of TemporalEntity or xsd:dateTimeStamp Literal. Evaluates to true if T1 or T2 are Instants (or xsd:dateTimeStamp Literal) and the condition in the comment holds."@en .

<https://w3id.org/idsa/code/MEMBER_OF>
        rdf:type      core:BinaryOperator , owl:NamedIndividual;
        rdfs:comment  "If a user is part of a certain organisation required for accessing a resource. Should be used together with a RightOperand pointing to an accessible endpoint providing this information."@en;
        rdfs:label    "memberOf"@en;
        rdfs:seeAlso  org:memberOf .

<https://w3id.org/idsa/code/MESSAGE_TYPE_NOT_SUPPORTED>
        rdf:type      core:RejectionReason , owl:NamedIndividual;
        rdfs:comment  "The sender of the rejection does not support the incoming message type (e.g., ids:QueryMessage).";
        rdfs:label    "MESSAGE_TYPE_NOT_SUPPORTED" .

<https://w3id.org/idsa/code/METHOD_NOT_SUPPORTED>
        rdf:type      core:RejectionReason , owl:NamedIndividual;
        rdfs:comment  "The sender of the rejection does not implement a certain functionality stated in the message (e.g., query language).";
        rdfs:label    "METHOD_NOT_SUPPORTED" .

<https://w3id.org/idsa/code/MET_BY>
        rdf:type      core:BinaryOperator , owl:NamedIndividual;
        rdfs:comment  "If a TemporalEntity or (xsd:dateTimeStamp Literal) T1 is met by another TemporalEntity or (xsd:dateTimeStamp Literal) T2, then the beginning of T1 is coincident with the end of T2."@en;
        rdfs:label    "met by"@en;
        rdfs:seeAlso  <http://www.w3.org/2006/time#intervalMetBy>;
        skos:note     "Compares an instance of TemporalEntity (or xsd:dateTimeStamp Literal) to another instance of TemporalEntity (or xsd:dateTimeStamp Literal). Evaluates to true if T1 or T2 are Instants (or xsd:dateTimeStamp Literal) and the condition in the comment holds."@en .

<https://w3id.org/idsa/code/MG>
        rdf:type    core:Language , owl:NamedIndividual;
        rdfs:label  "Malagasy"@en .

<https://w3id.org/idsa/code/MH>
        rdf:type    core:Language , owl:NamedIndividual;
        rdfs:label  "Marshallese"@en .

<https://w3id.org/idsa/code/MI>
        rdf:type    core:Language , owl:NamedIndividual;
        rdfs:label  "Māori"@en .

<https://w3id.org/idsa/code/MINIMAL_LOGGING>
        rdf:type      core:LogLevel , owl:NamedIndividual;
        rdfs:comment  "Minimal logging."@en;
        rdfs:label    "Minimal Logging"@en .

<https://w3id.org/idsa/code/MK>
        rdf:type    core:Language , owl:NamedIndividual;
        rdfs:label  "Macedonian"@en .

<https://w3id.org/idsa/code/ML>
        rdf:type    core:Language , owl:NamedIndividual;
        rdfs:label  "Malayalam"@en .

<https://w3id.org/idsa/code/MN>
        rdf:type    core:Language , owl:NamedIndividual;
        rdfs:label  "Mongolian"@en .

<https://w3id.org/idsa/code/MODIFY>
        rdf:type         odrl:Action , owl:NamedIndividual;
        rdfs:comment     "To change a resource locally."@en;
        rdfs:label       "modify"@en;
        skos:broader     odrl:modify;
        skos:note        "This action is always evaluated at the consumer side. It corresponds to 'allow changes of the copied resource'."@en;
        odrl:includedIn  <https://w3id.org/idsa/code/WRITE> .

<https://w3id.org/idsa/code/MODIFY_DATA_IN_REST>
        rdf:type      core:UsagePolicyClass , owl:NamedIndividual;
        rdfs:comment  "This policy restricts the usage of data assets with the obligation to anonymize the data before permission to use the data is granted. \n\t\t\t\t\tIn contrast to the idsc:MODIFY_DATA_IN_TRANSIT policy class, it demands the modifications to be done when data is stored."@en;
        rdfs:label    "Modfy data in rest"@en .

<https://w3id.org/idsa/code/MODIFY_DATA_IN_TRANSIT>
        rdf:type      core:UsagePolicyClass , owl:NamedIndividual;
        rdfs:comment  "This policy restricts the usage of data assets with the obligation to anonymize the data when it is leaving the Data Provider connector or when it is entering the Data Consumer connector"@en;
        rdfs:label    "Modfy data in transit"@en .

<https://w3id.org/idsa/code/MONTHLY>
        rdf:type          core:Frequency , skos:Concept , owl:NamedIndividual;
        rdfs:comment      "The event occurs once a month."@en;
        rdfs:isDefinedBy  <http://purl.org/cld/freq/>;
        rdfs:label        "Monthly"@en;
        rdfs:seeAlso      <https://www.loc.gov/marc/holdings/hd853855.html>;
        dcam:memberOf     <http://purl.org/cld/terms/Frequency>;
        skos:inScheme     <http://purl.org/cld/terms/Frequency>;
        skos:prefLabel    "Monthly"@en .

<https://w3id.org/idsa/code/MR>
        rdf:type    core:Language , owl:NamedIndividual;
        rdfs:label  "Marathi (Marāṭhī)"@en .

<https://w3id.org/idsa/code/MS>
        rdf:type    core:Language , owl:NamedIndividual;
        rdfs:label  "Malay"@en .

<https://w3id.org/idsa/code/MT>
        rdf:type    core:Language , owl:NamedIndividual;
        rdfs:label  "Maltese"@en .

<https://w3id.org/idsa/code/MULTIPART>
        rdf:type      core:IdsProtocolSpecification , owl:NamedIndividual;
        rdfs:comment  "The Multipart Messages implementation of the IDS interactions."@en;
        rdfs:label    "IDS over Multipart";
        rdfs:seeAlso  <https://github.com/International-Data-Spaces-Association/path/to/multipart/spec/> .

<https://w3id.org/idsa/code/MULTIPLY>
        rdf:type      odrl:Action , owl:NamedIndividual;
        rdfs:comment  "This action modifies a number by multiplying it to a given value."@en;
        rdfs:label    "multiply"@en;
        skos:note     "This action modifies a number by multiplying it to a given value. The field to be modified and the given value are specified in the policy as idsc:JSONPATH/idsc:XPATH and idsc:OPERAND, respectively."@en .

<https://w3id.org/idsa/code/MULTI_LINGUAL>
        rdf:type      core:Language , owl:NamedIndividual;
        rdfs:comment  "Code indicates that several languages are used or no concrete language can be determined.";
        rdfs:label    "Multilingual"@en .

<https://w3id.org/idsa/code/MY>
        rdf:type    core:Language , owl:NamedIndividual;
        rdfs:label  "Burmese"@en .

<https://w3id.org/idsa/code/NA>
        rdf:type    core:Language , owl:NamedIndividual;
        rdfs:label  "Nauruan"@en .

<https://w3id.org/idsa/code/NB>
        rdf:type    core:Language , owl:NamedIndividual;
        rdfs:label  "Norwegian Bokmål"@en .

<https://w3id.org/idsa/code/ND>
        rdf:type    core:Language , owl:NamedIndividual;
        rdfs:label  "Northern Ndebele"@en .

<https://w3id.org/idsa/code/NE>
        rdf:type    core:Language , owl:NamedIndividual;
        rdfs:label  "Nepali"@en .

<https://w3id.org/idsa/code/NEGOTIATION_BASIS>
        rdf:type      core:PaymentModality , owl:NamedIndividual;
        rdfs:comment  "To express that the exchange of resource is negotiation-based."@en;
        rdfs:label    "negotiation basis"@en .

<https://w3id.org/idsa/code/NEXT_POLICY>
        rdf:type         odrl:Action , owl:NamedIndividual;
        rdfs:comment     "To forward the resource under the same policy. Implies a permission to distribute."@en;
        rdfs:label       "next policy"@en;
        skos:broader     odrl:nextPolicy;
        skos:note        "This action is always evaluated at the consumer side."@en;
        odrl:includedIn  <https://w3id.org/idsa/code/DISTRIBUTE> .

<https://w3id.org/idsa/code/NG>
        rdf:type    core:Language , owl:NamedIndividual;
        rdfs:label  "Ndonga"@en .

<https://w3id.org/idsa/code/NL>
        rdf:type    core:Language , owl:NamedIndividual;
        rdfs:label  "Dutch"@en .

<https://w3id.org/idsa/code/NN>
        rdf:type    core:Language , owl:NamedIndividual;
        rdfs:label  "Norwegian Nynorsk"@en .

<https://w3id.org/idsa/code/NO>
        rdf:type    core:Language , owl:NamedIndividual;
        rdfs:label  "Norwegian"@en .

<https://w3id.org/idsa/code/NOT>
        rdf:type      core:BinaryOperator , owl:NamedIndividual;
        rdfs:comment  "Logical difference operator (false != true)."@en;
        rdfs:label    "not equals"@en;
        skos:broader  odrl:neq .

<https://w3id.org/idsa/code/NOTIFICATION_LEVEL>
        rdf:type      odrl:LeftOperand , owl:NamedIndividual;
        rdfs:comment  "Similar to the idsc:LOG_LEVEL."@en;
        rdfs:label    "notification level" .

<https://w3id.org/idsa/code/NOTIFY>
        rdf:type         odrl:Action , owl:NamedIndividual;
        rdfs:comment     "To log information or notify an instance about incidents. Can be used to define Clearing House interactions."@en;
        rdfs:label       "notify"@en;
        skos:broader     odrl:inform;
        skos:note        "This action can target the consumer and the data provider of the resource."@en;
        odrl:includedIn  <https://w3id.org/idsa/code/LOG> .

<https://w3id.org/idsa/code/NOT_AUTHENTICATED>
        rdf:type      core:RejectionReason , owl:NamedIndividual;
        rdfs:comment  "Authenticity of a message sender has failed or is not verifiable.";
        rdfs:label    "NOT_AUTHENTICATED" .

<https://w3id.org/idsa/code/NOT_AUTHORIZED>
        rdf:type      core:RejectionReason , owl:NamedIndividual;
        rdfs:comment  "Sender is not authorized to initiate the command.";
        rdfs:label    "NOT_AUTHORIZED" .

<https://w3id.org/idsa/code/NOT_FOUND>
        rdf:type      core:RejectionReason , owl:NamedIndividual;
        rdfs:comment  "Requested Resource was not found.";
        rdfs:label    "NOT_FOUND" .

<https://w3id.org/idsa/code/NO_LOGGING>
        rdf:type      core:LogLevel , owl:NamedIndividual;
        rdfs:comment  "No logging."@en;
        rdfs:label    "No Logging"@en .

<https://w3id.org/idsa/code/NR>
        rdf:type    core:Language , owl:NamedIndividual;
        rdfs:label  "Southern Ndebele"@en .

<https://w3id.org/idsa/code/NV>
        rdf:type    core:Language , owl:NamedIndividual;
        rdfs:label  "Navajo, Navaho"@en .

<https://w3id.org/idsa/code/NY>
        rdf:type    core:Language , owl:NamedIndividual;
        rdfs:label  "Chichewa, Chewa, Nyanja"@en .

<https://w3id.org/idsa/code/OAUTH2_JWT>
        rdf:type      core:AuthStandard , owl:NamedIndividual;
        rdfs:comment  "OAUTH2 via JWT" .

<https://w3id.org/idsa/code/OC>
        rdf:type    core:Language , owl:NamedIndividual;
        rdfs:label  "Occitan"@en .

<https://w3id.org/idsa/code/OJ>
        rdf:type    core:Language , owl:NamedIndividual;
        rdfs:label  "Ojibwe, Ojibwa"@en .

<https://w3id.org/idsa/code/OM>
        rdf:type    core:Language , owl:NamedIndividual;
        rdfs:label  "Oromo"@en .

<https://w3id.org/idsa/code/ONCE>
        rdf:type      core:Frequency , skos:Concept , owl:NamedIndividual;
        rdfs:comment  "The event occurs only once."@en;
        rdfs:label    "Once"@en .

<https://w3id.org/idsa/code/OPERAND>
        rdf:type      odrl:LeftOperand , owl:NamedIndividual;
        rdfs:comment  "To indicate the second operand value for the Actions idsc:ADD, idsc:MULTIPLY and idsc:DIVIDE."@en;
        rdfs:label    "operand"@en .

<https://w3id.org/idsa/code/OR>
        rdf:type    core:Language , owl:NamedIndividual;
        rdfs:label  "Oriya"@en .

<https://w3id.org/idsa/code/OS>
        rdf:type    core:Language , owl:NamedIndividual;
        rdfs:label  "Ossetian, Ossetic"@en .

<https://w3id.org/idsa/code/OTHER>
        rdf:type    core:TokenFormat , owl:NamedIndividual;
        rdfs:label  "Other" .

<https://w3id.org/idsa/code/OUTPUT_ENDPOINT>
        rdf:type      core:AppEndpointType , owl:NamedIndividual;
        rdfs:comment  "Endpoint is used for data output."@en;
        rdfs:label    "Output endpoint"@en .

<https://w3id.org/idsa/code/OVERLAPPED_BY>
        rdf:type      core:BinaryOperator , owl:NamedIndividual;
        rdfs:comment  "If a interval T1 is overlapped another proper interval T2, then the beginning of T1 is before the beginning of T2, the end of T1 is after the beginning of T2, and the end of T1 is before the end of T2."@en;
        rdfs:label    "overlapped by"@en;
        rdfs:seeAlso  <http://www.w3.org/2006/time#intervalOverlappedBy>;
        skos:note     "Compares an instance of time:Interval to another instance of time:Interval. Evaluates to false if compared to a non time:Interval or one interval is empty."@en .

<https://w3id.org/idsa/code/OVERLAPS>
        rdf:type      core:BinaryOperator , owl:NamedIndividual;
        rdfs:comment  "If a time:Interval T1 overlapps another time:Interval T2, then the beginning of T1 is after the beginning of T2, the beginning of T1 is before the end of T2, and the end of T1 is after the end of T2."@en;
        rdfs:label    "overlaps"@en;
        rdfs:seeAlso  <http://www.w3.org/2006/time#intervalOverlaps>;
        skos:note     "Compares an instance of time:Interval to another instance of time:Interval. Evaluates to false if compared to a non time:Interval or one interval is empty."@en .

<https://w3id.org/idsa/code/PA>
        rdf:type    core:Language , owl:NamedIndividual;
        rdfs:label  "(Eastern) Punjabi"@en .

<https://w3id.org/idsa/code/PARIS>
        rdf:type    core:QueryTarget , owl:NamedIndividual;
        rdfs:label  "PARTICIPANT INFORMATION SERVICE" .

<https://w3id.org/idsa/code/PARTICIPANT_CENTRAL_LEVEL_CONTROL_FRAMEWORK>
        rdf:type    core:ParticipantCertificationLevel , owl:NamedIndividual;
        rdfs:label  "Central Level Control Framework Certification of Participants"@en;
        core:includedCertificationLevel
                <https://w3id.org/idsa/code/PARTICIPANT_CENTRAL_LEVEL_MANAGEMENT_SYSTEM> .

<https://w3id.org/idsa/code/PARTICIPANT_CENTRAL_LEVEL_MANAGEMENT_SYSTEM>
        rdf:type    core:ParticipantCertificationLevel , owl:NamedIndividual;
        rdfs:label  "Central Level Management System Certification of Participants"@en;
        core:includedCertificationLevel
                <https://w3id.org/idsa/code/PARTICIPANT_MEMBER_LEVEL_MANAGEMENT_SYSTEM> .

<https://w3id.org/idsa/code/PARTICIPANT_ENTRY_LEVEL_MANAGEMENT_SYSTEM>
        rdf:type    core:ParticipantCertificationLevel , owl:NamedIndividual;
        rdfs:label  "Entry Level Management System Certification of Participants"@en;
        core:includedCertificationLevel
                <https://w3id.org/idsa/code/PARTICIPANT_ENTRY_LEVEL_SELF_ASSESSMENT> .

<https://w3id.org/idsa/code/PARTICIPANT_ENTRY_LEVEL_SELF_ASSESSMENT>
        rdf:type    core:ParticipantCertificationLevel , owl:NamedIndividual;
        rdfs:label  "Entry Level Self-Assessment Certification of Participants"@en .

<https://w3id.org/idsa/code/PARTICIPANT_MEMBER_LEVEL_CONTROL_FRAMEWORK>
        rdf:type    core:ParticipantCertificationLevel , owl:NamedIndividual;
        rdfs:label  "Member Level ControlFramework Certification of Participants"@en;
        core:includedCertificationLevel
                <https://w3id.org/idsa/code/PARTICIPANT_MEMBER_LEVEL_CONTROL_FRAMEWORK> .

<https://w3id.org/idsa/code/PARTICIPANT_MEMBER_LEVEL_MANAGEMENT_SYSTEM>
        rdf:type    core:ParticipantCertificationLevel , owl:NamedIndividual;
        rdfs:label  "Member Level Management System Certification of Participants"@en;
        core:includedCertificationLevel
                <https://w3id.org/idsa/code/PARTICIPANT_MEMBER_LEVEL_MANAGEMENT_SYSTEM> .

<https://w3id.org/idsa/code/PATH>
        rdf:type      odrl:LeftOperand , owl:NamedIndividual;
        rdfs:comment  "Path to specific attribute (default JsonPath). Must be used together with idsc:STRING_EQ, idsc:STRING_CONTAINS, idsc:STRING_IS_CONTAINED, or idsc:MATCHES operators. RightOperand must be a xsd:string."@en;
        rdfs:label    "path to attribute" .

<https://w3id.org/idsa/code/PAYMENT>
        rdf:type      odrl:LeftOperand , owl:NamedIndividual;
        rdfs:comment  "Monetary payment, without any further sepcification on the type, amount or purpose."@en;
        rdfs:label    "payment"@en .

<https://w3id.org/idsa/code/PAY_AMOUNT>
        rdf:type      odrl:LeftOperand , owl:NamedIndividual;
        rdfs:comment  "Monetary amount to pay, usually used with idsc:EQ. Datatype is double. Currency required."@en;
        rdfs:label    "payAmount"@en;
        skos:broader  odrl:payAmount;
        core:broader  <https://w3id.org/idsa/code/PAYMENT> .

<https://w3id.org/idsa/code/PI>
        rdf:type    core:Language , owl:NamedIndividual;
        rdfs:label  "Pāli"@en .

<https://w3id.org/idsa/code/PL>
        rdf:type    core:Language , owl:NamedIndividual;
        rdfs:label  "Polish"@en .

<https://w3id.org/idsa/code/POLICY_EVALUATION_TIME>
        rdf:type      odrl:LeftOperand , owl:NamedIndividual;
        rdfs:comment  "The current system time (as UTC xsd:dateTimeStamp) for evaluating a time-related constraint. Allowed operators are idsc:AFTER, idsc:BEFORE, idsc:CONTAINS, idsc:TEMPORAL_DISJOINT, idsc:DURING, idsc:TEMPORAL_EQUALS, idsc:FINISHED_BY, idsc:FINISHES, idsc:MEETS, idsc:MET_BY, idsc:OVERLAPS, idsc:OVERLAPPED_BY, idsc:STARTS, idsc:STARTED_BY and idsc:DURATION_EQ with RightOperand time:TemporalEntity."@en;
        rdfs:label    "policy evaluation time"@en;
        skos:broader  odrl:dateTime .

<https://w3id.org/idsa/code/PREPATUAL_DATA_SALE>
        rdf:type      core:UsagePolicyClass , owl:NamedIndividual;
        rdfs:comment  "This policy restricts the transfer of a Data Asset against a one-off payment in a given currency."@en;
        rdfs:label    "Prepatual data sale"@en .

<https://w3id.org/idsa/code/PROCESS_ENDPOINT>
        rdf:type      core:AppEndpointType , owl:NamedIndividual;
        rdfs:comment  "Endpoint is used to start (or control) app processing."@en;
        rdfs:label    "Process endpoint"@en .

<https://w3id.org/idsa/code/PRODUCTIVE_DEPLOYMENT>
        rdf:type      core:ConnectorDeployMode , owl:NamedIndividual;
        rdfs:comment  "Indicates that a Connector is deployed for productive use."@en;
        rdfs:label    "Productive Deployment"@en .

<https://w3id.org/idsa/code/PS>
        rdf:type    core:Language , owl:NamedIndividual;
        rdfs:label  "Pashto, Pushto"@en .

<https://w3id.org/idsa/code/PSEUDONYMIZED>
        rdf:type      core:ArtifactState , owl:NamedIndividual;
        rdfs:comment  "The artifact is pseudo pseudonymized."@en;
        rdfs:label    "is pseudonymized"@en .

<https://w3id.org/idsa/code/PT>
        rdf:type    core:Language , owl:NamedIndividual;
        rdfs:label  "Portuguese"@en .

<https://w3id.org/idsa/code/PURPOSE>
        rdf:type      odrl:LeftOperand , owl:NamedIndividual;
        rdfs:comment  "A defined purpose for exercising the action of the Rule. Use with idsc:IN or idsc:SAME_AS and RDF Resources."@en;
        rdfs:label    "purpose"@en;
        skos:broader  odrl:purpose .

<https://w3id.org/idsa/code/PURPOSE_RESTRICTED_DATA_USAGE>
        rdf:type      core:UsagePolicyClass , owl:NamedIndividual;
        rdfs:comment  "This policy restricts the usage of data assets limited to specific purposes."@en;
        rdfs:label    "Purpose restricted data usage"@en .

<https://w3id.org/idsa/code/QU>
        rdf:type    core:Language , owl:NamedIndividual;
        rdfs:label  "Quechua"@en .

<https://w3id.org/idsa/code/QUANTITY>
        rdf:type      odrl:LeftOperand , owl:NamedIndividual;
        rdfs:comment  "Quantity limitation for exercising the action of the Rule. Operators can be idsc:LT, idsc:LTEQ, idsc:EQ, idsc:GT, idsc:GTEQ. Datatype is xsd:double.";
        rdfs:label    "quantity" .

<https://w3id.org/idsa/code/QUARTERLY>
        rdf:type          core:Frequency , skos:Concept , owl:NamedIndividual;
        rdfs:comment      "The event occurs every three months."@en;
        rdfs:isDefinedBy  <http://purl.org/cld/freq/>;
        rdfs:label        "Quarterly"@en;
        rdfs:seeAlso      <https://www.loc.gov/marc/holdings/hd853855.html>;
        dcam:memberOf     <http://purl.org/cld/terms/Frequency>;
        skos:inScheme     <http://purl.org/cld/terms/Frequency>;
        skos:prefLabel    "Quarterly"@en .

<https://w3id.org/idsa/code/QUERY>
        rdf:type      core:IdsProtocolSpecification , owl:NamedIndividual;
        rdfs:comment  "Queries conforming to IDS specifications."@en;
        rdfs:label    "Query";
        rdfs:seeAlso  <https://www.w3.org/TR/sparql11-overview/> .

<https://w3id.org/idsa/code/READ>
        rdf:type         odrl:Action , owl:NamedIndividual;
        rdfs:comment     "To obtain data from the resource."@en;
        rdfs:label       "read"@en;
        skos:broader     odrl:read;
        skos:note        "This action is always evaluated at the provider side. It corresponds to 'give access to a resource'."@en;
        odrl:includedIn  <https://w3id.org/idsa/code/MODIFY> .

<https://w3id.org/idsa/code/RECIPIENT>
        rdf:type      odrl:LeftOperand , owl:NamedIndividual;
        rdfs:comment  "For example, the recipient of the notify/inform action."@en;
        rdfs:label    "recipient"@en .

<https://w3id.org/idsa/code/RECURRENCE_RATE>
        rdf:type      odrl:LeftOperand , owl:NamedIndividual;
        rdfs:comment  "The limit how often exercising the action of the Rule may be possible. Operators can be idsc:LT, idsc:LTEQ, idsc:EQ, idsc:GT, idsc:GTEQ. Datatype is xsd:double.";
        rdfs:label    "recurrence rate" .

<https://w3id.org/idsa/code/REMOTE_NOTIFICATION>
        rdf:type      core:UsagePolicyClass , owl:NamedIndividual;
        rdfs:comment  "This policy restricts the usage of data assets with the obligation to notify a specific party about the data usage."@en;
        rdfs:label    "Remote notification"@en .

<https://w3id.org/idsa/code/REPLACE>
        rdf:type      odrl:Action , owl:NamedIndividual;
        rdfs:comment  "To replace some value."@en;
        rdfs:label    "replace"@en;
        skos:note     "This action modifies a value by replacing it with a given value. The field to be modified and the given value are specified in the policy as idsc:JSONPATH/idsc:XPATH and idsc:REPLACE_WITH, respectively."@en .

<https://w3id.org/idsa/code/REPLACE_WITH>
        rdf:type      odrl:LeftOperand , owl:NamedIndividual;
        rdfs:comment  "Specifies a new value for a specific field. The action must be idsc:REPLACE and the operator must be idsc:EQUALS."@en;
        rdfs:label    "repace with"@en .

<https://w3id.org/idsa/code/RESTRICTED_NUMBER_OF_USAGES>
        rdf:type      core:UsagePolicyClass , owl:NamedIndividual;
        rdfs:comment  "This policy restricts the usage of data assets limited to numeric count of executions of actions. \n\t\t\t\t\tA mechanism is needed that counts the usage of data in order to enforce the policy."@en;
        rdfs:label    "Restricted number of usages"@en .

<https://w3id.org/idsa/code/RM>
        rdf:type    core:Language , owl:NamedIndividual;
        rdfs:label  "Romansh"@en .

<https://w3id.org/idsa/code/RN>
        rdf:type    core:Language , owl:NamedIndividual;
        rdfs:label  "Kirundi"@en .

<https://w3id.org/idsa/code/RO>
        rdf:type    core:Language , owl:NamedIndividual;
        rdfs:label  "Romanian"@en .

<https://w3id.org/idsa/code/ROLE>
        rdf:type      odrl:LeftOperand , owl:NamedIndividual;
        rdfs:comment  "As end user role, not the IDS participant type."@en;
        rdfs:label    "role"@en .

<https://w3id.org/idsa/code/ROLE_RESTRICTED_DATA_USAGE>
        rdf:type      core:UsagePolicyClass , owl:NamedIndividual;
        rdfs:comment  "This policy restricts the usage of the data to a specific role. \n\t\t\t\t\tFor example, you can instantiate a policy of this class that allows only the members of the engineering department to use your data. \n\t\t\t\t\tThis policy class faces few limitations, i.e., in order to evaluate the conditions, it requires that the user roles are available and follow a common vocabulary"@en;
        rdfs:label    "Role restricted data usage"@en .

<https://w3id.org/idsa/code/RSA>
        rdf:type    core:KeyType , owl:NamedIndividual;
        rdfs:label  "RSA"@en .

<https://w3id.org/idsa/code/RU>
        rdf:type    core:Language , owl:NamedIndividual;
        rdfs:label  "Russian"@en .

<https://w3id.org/idsa/code/RW>
        rdf:type    core:Language , owl:NamedIndividual;
        rdfs:label  "Kinyarwanda"@en .

<https://w3id.org/idsa/code/RequestTemplate>
        rdf:type      core:PolicyTemplate , owl:NamedIndividual;
        rdfs:comment  "A generic template for policy requests with one permission and several constraints";
        rdfs:label    "Policy Request Template";
        skos:note     "{ \n\t\t\"@context\": \"https://w3id.org/idsa/contexts/context.jsonld\",\n\t\t\"@type\": \"ContractRequest\", \n\t\t\"uid\": \"<contract ID>\", \n\t\t\"refersTo\": \"idsc:RequestTemplate\" ,\n\t\t\"target\": \"[<Representation URI>|<Artifact URI>]\",\n\t\t\"ids:provider\": \"<Provider Participant URI>\",\n\t\t\"ids:consumer\": \"<Consumer Participant URI>\", \n\t\t\"odrl:permission\": {\n\t\t\t\"odrl:action\": \"[ids:use|ids:read|...]\" ,\n\t\t\t[\"odrl:constraint\" : {\n\t\t\t\t\t \"odrl:leftOperand\" : \"<Attribute URI>\",\n\t\t\t\t\t \"odrl:operator\" : \"[ids:eq|ids:lt|ids:gt]\",\n\t\t\t\t\t \"odrl:rightOperand\" : \"[<Value URI>|<Value Literal>]\"\n\t\t\t } [,]]*\n\t\t} }" , "@prefix ids: <https://w3id.org/idsa/core/> .\n\t\t@prefix idsc: <https://w3id.org/idsa/code/> .\n\t\t@prefix rdf: <http://www.w3.org/1999/02/22-rdf-syntax-ns#> .\n\t\t@prefix rdfs: <http://www.w3.org/2000/01/rdf-schema#> .\n\t\t@prefix xsd: <http://www.w3.org/2001/XMLSchema#> .\n\n\t\t[<contract URI>| [] ] a ids:ContractRequest ;\n\t\t\tids:uid <contract ID> ;\n\t\t\tids:refersTo idsc:RequestTemplate ;\n\t\t\tids:target [<Representation URI>|<Artifact URI>] ;\n\t\t\tids:consumer <Consumer Participant URI> ;\n\t\t\tids:provider <Provider Participant URI>\n\t\t\t[odrl:permission[\n\t\t\t\todrl:action ids:[use|read|...] ;\n\t\t\t\todrl:constraint [\n\t\t\t\t\todrl:leftOperand <Attribute URI> ;\n\t\t\t\t\todrl:operator [ids:eq|ids:lt|ids:gt] ;\n\t\t\t\t\todrl:rightOperand [<Value URI>|<Value Literal>]\n\t\t\t\t]\n\t\t\t] ;]*\n\t\t." , "The <Consumer Participant URI> asks <Provider Participant URI> to [ids:use|ids:read|...] \n\t\tits [<Representation URI>|<Artifact URI>].\n\t\tOptional: This only holds if <Attribute URI> is [equal|lower than|greater than] the [<Value URI>|<Value Literal>].\n\t\tOptional: This only holds if also <Attribute URI> is [equal|lower than|greater than] the [<Value URI>|<Value Literal>]."@en .

<https://w3id.org/idsa/code/SA>
        rdf:type    core:Language , owl:NamedIndividual;
        rdfs:label  "Sanskrit (Saṁskṛta)"@en .

<https://w3id.org/idsa/code/SAME_AS>
        rdf:type      core:BinaryOperator , owl:NamedIndividual;
        rdfs:comment  "Logical equals operator comparing two RDF URIs. Is true if at least one owl:sameAs relation exists."@en;
        rdfs:label    "is same as"@en;
        rdfs:seeAlso  owl:sameAs;
        skos:note     "A owl:sameAs A is always true."@en .

<https://w3id.org/idsa/code/SAML_1_1>
        rdf:type    core:TokenFormat , owl:NamedIndividual;
        rdfs:label  "Security Assertion Markup Language (SAML) 1.1" .

<https://w3id.org/idsa/code/SAML_2_0>
        rdf:type    core:TokenFormat , owl:NamedIndividual;
        rdfs:label  "Security Assertion Markup Language (SAML) 2.0" .

<https://w3id.org/idsa/code/SC>
        rdf:type    core:Language , owl:NamedIndividual;
        rdfs:label  "Sardinian"@en .

<https://w3id.org/idsa/code/SCHEMA_DEFINITION>
        rdf:type      terms:DCMIType , owl:NamedIndividual;
        rdfs:comment  "Formal, machine-interpretable definition of a data schema, e.g., XMLSchema, JSONSchema"@en;
        rdfs:label    "Schema definition" .

<https://w3id.org/idsa/code/SD>
        rdf:type    core:Language , owl:NamedIndividual;
        rdfs:label  "Sindhi"@en .

<https://w3id.org/idsa/code/SE>
        rdf:type    core:Language , owl:NamedIndividual;
        rdfs:label  "Northern Sami"@en .

<https://w3id.org/idsa/code/SECURITY_LEVEL>
        rdf:type      odrl:LeftOperand , owl:NamedIndividual;
        rdfs:comment  "The security level the consuming connector must have. Use together with idsc:SAME_AS or idsc:IN. The value decides which attribute dimension is regarded."@en;
        rdfs:label    "security level" .

<https://w3id.org/idsa/code/SECURITY_LEVEL_RESTRICTED_POLICY>
        rdf:type      core:UsagePolicyClass , owl:NamedIndividual;
        rdfs:comment  "This policy restricts the usage of data assets limited to a security level the consumer must conform to."@en;
        rdfs:label    "Security level restricted policy"@en .

<https://w3id.org/idsa/code/SELF_DESCRIPTION_ENDPOINT>
        rdf:type      core:AppEndpointType , owl:NamedIndividual;
        rdfs:comment  "Pre-defined endpoint used to return the corresponding self-description of the data app."@en;
        rdfs:label    "Self-description endpoint"@en .

<https://w3id.org/idsa/code/SEMIANNUAL>
        rdf:type          core:Frequency , skos:Concept , owl:NamedIndividual;
        rdfs:comment      "The event occurs twice a year."@en;
        rdfs:isDefinedBy  <http://purl.org/cld/freq/>;
        rdfs:label        "Semiannual"@en;
        rdfs:seeAlso      <https://www.loc.gov/marc/holdings/hd853855.html>;
        dcam:memberOf     <http://purl.org/cld/terms/Frequency>;
        skos:inScheme     <http://purl.org/cld/terms/Frequency>;
        skos:prefLabel    "Semiannual"@en .

<https://w3id.org/idsa/code/SEMIMONTHLY>
        rdf:type          core:Frequency , skos:Concept , owl:NamedIndividual;
        rdfs:comment      "The event occurs twice a month."@en;
        rdfs:isDefinedBy  <http://purl.org/cld/freq/>;
        rdfs:label        "Semimonthly"@en;
        rdfs:seeAlso      <https://www.loc.gov/marc/holdings/hd853855.html>;
        dcam:memberOf     <http://purl.org/cld/terms/Frequency>;
        skos:inScheme     <http://purl.org/cld/terms/Frequency>;
        skos:prefLabel    "Semimonthly"@en .

<https://w3id.org/idsa/code/SEMIWEEKLY>
        rdf:type          core:Frequency , skos:Concept , owl:NamedIndividual;
        rdfs:comment      "The event occurs twice a week."@en;
        rdfs:isDefinedBy  <http://purl.org/cld/freq/>;
        rdfs:label        "Semiweekly"@en;
        rdfs:seeAlso      <https://www.loc.gov/marc/holdings/hd853855.html>;
        dcam:memberOf     <http://purl.org/cld/terms/Frequency>;
        skos:inScheme     <http://purl.org/cld/terms/Frequency>;
        skos:prefLabel    "Semiweekly"@en .

<https://w3id.org/idsa/code/SERVICE_ISOLATION_LEAST_PRIVILEGE>
        rdf:type    core:ServiceIsolationGuarantee , owl:NamedIndividual;
        rdfs:label  "Service Isolation Least Privilege" .

<https://w3id.org/idsa/code/SERVICE_ISOLATION_NONE>
        rdf:type    core:ServiceIsolationGuarantee , owl:NamedIndividual;
        rdfs:label  "Service Isolation None" .

<https://w3id.org/idsa/code/SERVICE_ISOLATION_PROCESS_GROUP>
        rdf:type    core:ServiceIsolationGuarantee , owl:NamedIndividual;
        rdfs:label  "Service Isolation Process Group" .

<https://w3id.org/idsa/code/SG>
        rdf:type    core:Language , owl:NamedIndividual;
        rdfs:label  "Sango"@en .

<https://w3id.org/idsa/code/SHORTER>
        rdf:type      core:BinaryOperator , owl:NamedIndividual;
        rdfs:comment  "If a temporal entity T1 is shorter than another temporal entity T2, then the length or duration of T1 is shorter. Instants and xsd:dateTimeStamp Literals have always the duration 'P0Y0M0DT0H0M0S'^^xsd:duration and therefore have always the same duration."@en;
        rdfs:label    "shorter"@en;
        skos:note     "Compares an instance of time:TemporalEntity with an instance of xsd:duration."@en .

<https://w3id.org/idsa/code/SHORTER_EQ>
        rdf:type      core:BinaryOperator , owl:NamedIndividual;
        rdfs:comment  "If a temporal entity T1 is shorter or equals than another temporal entity T2, then the length or duration of T1 is shorter or their length or their duration is equal. Instants and xsd:dateTimeStamp Literals have always the duration 'P0Y0M0DT0H0M0S'^^xsd:duration and therefore have always the same duration."@en;
        rdfs:label    "shorter or equals"@en;
        skos:note     "Compares an instance of time:TemporalEntity with an instance of xsd:duration."@en .

<https://w3id.org/idsa/code/SHUFFLE>
        rdf:type      odrl:Action , owl:NamedIndividual;
        rdfs:comment  "This action modifies a value by replacing it with an anagram of the value."@en;
        rdfs:label    "shuffle"@en;
        skos:note     "This action modifies a value by replacing it with an anagram of the value. The field to be modified is specified in the policy as idsc:JSONPATH/idsc:XPATH."@en .

<https://w3id.org/idsa/code/SI>
        rdf:type    core:Language , owl:NamedIndividual;
        rdfs:label  "Sinhalese, Sinhala"@en .

<https://w3id.org/idsa/code/SK>
        rdf:type    core:Language , owl:NamedIndividual;
        rdfs:label  "Slovak"@en .

<https://w3id.org/idsa/code/SL>
        rdf:type    core:Language , owl:NamedIndividual;
        rdfs:label  "Slovene"@en .

<https://w3id.org/idsa/code/SM>
        rdf:type    core:Language , owl:NamedIndividual;
        rdfs:label  "Samoan"@en .

<https://w3id.org/idsa/code/SN>
        rdf:type    core:Language , owl:NamedIndividual;
        rdfs:label  "Shona"@en .

<https://w3id.org/idsa/code/SO>
        rdf:type    core:Language , owl:NamedIndividual;
        rdfs:label  "Somali"@en .

<https://w3id.org/idsa/code/SPARQL>
        rdf:type    core:QueryLanguage , owl:NamedIndividual;
        rdfs:label  "SPARQL" .

<https://w3id.org/idsa/code/SPATIAL_CONTAINS>
        rdf:type      core:BinaryOperator , owl:NamedIndividual;
        rdfs:comment  "Spatial operator 'contains' as defined by the Egenhofer Topological Relations family: An object A contains another object B if A and B share interior but no bounding faces; if B has bounding faces which are interior faces of , and none of A's bounding faces coincides with any of B's interior faces. (https://doi.org/10.1007/3-540-51295-0_148 Definition 5)"@en;
        rdfs:label    "contains"@en;
        rdfs:seeAlso  <http://www.opengis.net/ont/geosparql#ehContains>;
        skos:note     "In addition, a polygom contains a point iff the point is in the polygom's interior (the point itself has no interior)."@en .

<https://w3id.org/idsa/code/SPATIAL_EQUALS>
        rdf:type      core:BinaryOperator , owl:NamedIndividual;
        rdfs:comment  "Spatial operator 'equals' as defined by the Egenhofer Topological Relations family: Two objects are equal if both intersections of bounding and interior faces are not empty while the two boundary-interior intersections are empty. (https://doi.org/10.1007/3-540-51295-0_148 Definition 3)"@en;
        rdfs:label    "equals"@en;
        rdfs:seeAlso  <http://www.opengis.net/ont/geosparql#ehEquals>;
        skos:note     "In addition, two spatial points are equal iff both coordinates are equal (points have no interior)."@en .

<https://w3id.org/idsa/code/SPATIAL_MEET>
        rdf:type      core:BinaryOperator , owl:NamedIndividual;
        rdfs:comment  "Spatial operator 'meet' as defined by the Egenhofer Topological Relations family: If the intersection among the bounding faces is not empty, whereas all other 3 intersections are empty, then the two objects meet. (https://doi.org/10.1007/3-540-51295-0_148 Definition 2)"@en;
        rdfs:label    "meet"@en;
        rdfs:seeAlso  <http://www.opengis.net/ont/geosparql#ehMeet> .

<https://w3id.org/idsa/code/SPATIAL_OVERLAP>
        rdf:type      core:BinaryOperator , owl:NamedIndividual;
        rdfs:comment  "Spatial operator 'overlap' as defined by the Egenhofer Topological Relations family: Two objects overlap if they have common interior faces and the bounding faces have common parts with the opposite interior faces. (https://doi.org/10.1007/3-540-51295-0_148 Definition 8)"@en;
        rdfs:label    "overlap"@en;
        rdfs:seeAlso  <http://www.opengis.net/ont/geosparql#ehOverlap> .

<https://w3id.org/idsa/code/SQ>
        rdf:type    core:Language , owl:NamedIndividual;
        rdfs:label  "Albanian"@en .

<https://w3id.org/idsa/code/SQL>
        rdf:type    core:QueryLanguage , owl:NamedIndividual;
        rdfs:label  "SQL" .

<https://w3id.org/idsa/code/SR>
        rdf:type    core:Language , owl:NamedIndividual;
        rdfs:label  "Serbian"@en .

<https://w3id.org/idsa/code/SS>
        rdf:type    core:Language , owl:NamedIndividual;
        rdfs:label  "Swati"@en .

<https://w3id.org/idsa/code/ST>
        rdf:type    core:Language , owl:NamedIndividual;
        rdfs:label  "Southern Sotho"@en .

<https://w3id.org/idsa/code/STARTED_BY>
        rdf:type      core:BinaryOperator , owl:NamedIndividual;
        rdfs:comment  "If a TemporalEntity T1 is started by another proper interval T2, then the beginning of T1 is coincident with the beginning of T2, and the end of T1 is after the end of T2."@en;
        rdfs:label    "started by"@en;
        rdfs:seeAlso  <http://www.w3.org/2006/time#intervalStartedBy>;
        skos:note     "Compares an instance of TemporalEntity (or xsd:dateTimeStamp Literal) to instance of time:Interval. Evaluates to false if T1 is an Instant (or xsd:dateTimeStamp Literal) as the end of T1 can then not be idsc:AFTER the end of T2."@en .

<https://w3id.org/idsa/code/STARTS>
        rdf:type      core:BinaryOperator , owl:NamedIndividual;
        rdfs:comment  "If an interval T1 starts with a TemporalEntity T2, then the beginning of T1 is coincident with the beginning of T2, and the end of T1 is before the end of T2."@en;
        rdfs:label    "starts"@en;
        rdfs:seeAlso  <http://www.w3.org/2006/time#intervalStarts>;
        skos:note     "Compares an instance of time:Interval to another instance of TemporalEntity (or xsd:dateTimeStamp Literal). Evaluates to false if T2 is not a time:Interval as then the end of T1 can never be idsc:BEFORE the end of T2"@en .

<https://w3id.org/idsa/code/STATE>
        rdf:type      odrl:LeftOperand , owl:NamedIndividual;
        rdfs:comment  "Specifies whether an (external) resource is true/false, active/inactive, has happened/not happened, etc. Operator must be idsc:EQUALS with RightOperands of datatype xsd:anyURI. The referenced URI should point to a (remote) resource which returns a xsd:boolean value."@en;
        rdfs:label    "state"@en .

<https://w3id.org/idsa/code/STATE_RESTRICTED_POLICY>
        rdf:type      core:UsagePolicyClass , owl:NamedIndividual;
        rdfs:comment  "This policy restricts the usage of data assets limited to specific states. Possible states include, for example, that the contract for the given data asset has not yet expired."@en;
        rdfs:label    "State restricted policy"@en .

<https://w3id.org/idsa/code/STATUS_ENDPOINT>
        rdf:type      core:AppEndpointType , owl:NamedIndividual;
        rdfs:comment  "Endpoint is used to get app health / lifecycle status."@en;
        rdfs:label    "Status endpoint"@en .

<https://w3id.org/idsa/code/STRING_CONTAINS>
        rdf:type      core:BinaryOperator , owl:NamedIndividual;
        rdfs:comment  "Contains operator for strings. Evaluates to true iff the LeftOperand contains the complete RightOperand."@en;
        rdfs:label    "string contains"@en .

<https://w3id.org/idsa/code/STRING_EQ>
        rdf:type      core:BinaryOperator , owl:NamedIndividual;
        rdfs:comment  "Equals operator for strings. Evaluates to true iff all characters and their sequence is the same."@en;
        rdfs:label    "string equals"@en .

<https://w3id.org/idsa/code/STRING_IS_CONTAINED>
        rdf:type      core:BinaryOperator , owl:NamedIndividual;
        rdfs:comment  "Contained in operator for strings. Evaluates to true iff the LeftOperand is contained completely by the RightOperand."@en;
        rdfs:label    "string is contained in"@en .

<https://w3id.org/idsa/code/SU>
        rdf:type    core:Language , owl:NamedIndividual;
        rdfs:label  "Sundanese"@en .

<https://w3id.org/idsa/code/SV>
        rdf:type    core:Language , owl:NamedIndividual;
        rdfs:label  "Swedish"@en .

<https://w3id.org/idsa/code/SW>
        rdf:type    core:Language , owl:NamedIndividual;
        rdfs:label  "Swahili"@en .

<https://w3id.org/idsa/code/SWT>
        rdf:type    core:TokenFormat , owl:NamedIndividual;
        rdfs:label  "Simple Web Token" .

<https://w3id.org/idsa/code/SYSTEM>
        rdf:type      odrl:LeftOperand , owl:NamedIndividual;
        rdfs:comment  "Execution system or execution environment that is used to access the asset under consideration, usually an IDS Connector. The regarded data object should correspond to the IDS Connector class and its attributes. Must be used together with idsc:SAME_AS, idsc:NOT, idsc:HAS_STATE, idsc:IN, idsc:COVERED_BY idsc:INSIDE, idsc:SPATIAL_EQUALS, idsc:DISJOINT, or idsc:INSIDE_NETWORK operators. RightOperandReference must be a URI identifying the target system(s)."@en;
        rdfs:label    "execution system" .

<https://w3id.org/idsa/code/SYSTEM_DEVICE>
        rdf:type      odrl:LeftOperand , owl:NamedIndividual;
        rdfs:comment  "The ODRL definitions is “An identified computing system or computing device used for exercising the action of the Rule.” "@en;
        rdfs:label    "system device" .

<https://w3id.org/idsa/code/TA>
        rdf:type    core:Language , owl:NamedIndividual;
        rdfs:label  "Tamil"@en .

<https://w3id.org/idsa/code/TARGET_POLICY>
        rdf:type      odrl:LeftOperand , owl:NamedIndividual;
        rdfs:comment  "In order to attach/address a policy to a contract. "@en;
        rdfs:label    "target policy"@en .

<https://w3id.org/idsa/code/TE>
        rdf:type    core:Language , owl:NamedIndividual;
        rdfs:label  "Telugu"@en .

<https://w3id.org/idsa/code/TEMPORAL_DISJOINT>
        rdf:type      core:BinaryOperator , owl:NamedIndividual;
        rdfs:comment  "If a TemporalEntity (or xsd:dateTimeStamp) T1 is disjoint with another time:TemporalEntity (or xsd:dateTimeStamp) T2, then T1 is idsc:BEFORE or idsc:AFTER to T2."@en;
        rdfs:label    "disjoint"@en;
        rdfs:seeAlso  <http://www.w3.org/2006/time#intervalDisjoint>;
        skos:note     "Compares an instance of time:TemporalEntity or xsd:dateTimeStamp Literal to an instance of time:TemporalEntity or xsd:dateTimeStamp Literal."@en .

<https://w3id.org/idsa/code/TEMPORAL_EQUALS>
        rdf:type      core:BinaryOperator , owl:NamedIndividual;
        rdfs:comment  "If a TemporalEntity (or xsd:dateTimeStamp Literal) T1 is equals another TemporalEntity (or xsd:dateTimeStamp Literal) T2, then the beginning of T1 is coincident with the beginning of T2, and the end of T1 is coincident with the end of T2. The beginning and ending is the same for instances of time:Instant (or xsd:dateTimeStamp Literal)."@en;
        rdfs:label    "interval equals"@en;
        rdfs:seeAlso  <http://www.w3.org/2006/time#intervalEquals>;
        skos:note     "Compares an instance of TemporalEntity or xsd:dateTimeStamp Literal to another TemporalEntity or xsd:dateTimeStamp. Evaluates to false if a DurationEntity is involved."@en .

<https://w3id.org/idsa/code/TEMPORARILY_NOT_AVAILABLE>
        rdf:type      core:RejectionReason , owl:NamedIndividual;
        rdfs:comment  "The requested resource, representation or artifact is temporarily not available but might be back later.";
        rdfs:label    "TEMPORARILY_NOT_AVAILABLE" .

<https://w3id.org/idsa/code/TEST_DEPLOYMENT>
        rdf:type      core:ConnectorDeployMode , owl:NamedIndividual;
        rdfs:comment  "Indicates that a Connector is deployed for testing."@en;
        rdfs:label    "Test Deployment"@en .

<https://w3id.org/idsa/code/TG>
        rdf:type    core:Language , owl:NamedIndividual;
        rdfs:label  "Tajik"@en .

<https://w3id.org/idsa/code/TH>
        rdf:type    core:Language , owl:NamedIndividual;
        rdfs:label  "Thai"@en .

<https://w3id.org/idsa/code/THREE_TIMES_A_MONTH>
        rdf:type          core:Frequency , skos:Concept , owl:NamedIndividual;
        rdfs:comment      "The event occurs three times a month."@en;
        rdfs:isDefinedBy  <http://purl.org/cld/freq/>;
        rdfs:label        "Three times a month"@en;
        rdfs:seeAlso      <https://www.loc.gov/marc/holdings/hd853855.html>;
        dcam:memberOf     <http://purl.org/cld/terms/Frequency>;
        skos:inScheme     <http://purl.org/cld/terms/Frequency>;
        skos:prefLabel    "Three times a month"@en .

<https://w3id.org/idsa/code/THREE_TIMES_A_WEEK>
        rdf:type          core:Frequency , skos:Concept , owl:NamedIndividual;
        rdfs:comment      "The event occurs three times a week."@en;
        rdfs:isDefinedBy  <http://purl.org/cld/freq/>;
        rdfs:label        "Three times a week"@en;
        rdfs:seeAlso      <https://www.loc.gov/marc/holdings/hd853855.html>;
        dcam:memberOf     <http://purl.org/cld/terms/Frequency>;
        skos:inScheme     <http://purl.org/cld/terms/Frequency>;
        skos:prefLabel    "Three times a week"@en .

<https://w3id.org/idsa/code/THREE_TIMES_A_YEAR>
        rdf:type          core:Frequency , skos:Concept , owl:NamedIndividual;
        rdfs:comment      "The event occurs three times a year."@en;
        rdfs:isDefinedBy  <http://purl.org/cld/freq/>;
        rdfs:label        "Three times a year"@en;
        rdfs:seeAlso      <https://www.loc.gov/marc/holdings/hd853855.html>;
        dcam:memberOf     <http://purl.org/cld/terms/Frequency>;
        skos:inScheme     <http://purl.org/cld/terms/Frequency>;
        skos:prefLabel    "Three times a year"@en .

<https://w3id.org/idsa/code/TI>
        rdf:type    core:Language , owl:NamedIndividual;
        rdfs:label  "Tigrinya"@en .

<https://w3id.org/idsa/code/TK>
        rdf:type    core:Language , owl:NamedIndividual;
        rdfs:label  "Turkmen"@en .

<https://w3id.org/idsa/code/TL>
        rdf:type    core:Language , owl:NamedIndividual;
        rdfs:label  "Tagalog"@en .

<https://w3id.org/idsa/code/TN>
        rdf:type    core:Language , owl:NamedIndividual;
        rdfs:label  "Tswana"@en .

<https://w3id.org/idsa/code/TO>
        rdf:type    core:Language , owl:NamedIndividual;
        rdfs:label  "Tonga (Tonga Islands)"@en .

<https://w3id.org/idsa/code/TOO_MANY_RESULTS>
        rdf:type      core:RejectionReason , owl:NamedIndividual;
        rdfs:comment  "Processing of the command would lead to too many results (computational or bandwidth limitations)";
        rdfs:label    "TOO_MANY_RESULTS" .

<https://w3id.org/idsa/code/TR>
        rdf:type    core:Language , owl:NamedIndividual;
        rdfs:label  "Turkish"@en .

<https://w3id.org/idsa/code/TRACK_PROVENANCE>
        rdf:type         odrl:Action , owl:NamedIndividual;
        rdfs:comment     "To accept that the use of the Asset may be tracked."@en;
        rdfs:label       "track provenance"@en;
        skos:note        "This action is always evaluated at the consumer side."@en;
        odrl:includedIn  <https://w3id.org/idsa/code/NOTIFY> .

<https://w3id.org/idsa/code/TRIENNIAL>
        rdf:type          core:Frequency , owl:NamedIndividual;
        rdfs:comment      "The event occurs every three years."@en;
        rdfs:isDefinedBy  <http://purl.org/cld/freq/>;
        rdfs:label        "Triennial"@en;
        rdfs:seeAlso      <https://www.loc.gov/marc/holdings/hd853855.html>;
        dcam:memberOf     <http://purl.org/cld/terms/Frequency>;
        skos:inScheme     <http://purl.org/cld/terms/Frequency>;
        skos:prefLabel    "Triennial"@en .

<https://w3id.org/idsa/code/TRUST_PLUS_SECURITY_PROFILE>
        rdf:type                core:SecurityProfile , owl:NamedIndividual;
        rdfs:comment            "The Security Profile TRUST+ as defined by the IDS certification criteria."@en;
        rdfs:label              "Trust Plus security profile"@en;
        core:securityGuarantee  <https://w3id.org/idsa/code/USAGE_CONTROL_REMOTE_COMPLIANCE_VERIFICATION> , <https://w3id.org/idsa/code/SERVICE_ISOLATION_LEAST_PRIVILEGE> , <https://w3id.org/idsa/code/LOCAL_DATA_CONFIDENTIALITY_FULL_ENCRYPTION> , <https://w3id.org/idsa/code/INTEGRITY_VERIFICATION_SCOPE_KERNEL_CORE_CONTAINER_APPLICATION> , <https://w3id.org/idsa/code/INTEGRITY_VERIFICATION_REMOTE> , <https://w3id.org/idsa/code/AUTHENTICATION_MUTUAL> , <https://w3id.org/idsa/code/AUDIT_REMOTE_TRACING> , <https://w3id.org/idsa/code/APP_RESOURCES_REMOTE_VERIFICATION> .

<https://w3id.org/idsa/code/TRUST_SECURITY_PROFILE>
        rdf:type                core:SecurityProfile , owl:NamedIndividual;
        rdfs:comment            "The Security Profile TRUST as defined by the IDS certification criteria."@en;
        rdfs:label              "Trust security profile"@en;
        core:securityGuarantee  <https://w3id.org/idsa/code/USAGE_CONTROL_POLICY_ENFORCEMENT> , <https://w3id.org/idsa/code/SERVICE_ISOLATION_LEAST_PRIVILEGE> , <https://w3id.org/idsa/code/LOCAL_DATA_CONFIDENTIALITY_FULL_ENCRYPTION> , <https://w3id.org/idsa/code/INTEGRITY_VERIFICATION_SCOPE_KERNEL_CORE_CONTAINER> , <https://w3id.org/idsa/code/INTEGRITY_VERIFICATION_REMOTE> , <https://w3id.org/idsa/code/AUTHENTICATION_MUTUAL> , <https://w3id.org/idsa/code/AUDIT_LOCAL_LOGGING> , <https://w3id.org/idsa/code/APP_RESOURCES_LOCAL_ENFORCEMENT> .

<https://w3id.org/idsa/code/TS>
        rdf:type    core:Language , owl:NamedIndividual;
        rdfs:label  "Tsonga"@en .

<https://w3id.org/idsa/code/TT>
        rdf:type    core:Language , owl:NamedIndividual;
        rdfs:label  "Tatar"@en .

<https://w3id.org/idsa/code/TW>
        rdf:type    core:Language , owl:NamedIndividual;
        rdfs:label  "Twi"@en .

<https://w3id.org/idsa/code/TWO_TIMES_A_DAY>
        rdf:type      core:Frequency , skos:Concept , owl:NamedIndividual;
        rdfs:comment  "The event occurs twice a day."@en;
        rdfs:label    "Two times a day"@en .

<https://w3id.org/idsa/code/TY>
        rdf:type    core:Language , owl:NamedIndividual;
        rdfs:label  "Tahitian"@en .

<https://w3id.org/idsa/code/UG>
        rdf:type    core:Language , owl:NamedIndividual;
        rdfs:label  "Uyghur"@en .

<https://w3id.org/idsa/code/UK>
        rdf:type    core:Language , owl:NamedIndividual;
        rdfs:label  "Ukrainian"@en .

<https://w3id.org/idsa/code/UNKNOWN>
        rdf:type    core:TokenFormat , owl:NamedIndividual;
        rdfs:label  "Unknown" .

<https://w3id.org/idsa/code/UR>
        rdf:type    core:Language , owl:NamedIndividual;
        rdfs:label  "Urdu"@en .

<https://w3id.org/idsa/code/USAGE_CONTROL_NONE>
        rdf:type    core:UsageControlGuarantee , owl:NamedIndividual;
        rdfs:label  "Usage Control None" .

<https://w3id.org/idsa/code/USAGE_CONTROL_POLICY_ENFORCEMENT>
        rdf:type    core:UsageControlGuarantee , owl:NamedIndividual;
        rdfs:label  "Usage Control Policy Enforcement" .

<https://w3id.org/idsa/code/USAGE_CONTROL_REMOTE_COMPLIANCE_VERIFICATION>
        rdf:type    core:UsageControlGuarantee , owl:NamedIndividual;
        rdfs:label  "Usage Control Remote Compliance Verification" .

<https://w3id.org/idsa/code/USAGE_POLICY_ENDPOINT>
        rdf:type      core:AppEndpointType , owl:NamedIndividual;
        rdfs:comment  "Endpoint is used for usage policy / usage control related scenarios."@en;
        rdfs:label    "Usage policy endpoint"@en .

<https://w3id.org/idsa/code/USE>
        rdf:type      odrl:Action , owl:NamedIndividual;
        rdfs:comment  "To use a resource in any possible way. Includes all other actions."@en;
        rdfs:label    "use"@en;
        skos:broader  odrl:use;
        skos:note     "This action is always evaluated at the consumer side."@en .

<https://w3id.org/idsa/code/USER>
        rdf:type      odrl:LeftOperand , owl:NamedIndividual;
        rdfs:comment  "The user of a system at the *consuming connector* requesting access to a resource. Recommended usage for checking whether the user's role is sufficient for his/her desired action. Allowed operators are idsc:MEMBER_OF, idsc:HAS_MEMBERSHIP, idsc:HAS_SITE with a RightOperand referencing a (set of) acceptable organisations (ids:Participant),memberships, sites. Preferred behaviour is that the RightOperand dereferences to an endpoint hosting the required role information."@en;
        rdfs:label    "user"@en .

<https://w3id.org/idsa/code/USE_DATA_AND_DELETE_AFTER>
        rdf:type      core:UsagePolicyClass , owl:NamedIndividual;
        rdfs:comment  "This policy restricts the usage of data assets with the obligation to delete the asset after usage."@en;
        rdfs:label    "Use data and delete after"@en .

<https://w3id.org/idsa/code/UZ>
        rdf:type    core:Language , owl:NamedIndividual;
        rdfs:label  "Uzbek"@en .

<https://w3id.org/idsa/code/VE>
        rdf:type    core:Language , owl:NamedIndividual;
        rdfs:label  "Venda"@en .

<https://w3id.org/idsa/code/VERSION_NOT_SUPPORTED>
        rdf:type      core:RejectionReason , owl:NamedIndividual;
        rdfs:comment  "The version of the information model against which the referenced message should be interpreted, is not supported by the recipient.";
        rdfs:label    "VERSION_NOT_SUPPORTED" .

<https://w3id.org/idsa/code/VI>
        rdf:type    core:Language , owl:NamedIndividual;
        rdfs:label  "Vietnamese"@en .

<https://w3id.org/idsa/code/VO>
        rdf:type    core:Language , owl:NamedIndividual;
        rdfs:label  "Volapük"@en .

<https://w3id.org/idsa/code/WA>
        rdf:type    core:Language , owl:NamedIndividual;
        rdfs:label  "Walloon"@en .

<https://w3id.org/idsa/code/WEEKLY>
        rdf:type          core:Frequency , skos:Concept , owl:NamedIndividual;
        rdfs:comment      "The event occurs once a week."@en;
        rdfs:isDefinedBy  <http://purl.org/cld/freq/>;
        rdfs:label        "Weekly"@en;
        rdfs:seeAlso      <https://www.loc.gov/marc/holdings/hd853855.html>;
        dcam:memberOf     <http://purl.org/cld/terms/Frequency>;
        skos:inScheme     <http://purl.org/cld/terms/Frequency>;
        skos:prefLabel    "Weekly"@en .

<https://w3id.org/idsa/code/WO>
        rdf:type    core:Language , owl:NamedIndividual;
        rdfs:label  "Wolof"@en .

<https://w3id.org/idsa/code/WRITE>
        rdf:type         odrl:Action , owl:NamedIndividual;
        rdfs:comment     "To change a remote resource."@en;
        rdfs:label       "write"@en;
        skos:note        "This action is always evaluated at the provider side. It corresponds to 'allow changes of a resource' but *not* including its deletion."@en;
        odrl:includedIn  <https://w3id.org/idsa/code/USE> .

<https://w3id.org/idsa/code/XH>
        rdf:type    core:Language , owl:NamedIndividual;
        rdfs:label  "Xhosa"@en .

<https://w3id.org/idsa/code/XPATH>
        rdf:type      odrl:LeftOperand , owl:NamedIndividual;
        rdfs:comment  "An expression that refers to specific elements of an XML document."@en;
        rdfs:label    "xpath"@en .

<https://w3id.org/idsa/code/XQUERY>
        rdf:type    core:QueryLanguage , owl:NamedIndividual;
        rdfs:label  "XQUERY" .

<https://w3id.org/idsa/code/YI>
        rdf:type    core:Language , owl:NamedIndividual;
        rdfs:label  "Yiddish"@en .

<https://w3id.org/idsa/code/YO>
        rdf:type    core:Language , owl:NamedIndividual;
        rdfs:label  "Yoruba"@en .

<https://w3id.org/idsa/code/ZA>
        rdf:type    core:Language , owl:NamedIndividual;
        rdfs:label  "Zhuang, Chuang"@en .

<https://w3id.org/idsa/code/ZH>
        rdf:type    core:Language , owl:NamedIndividual;
        rdfs:label  "Chinese"@en .

<https://w3id.org/idsa/code/ZU>
        rdf:type    core:Language , owl:NamedIndividual;
        rdfs:label  "Zulu"@en .

<https://w3id.org/idsa/core>
        rdf:type                       owl:Ontology;
        rdfs:comment                   "This ontology defines classes and properties for describing participants, infrastructure, data and services of the International Data Spaces (formerly known as Industrial Data Space).";
        rdfs:isDefinedBy               core:;
        rdfs:label                     "IDS Information Model"@en;
        rdfs:seeAlso                   <https://international-data-spaces-association.github.io/InformationModel/>;
        ns:license                     <http://www.apache.org/licenses/LICENSE-2.0>;
        terms:contributor              <https://github.com/HaydarAk> , <https://github.com/JohannesLipp> , <https://github.com/Maboeckmann> , <https://github.com/clange> , <https://github.com/jlangkau> , <https://github.com/lcomet> , <https://github.com/mkollenstart> , <https://github.com/sebbader>;
        terms:contributor              [] ;
        terms:contributor              [ rdf:type   foaf:Person , terms:Agent;
                                         foaf:name  "Andreas Müller"
                                       ];
        terms:contributor              [ rdf:type   foaf:Person , terms:Agent;
                                         foaf:name  "Anna Kasprzik"
                                       ];
        terms:created                  "2017-09-26"^^xsd:date;
        terms:creator                  <https://github.com/jpullmann> , <http://sebastian.tramp.name> , <https://github.com/cmader>;
        terms:modified                 "2022-06-01"^^xsd:date;
        terms:title                    "The International Data Spaces Information Model"@en;
        vann:preferredNamespacePrefix  "ids";
        vann:preferredNamespaceUri     "https://w3id.org/idsa/core/";
        void:vocabulary                foaf: , void: , <http://purl.org/vocommons/voaf#> , vann: , terms:;
        owl:versionInfo                "4.2.0" .
core:   rdf:type         <http://purl.org/vocommons/voaf#Vocabulary> , owl:NamedIndividual;
        terms:publisher  core:IDSA .

core:AccessTokenRequestMessage
        rdf:type         owl:Class;
        rdfs:comment     "Message requesting an access token. This is intended for point-to-point communication with, e.g., Brokers."@en;
        rdfs:label       "AccessToken Request Message"@en;
        rdfs:subClassOf  core:RequestMessage .

core:AccessTokenResponseMessage
        rdf:type         owl:Class;
        rdfs:comment     "Response to an access token request, intended for point-to-point communication."@en;
        rdfs:label       "Access Token Response"@en;
        rdfs:subClassOf  core:ResponseMessage .

core:AppAvailableMessage
        rdf:type         owl:Class;
        rdfs:comment     "Message indicating that a specific App should be available (again) in the AppStore."@en;
        rdfs:label       "App Available Message"@en;
        rdfs:subClassOf  core:AppNotificationMessage .

core:AppDeleteMessage
        rdf:type         owl:Class;
        rdfs:comment     "Message indicating that an App should be deleted from the AppStore."@en;
        rdfs:label       "App Delete Message"@en;
        rdfs:subClassOf  core:AppNotificationMessage .

core:AppEndpoint  rdf:type  owl:Class;
        rdfs:comment     "Description of endpoints a DataApp offers."@en;
        rdfs:label       "DataApp Endpoint"@en;
        rdfs:subClassOf  core:Endpoint .

core:AppEndpointType  rdf:type  owl:Class;
        rdfs:comment  "Class of endpoint types a data app offers."@en;
        rdfs:label    "App endpoint type"@en .

core:AppExecutionResources
        rdf:type             owl:Class;
        rdfs:comment         "Resource control for deployed services."@en;
        rdfs:label           "App execution resources"@en;
        rdfs:subClassOf      core:SecurityGuarantee;
        owl:equivalentClass  [ rdf:type   owl:Class;
                               owl:oneOf  ( <https://w3id.org/idsa/code/APP_RESOURCES_LOCAL_ENFORCEMENT> <https://w3id.org/idsa/code/APP_RESOURCES_NONE> <https://w3id.org/idsa/code/APP_RESOURCES_REMOTE_VERIFICATION> )
                             ] .

core:AppNotificationMessage
        rdf:type         owl:Class;
        rdfs:comment     "Superclass of all messages, indicating a change of a DataApp. Unlike Resource-related Messages, AppNotificationMessages should lead to a state change for an app at the recipient, the AppStore."@en;
        rdfs:label       "App Notification Message"@en;
        rdfs:subClassOf  core:ResourceNotificationMessage .

core:AppRegistrationRequestMessage
        rdf:type         owl:Class;
        rdfs:comment     "Message that asks for registration or update of a data app to the App Store. Payload contains app-related metadata (instance of class ids:AppResource). Message header may contain an app identifier parameter of a prior registered data app. If the app identifier is supplied, the message should be interpreted as a registration for an app update. Otherwise this message is used to register a new app. "@en;
        rdfs:label       "App Registration Request Message"@en;
        rdfs:subClassOf  core:RequestMessage .

core:AppRegistrationResponseMessage
        rdf:type         owl:Class;
        rdfs:comment     "Message that follows up an AppRegistrationRequestMessage and contains the app registration confimation."@en;
        rdfs:label       "App Registration Response Message"@en;
        rdfs:subClassOf  core:ResponseMessage .

core:AppRepresentation
        rdf:type         owl:Class;
        rdfs:comment     "App representation"@en;
        rdfs:label       "App Representation"@en;
        rdfs:subClassOf  core:SoftwareRepresentation .

core:AppResource  rdf:type  owl:Class;
        rdfs:comment     "Resource comprising IDS data apps."@en;
        rdfs:label       "App Resource"@en;
        rdfs:subClassOf  core:Resource .

core:AppResourceCatalog
        rdf:type         owl:Class;
        rdfs:comment     "Class that aggregates App Resources from a (distributable) Catalog. May be used to list installed apps in a component."@en;
        rdfs:label       "App Resource Catalog"@en;
        rdfs:subClassOf  core:Described , odrl:AssetCollection , <http://www.w3.org/ns/dcat#Catalog> .

core:AppRoute  rdf:type  owl:Class;
        rdfs:comment     "\n    ids:AppRoute describes the communication between data apps (such as in a data processing pipeline) inside an IDS Connector.\n    An ids:AppRoute consist of multiple app endpoints which exchange data. The communication pipeline between two adjacent data apps is represented by the ids:RouteStep class.\n    ids:AppRoute also holds the information about the app endpoints, which are at the start and end of the whole processing pipeline.\n    "@en;
        rdfs:label       "App Route"@en;
        rdfs:subClassOf  core:Described .

core:AppStore  rdf:type  owl:Class;
        rdfs:comment     "Secure platform for distributing Data Apps."@en;
        rdfs:label       "App Store"@en;
        rdfs:subClassOf  core:Connector .

core:AppStoreCatalog  rdf:type  owl:Class;
        rdfs:comment     "Class that aggregates AppStores from a (distributable) Catalog."@en;
        rdfs:label       "AppStore Catalog"@en;
        rdfs:subClassOf  core:Described , core:ConnectorCatalog .

core:AppUnavailableMessage
        rdf:type         owl:Class;
        rdfs:comment     "Message indicating that a specific App should be unavailable in the AppStore."@en;
        rdfs:label       "App Unavailable Message"@en;
        rdfs:subClassOf  core:AppNotificationMessage .

core:AppUploadMessage
        rdf:type         owl:Class;
        rdfs:comment     "Message that usually follows a AppRegistrationResponseMessage and is used to upload a data app to the app store. Payload contains data app. Note that the message must refer to the prior sent, corresponding AppResource instance. The IRI of the ids:appArtifactReference must must match the IRI of the artifact which is the value for the ids:instance property. The ids:instance is specific for each representation. Therefore, if someone wants to upload multiple representations for an app, he has to state them using multiple ids:instance properties inside the AppRepresentation (and therefore inside the AppResource). Otherwise no mapping between payload and app metadata can be achieved."@en;
        rdfs:label       "App Upload Message"@en;
        rdfs:subClassOf  core:UploadMessage .

core:AppUploadResponseMessage
        rdf:type         owl:Class;
        rdfs:comment     "Message that follows up an AppUploadMessage and contains the app upload confimation."@en;
        rdfs:label       "App Upload Response Message"@en;
        rdfs:subClassOf  core:UploadResponseMessage .

core:Artifact  rdf:type   owl:Class;
        rdfs:comment      "Instance of a Representation materialized at a partiuclar version and point in time. Possesses characteristics like file name, size, creation date etc."@en;
        rdfs:label        "Artifact"@en;
        rdfs:subClassOf   core:RepresentationInstance , core:Described , odrl:Asset;
        owl:disjointWith  core:Value .

core:ArtifactRequestMessage
        rdf:type         owl:Class;
        rdfs:comment     "Message asking for retrieving the specified Artifact as the payload of an ArtifactResponse message."@en;
        rdfs:label       "Artifact Request Message"@en;
        rdfs:subClassOf  core:RequestMessage .

core:ArtifactResponseMessage
        rdf:type         owl:Class;
        rdfs:comment     "Message that follows up a RetrieveArtifact Message and contains the Artifact's data in the payload section."@en;
        rdfs:label       "Artifact Response Message"@en;
        rdfs:subClassOf  core:ResponseMessage .

core:ArtifactState  rdf:type  owl:Class;
        rdfs:comment  "The state which an ids:Artifact may have or not."@en;
        rdfs:label    "Artifact State"@en .

core:Audience  rdf:type  owl:Class;
        rdfs:comment  "The class of audiences (recipients) used in the JWT. "@en;
        rdfs:label    "Audience"@en;
        rdfs:seeAlso  <https://tools.ietf.org/html/rfc7519> .

core:AudioRepresentation
        rdf:type         owl:Class;
        rdfs:comment     "Audio representation"@en;
        rdfs:label       "Audio Representation"@en;
        rdfs:subClassOf  core:Described , <http://www.w3.org/ns/dcat#Distribution> .

core:AudioResource  rdf:type  owl:Class;
        rdfs:comment     "Resource (at least partially) comprising audio content."@en;
        rdfs:label       "Audio Resource"@en;
        rdfs:subClassOf  core:Resource .

core:AuditGuarantee  rdf:type  owl:Class;
        rdfs:comment         "Local audit logging (including integrity protection) is the baseline for auditing and clearing. Remote audit log tracing provides means to do external audit verification."@en;
        rdfs:label           "Audit guarantee"@en;
        rdfs:subClassOf      core:SecurityGuarantee;
        owl:equivalentClass  [ rdf:type   owl:Class;
                               owl:oneOf  ( <https://w3id.org/idsa/code/AUDIT_LOCAL_LOGGING> <https://w3id.org/idsa/code/AUDIT_NONE> <https://w3id.org/idsa/code/AUDIT_REMOTE_TRACING> )
                             ] .

core:AuthInfo  rdf:type  owl:Class;
        rdfs:comment  "Holds authentication information so that connections to the Connector's data offerings can be establised."@en;
        rdfs:label    "AuthInfo"@en .

core:AuthStandard  rdf:type  owl:Class;
        rdfs:comment  "The class of authentication standards that may be supported by Connectors."@en;
        rdfs:label    "AuthStandard"@en .

core:AuthenticationGuarantee
        rdf:type             owl:Class;
        rdfs:comment         "Authentication mechanism applied prior to opening a connection. Examples are the verification server's identity or doing mutual authentication."@en;
        rdfs:label           "Authentication"@en;
        rdfs:subClassOf      core:SecurityGuarantee;
        owl:equivalentClass  [ rdf:type   owl:Class;
                               owl:oneOf  ( <https://w3id.org/idsa/code/AUTHENTICATION_MUTUAL> <https://w3id.org/idsa/code/AUTHENTICATION_NONE> <https://w3id.org/idsa/code/AUTHENTICATION_SERVER_SIDE> )
                             ] .

core:BaseConnector  rdf:type  owl:Class;
        rdfs:comment     "Implementation of the Connector specification providing only restricted security capabilities."@en;
        rdfs:label       "Base Connector"@en;
        rdfs:subClassOf  core:Connector .

core:BasicAuthentication
        rdf:type         owl:Class;
        rdfs:comment     "Basic authentication using username / password "@en;
        rdfs:label       "User Authentication"@en;
        rdfs:seeAlso     <https://tools.ietf.org/html/rfc7617>;
        rdfs:subClassOf  core:UserAuthentication .

core:BinaryOperator  rdf:type  owl:Class;
        rdfs:comment     "The class of binary operators."@en;
        rdfs:label       "BinaryOperator"@en;
        rdfs:subClassOf  odrl:Operator .

core:BoundingPolygon  rdf:type  owl:Class;
        rdfs:comment     "Defines an area of interest as a set of connected points."@en;
        rdfs:label       "BoundingPolygon"@en;
        rdfs:subClassOf  core:Geometry .

core:Broker  rdf:type    owl:Class;
        rdfs:comment     "Broker holding an index of published data endpoints."@en;
        rdfs:label       "Broker"@en;
        rdfs:subClassOf  core:Connector .

core:BrokerCatalog  rdf:type  owl:Class;
        rdfs:comment     "Class that aggregates Brokers from a (distributable) Catalog."@en;
        rdfs:label       "Broker Catalog"@en;
        rdfs:subClassOf  core:Described , core:ConnectorCatalog .

core:BusinessIdentifier
        rdf:type      owl:Class;
        rdfs:comment  "A business identifier is a identification number used to identify a company. E.g., the Data Universal Numbering System, abbreviated as DUNS"@en;
        rdfs:label    "Business Identifier"@en .

core:Certification  rdf:type  owl:Class;
        rdfs:comment     "Abstract certification of compliance according to given Certification Scheme."@en;
        rdfs:label       "Certification"@en;
        rdfs:subClassOf  core:ManagedEntity .

core:CertificationLevel
        rdf:type      owl:Class;
        rdfs:comment  "Level of Certification"@en;
        rdfs:label    "Certification Level"@en .

core:ClearingHouse  rdf:type  owl:Class;
        rdfs:comment     "The Clearing House provides clearing and settlement services B2B interactions within the International Data Spaces."@en;
        rdfs:label       "Clearing House"@en;
        rdfs:subClassOf  core:InfrastructureComponent .

core:ClearingHouseCatalog
        rdf:type         owl:Class;
        rdfs:comment     "Class that aggregates Clearing Houses from a (distributable) Catalog."@en;
        rdfs:label       "Clearing House Catalog"@en;
        rdfs:subClassOf  core:Described , odrl:AssetCollection , <http://www.w3.org/ns/dcat#Catalog> .

core:CommandMessage  rdf:type  owl:Class;
        rdfs:comment     "Command messages are usually sent when a response is expected by the sender. Changes state on the recipient side. Therefore, commands are not 'safe' in the sense of REST."@en;
        rdfs:label       "Command Message"@en;
        rdfs:subClassOf  core:RequestMessage .

core:ComponentCertification
        rdf:type          owl:Class;
        rdfs:comment      "Process and result of certifying a software component/servivce in order to become a certified part of the International Data Space infrastructure."@en;
        rdfs:label        "Component Certification"@en;
        rdfs:subClassOf   core:Certification;
        rdfs:subClassOf   [ rdf:type           owl:Restriction;
                            owl:allValuesFrom  core:ComponentCertificationLevel;
                            owl:onProperty     core:certificationLevel
                          ];
        owl:disjointWith  core:ParticipantCertification .

core:ComponentCertificationLevel
        rdf:type          owl:Class;
        rdfs:comment      "Level of a Component Certification"@en;
        rdfs:label        "Component Certification Level"@en;
        rdfs:subClassOf   core:CertificationLevel;
        owl:disjointWith  core:ParticipantCertificationLevel .

core:ConfigurationModel
        rdf:type      owl:Class;
        rdfs:comment  "Configuration Model is used for Connector deployment."@en;
        rdfs:label    "Configuration Model"@en .

core:Connector  rdf:type  owl:Class;
        rdfs:comment     "Dedicated communication server for sending and receiving data in compliance with the Connector specification. There are different types of Connectors according to provided capabilities."@en;
        rdfs:label       "Connector"@en;
        rdfs:subClassOf  core:InfrastructureComponent .

core:ConnectorCatalog
        rdf:type         owl:Class;
        rdfs:comment     "Class that aggregates Connectors from a (distributable) Catalog."@en;
        rdfs:label       "Connector Catalog"@en;
        rdfs:subClassOf  core:Described , odrl:AssetCollection , <http://www.w3.org/ns/dcat#Catalog> .

core:ConnectorCertificateGrantedMessage
        rdf:type         owl:Class;
        rdfs:comment     "Whenever a Connector has been successfully certified by the Certification Body, the Identity Provider can use this message to notify Infrastructure Components."@en;
        rdfs:label       "Connector Certificate Granted Message"@en;
        rdfs:subClassOf  core:ConnectorNotificationMessage .

core:ConnectorCertificateRevokedMessage
        rdf:type         owl:Class;
        rdfs:comment     "Indicates that a (previously certified) Connector is no more certified. This could happen, for instance, if the Certification Body revokes a granted certificate or if the certificate just expires."@en;
        rdfs:label       "Connector Certificate Revoked Message"@en;
        rdfs:subClassOf  core:ConnectorNotificationMessage .

core:ConnectorDeployMode
        rdf:type      owl:Class;
        rdfs:comment  "Deploy mode of a Connector. Used mainly to capture a Connectors deployment type in the Configuration Model."@en;
        rdfs:label    "Connector Deploy Mode"@en .

core:ConnectorEndpoint
        rdf:type         owl:Class;
        rdfs:comment     "Connector-specific endpoint exposing Artifacts."@en;
        rdfs:label       "Connector Endpoint"@en;
        rdfs:subClassOf  core:Endpoint .

core:ConnectorNotificationMessage
        rdf:type         owl:Class;
        rdfs:comment     "Superclass of all messages, indicating a change of a connector's conditions."@en;
        rdfs:label       "Connector Notification Message"@en;
        rdfs:subClassOf  core:NotificationMessage .

core:ConnectorStatus  rdf:type  owl:Class;
        rdfs:comment  "Connector Status is used to represent a Connectors current state inside the Configuration Model."@en;
        rdfs:label    "Connector Status"@en .

core:ConnectorUnavailableMessage
        rdf:type         owl:Class;
        rdfs:comment     "Event notifying the recipient(s) that a connector will be unavailable. The same connector may be available again in the future."@en;
        rdfs:label       "Connector Unavailable Message"@en;
        rdfs:subClassOf  core:ConnectorNotificationMessage .

core:ConnectorUpdateMessage
        rdf:type         owl:Class;
        rdfs:comment     "Event notifying the recipient(s) about the availability and current configuration of a connector. The payload of the message must contain the updated connector's self-description."@en;
        rdfs:label       "Connector Update Message"@en;
        rdfs:subClassOf  core:ConnectorNotificationMessage .

core:ConnectorbasedAgreement
        rdf:type         owl:Class;
        rdfs:comment     "The ContractAgreement class representing the 'Connector-restricted Data Usage' policy class."@en;
        rdfs:label       "Connector-restricted Data Usage Agreement"@en;
        rdfs:subClassOf  core:ContractAgreement .

core:ConnectorbasedOffer
        rdf:type         owl:Class;
        rdfs:comment     "The ContractOffer class representing the 'Connector-restricted Data Usage' policy class."@en;
        rdfs:label       "Connector-restricted Data Usage Offer"@en;
        rdfs:subClassOf  core:ContractOffer .

core:ConnectorbasedRequest
        rdf:type         owl:Class;
        rdfs:comment     "The ContractRequest class representing the 'Connector-restricted Data Usage' policy class."@en;
        rdfs:label       "Connector-restricted Data Usage Request"@en;
        rdfs:subClassOf  core:ContractRequest .

core:Contract  rdf:type  owl:Class;
        rdfs:comment     "Abstract set of rules governing the usage of a Resource."@en;
        rdfs:label       "Contract"@en;
        rdfs:subClassOf  odrl:Policy .

core:ContractAgreement
        rdf:type          owl:Class;
        rdfs:comment      "Contract governing the actual usage of a Resource that has been agreed by all parties."@en;
        rdfs:label        "Contract agreement"@en;
        rdfs:subClassOf   core:Contract , odrl:Agreement;
        owl:disjointWith  core:ContractRequest , core:ContractOffer .

core:ContractAgreementMessage
        rdf:type         owl:Class;
        rdfs:comment     "Message containing a contract, as an instance of ids:ContractAgreement, with resource access modalities on which two parties have agreed in the payload."@en;
        rdfs:label       "Contract Agreement Message"@en;
        rdfs:subClassOf  core:ResponseMessage .

core:ContractOffer  rdf:type  owl:Class;
        rdfs:comment      "Contract issued by the Data Provider offering the usage of a Resource at particular conditions."@en;
        rdfs:label        "Contract offer"@en;
        rdfs:subClassOf   core:Contract , odrl:Offer;
        owl:disjointWith  core:ContractRequest .

core:ContractOfferMessage
        rdf:type         owl:Class;
        rdfs:comment     "Message containing a offered content contract (as offered by a data provider to the data consumer) in the associated payload (which is an instance of ids:ContractOffer). In contrast to the ids:ContractResponseMessage, the ids:ContractOfferMessage is not related to a previous contract "@en;
        rdfs:label       "Contract Offer Message"@en;
        rdfs:subClassOf  core:NotificationMessage .

core:ContractRejectionMessage
        rdf:type         owl:Class;
        rdfs:comment     "Message indicating rejection of a contract."@en;
        rdfs:label       "Contract Rejection Message"@en;
        rdfs:subClassOf  core:RejectionMessage .

core:ContractRequest  rdf:type  owl:Class;
        rdfs:comment     "Contract issued by the Data Consumer requesting the usage of a Resource at particular conditions."@en;
        rdfs:label       "Contract request"@en;
        rdfs:subClassOf  core:Contract , odrl:Request .

core:ContractRequestMessage
        rdf:type         owl:Class;
        rdfs:comment     "Message containing a suggested content contract (as offered by the data consumer to the data provider) in the associated payload (which is an instance of ids:ContractRequest)."@en;
        rdfs:label       "Contract Request Message"@en;
        rdfs:subClassOf  core:RequestMessage .

core:ContractResponseMessage
        rdf:type         owl:Class;
        rdfs:comment     "Message containing a response to a contract request (of a data consumer) in form of a counter-proposal of a contract in the associated payload (which is an instance of ids:ContractOffer). "@en;
        rdfs:label       "Contract Response Message"@en;
        rdfs:subClassOf  core:ResponseMessage .

core:ContractSupplementMessage
        rdf:type         owl:Class;
        rdfs:comment     "Message containing supplemental information to access resources of a contract (e.g., resource access tokens)."@en;
        rdfs:label       "Contract Supplement Message"@en;
        rdfs:subClassOf  core:NotificationMessage .

core:CustomMediaType  rdf:type  owl:Class;
        rdfs:comment     "A selection of custom media types to be used for data published on the IDS when no IANA type is available."@en;
        rdfs:label       "Custom Media Type"@en;
        rdfs:subClassOf  terms:MediaType .

core:DAPS  rdf:type      owl:Class;
        rdfs:comment     "The Dynamic Attribute Provisioning Service (DAPS) is a component of the Identity Provider and manages and issues the Dynamic Attribute Tokens (DAT), acting as digtial proofs for dynamic attributes of both connectors and participants."@en;
        rdfs:label       "Dynamic Attribute Provisioning Service"@en;
        rdfs:subClassOf  core:InfrastructureComponent .

core:DatPayload  rdf:type  owl:Class;
        rdfs:comment     "The Dynamic Attribute Token (DAT) Payload is the JSON Element of any DAT containing the claims of the token bearer. This payload itself is a JSON-LD encoded RDF class with a defined set of attributes. These attributes are either defined by RFC 7519 or by the IDS Information Model. As a direct consequence of regarding the DAT Payload as JSON-LD, *all* DAT Payloads must have exactly one \"@context\" attribute with the IDS context URI as its value and a \"@type\" with ids:DatPayload as its value."@en;
        rdfs:label       "DAT Payload"@en;
        rdfs:seeAlso     <https://tools.ietf.org/html/rfc7519>;
        rdfs:subClassOf  core:JwtPayload .

core:DatRequestPayload
        rdf:type         owl:Class;
        rdfs:comment     "The Dynamic Attribute Token (DAT) *Request* Payload is the JSON Element of any DAT containing the claims of the token bearer. This payload itself is a JSON-LD encoded RDF class with a defined set of attributes. These attributes are either defined by RFC 7519 or by the IDS Information Model. As a direct consequence of regarding the DAT Payload as JSON-LD, *all* DAT Payloads must have exactly one \"@context\" attribute with the IDS context URI as its value and a \"@type\" with ids:DatPayload as its value. Note that, different to the DatPayload, the DatRequestPayload contains the *self-claims* of a connector and is not yet signed by any DAPS. Consequently, no other connector must accept a DatRequest object as a DAT. A DatRequest and its contained DatRequestPayload is *only* intended for interactions with a DAPS and *nothing else*!"@en;
        rdfs:label       "DAT Request Payload"@en;
        rdfs:seeAlso     <https://tools.ietf.org/html/rfc7519>;
        rdfs:subClassOf  core:JwtPayload .

core:DataApp  rdf:type  owl:Class;
        rdfs:comment  "Self-contained, self-descriptive software package that is distributed via the App Store and deployed inside a Connector; provides access to data and data processing capa­bilities; the interface of a Data App is semantically described by the IDS Information Model."@en;
        rdfs:label    "DataApp"@en .

core:DataRepresentation
        rdf:type         owl:Class;
        rdfs:comment     "Physical representation of (structured) data."@en;
        rdfs:label       "Data representation"@en;
        rdfs:subClassOf  core:Described , <http://www.w3.org/ns/dcat#Distribution> .

core:DataResource  rdf:type  owl:Class;
        rdfs:comment     "Resource (at least partially) comprising data content."@en;
        rdfs:label       "Data Resource"@en;
        rdfs:subClassOf  core:Resource .

core:DeleteAfterIntervalAgreement
        rdf:type         owl:Class;
        rdfs:comment     "The ContractAgreement class representing the 'Interval-restricted Data Usage' policy class with the further obligation to delete the data."@en;
        rdfs:label       "Delete After Interval Agreement"@en;
        rdfs:subClassOf  core:ContractAgreement .

core:DeleteAfterIntervalOffer
        rdf:type         owl:Class;
        rdfs:comment     "The ContractOffer class representing the 'Interval-restricted Data Usage' policy class with the further obligation to delete the data."@en;
        rdfs:label       "Sales Offer"@en;
        rdfs:subClassOf  core:ContractOffer .

core:DeleteAfterIntervalRequest
        rdf:type         owl:Class;
        rdfs:comment     "The ContractRequest class representing the 'Interval-restricted Data Usage' policy class with the further obligation to delete the data."@en;
        rdfs:label       "Sales Request"@en;
        rdfs:subClassOf  core:ContractRequest .

core:Described  rdf:type  owl:Class;
        rdfs:comment  "Entity described by a minimal textual annotation, i.e. a title and description."@en;
        rdfs:label    "described"@en .

core:DescribedSemantically
        rdf:type      owl:Class;
        rdfs:comment  "Entity described semantically."@en;
        rdfs:label    "DescribedSemantically"@en .

core:DescriptionRequestMessage
        rdf:type         owl:Class;
        rdfs:comment     "Message requesting metadata. If no URI is supplied via the ids:requestedElement field, this messages is treated like a self-description request and the recipient should return its self-description via an ids:DescriptionResponseMessage. However, if a URI is supplied, the Connector should either return metadata about the requested element via an ids:DescriptionResponseMessage, or send an ids:RejectionMessage, e.g., because the element was not found."@en;
        rdfs:label       "Description Request Message"@en;
        rdfs:subClassOf  core:RequestMessage .

core:DescriptionResponseMessage
        rdf:type         owl:Class;
        rdfs:comment     "Message containing the metadata, which a Connector previously requested via the ids:DescriptionRequestMessage, in its payload."@en;
        rdfs:label       "Description Response Message"@en;
        rdfs:subClassOf  core:ResponseMessage .

core:DigitalContent  rdf:type  owl:Class;
        rdfs:comment     "Digital content of a particular type providing hints on its usage, e.g., listening to an Audio, navigating a Structure or accessing a List by an index."@en;
        rdfs:label       "Digital content"@en;
        rdfs:seeAlso     <https://github.com/twosixlabs/icas-ontology/blob/master/ontology/mime.ttl> , <https://en.wikipedia.org/wiki/Digital_content> , <http://www.ontodm.com/doku.php?id=ontodt> , <http://www.ddialliance.org/Specification/DDI-CV/GeneralDataFormat_2.0.html> , <http://schema.org/additionalType> , <http://schema.org/DataType>;
        rdfs:subClassOf  core:Described , <http://www.w3.org/ns/dcat#Dataset> .

core:DistributeEcryptedAgreement
        rdf:type         owl:Class;
        rdfs:comment     "The ContractAgreement class representing the 'Distribute only if Encrypted' policy class."@en;
        rdfs:label       "Distribute Encrypted Agreement"@en;
        rdfs:subClassOf  core:ContractAgreement .

core:DistributeEcryptedOffer
        rdf:type         owl:Class;
        rdfs:comment     "The ContractOffer class representing the 'Distribute only if Encrypted' policy class."@en;
        rdfs:label       "Distribute Encrypted Offer"@en;
        rdfs:subClassOf  core:ContractOffer .

core:DistributeEcryptedRequest
        rdf:type         owl:Class;
        rdfs:comment     "The ContractRequest class representing the 'Distribute only if Encrypted' policy class."@en;
        rdfs:label       "Distribute Encrypted Request"@en;
        rdfs:subClassOf  core:ContractRequest .

core:DurationAgreement
        rdf:type         owl:Class;
        rdfs:comment     "The ContractAgreement class representing the 'Duration-restricted Data Usage' policy class."@en;
        rdfs:label       "Duration Agreement"@en;
        rdfs:subClassOf  core:ContractAgreement .

core:DurationEntity  rdf:type  owl:Class;
        rdfs:comment     "A relative temporal entity of a certain length. Different to time:Interval, the starting point is not (yet) defined. Specifying a starting or ending point automatically transformes an instance of ids:DurationEntity to an time:Interval."@en;
        rdfs:label       "Duration"@en;
        rdfs:subClassOf  <http://www.w3.org/2006/time#TemporalEntity> .

core:DurationOffer  rdf:type  owl:Class;
        rdfs:comment     "The ContractOffer class representing the 'Duration-restricted Data Usage' policy class."@en;
        rdfs:label       "Sales Offer"@en;
        rdfs:subClassOf  core:ContractOffer .

core:DurationRequest  rdf:type  owl:Class;
        rdfs:comment     "The ContractRequest class representing the 'Duration-restricted Data Usage' policy class."@en;
        rdfs:label       "Sales Request"@en;
        rdfs:subClassOf  core:ContractRequest .

core:DynamicAttributeToken
        rdf:type         owl:Class;
        rdfs:comment     "A JSON Web Token (e.g., for authorization) mediated as part of the message, formerly known as the 'DAPS Token'. The complete JWT *including* header, payload and signiture is referenced by this class and *not* only the JSON element in the payload. See ids:DatPayload for the payload definition."@en;
        rdfs:label       "Dynamic Attribute Token (DAT)."@en;
        rdfs:seeAlso     core:DatPayload , <https://tools.ietf.org/html/rfc7519>;
        rdfs:subClassOf  core:Token .

core:Endpoint  rdf:type  owl:Class;
        rdfs:comment  "Access point of data exchange, service interaction and service description."@en;
        rdfs:label    "Endpoint"@en .

core:EvaluationFacility
        rdf:type      owl:Class;
        rdfs:comment  "Evaluation Facilities carry out the evaluation work during a certification process and issue the corresponding Certifications."@en;
        rdfs:label    "Evaluation Facility"@en .

core:EventAgreement  rdf:type  owl:Class;
        rdfs:comment     "The ContractAgreement class representing the 'Event-restricted Usage Policy' policy class."@en;
        rdfs:label       "Event-restricted Data Usage Agreement"@en;
        rdfs:subClassOf  core:ContractAgreement .

core:EventOffer  rdf:type  owl:Class;
        rdfs:comment     "The ContractOffer class representing the 'Event-restricted Usage Policy' policy class."@en;
        rdfs:label       "Event-restricted Data Usage Offer"@en;
        rdfs:subClassOf  core:ContractOffer .

core:EventRequest  rdf:type  owl:Class;
        rdfs:comment     "The ContractRequest class representing the 'Event-restricted Usage Policy' policy class."@en;
        rdfs:label       "Event-restricted Data Usage Request"@en;
        rdfs:subClassOf  core:ContractRequest .

core:Frequency  rdf:type  owl:Class;
        rdfs:comment  "Class of all frequencies."@en;
        rdfs:label    "Frequency"@en .

core:GenericEndpoint  rdf:type  owl:Class;
        rdfs:comment     "Generic endpoints describe non-IDS-specific endpoints, e.g., to integrate external services."@en;
        rdfs:label       "Generic Endpoint"@en;
        rdfs:subClassOf  core:Endpoint .

core:GeoFeature  rdf:type  owl:Class;
        rdfs:comment     "A location identified by a geonames URL."@en;
        rdfs:label       "GeoFeature"@en;
        rdfs:subClassOf  core:Location , <http://www.geonames.org/ontology#Feature> .

core:GeoPoint  rdf:type  owl:Class;
        rdfs:comment     "A location identified by geo coordinates."@en;
        rdfs:label       "GeoPoint"@en;
        rdfs:subClassOf  core:Location .

core:Geometry  rdf:type  owl:Class;
        rdfs:comment     "Geometrical shape indicating a spatial area of interest."@en;
        rdfs:label       "Geometry"@en;
        rdfs:subClassOf  core:Location , <http://www.w3.org/ns/locn#Geometry> .

core:HTTPAuthentication
        rdf:type         owl:Class;
        rdfs:comment     "HTTP authentication."@en;
        rdfs:label       "HTTP Authentication"@en;
        rdfs:subClassOf  core:BasicAuthentication .

core:IANAMediaType  rdf:type  owl:Class;
        rdfs:comment     "The class of media types registered with IANA."@en;
        rdfs:label       "IANA Media Type"@en;
        rdfs:seeAlso     <https://www.iana.org/assignments/media-types/> , <http://www.sparontologies.net/mediatype/> , <http://dx.doi.org/10.6084/m9.figshare.1608294>;
        rdfs:subClassOf  terms:MediaType .

core:IDSA  rdf:type    foaf:Organization , terms:Agent , owl:NamedIndividual;
        rdfs:label     "International Data Spaces Association";
        foaf:homepage  <https://www.internationaldataspaces.org> .

core:IdentityProvider
        rdf:type         owl:Class;
        rdfs:comment     "The Identity Provider manages and validates the digital identity of International Data Spaces Participants."@en;
        rdfs:label       "Identity provider"@en;
        rdfs:subClassOf  core:InfrastructureComponent .

core:IdsProtocolSpecification
        rdf:type      owl:Class;
        rdfs:comment  "List of all defined Protocol Specifications, for instance IDS-CP or IDS over Multipart."@en;
        rdfs:label    "Protocol Specification" .

core:ImageRepresentation
        rdf:type         owl:Class;
        rdfs:comment     "Image representation"@en;
        rdfs:label       "Image Representation"@en;
        rdfs:subClassOf  core:Described , <http://www.w3.org/ns/dcat#Distribution> .

core:ImageResource  rdf:type  owl:Class;
        rdfs:comment     "Resource (at least partially) comprising image content."@en;
        rdfs:label       "Image Resource"@en;
        rdfs:subClassOf  core:Resource .

core:InfrastructureComponent
        rdf:type         owl:Class;
        rdfs:comment     "The class of all infrastructure components of the IDS."@en;
        rdfs:label       "InfrastructureComponent"@en;
        rdfs:subClassOf  core:ManagedEntity .

core:IntegrityGuarantee
        rdf:type             owl:Class;
        rdfs:comment         "Level of integrity protection and verification of the installed software stack. Trusted boot is an example of local integrity protection, remote integrity verification comprises, for example, remote attestation."@en;
        rdfs:label           "Integrity protection and verification"@en;
        rdfs:subClassOf      core:SecurityGuarantee;
        owl:equivalentClass  [ rdf:type   owl:Class;
                               owl:oneOf  ( <https://w3id.org/idsa/code/INTEGRITY_PROTECTION_LOCAL> <https://w3id.org/idsa/code/INTEGRITY_PROTECTION_NONE> <https://w3id.org/idsa/code/INTEGRITY_VERIFICATION_REMOTE> )
                             ] .

core:IntegrityVerificationScopeGuarantee
        rdf:type             owl:Class;
        rdfs:comment         "Level/extent of verifying the software stack."@en;
        rdfs:label           "Integrity verification scope"@en;
        rdfs:subClassOf      core:SecurityGuarantee;
        owl:equivalentClass  [ rdf:type   owl:Class;
                               owl:oneOf  ( <https://w3id.org/idsa/code/INTEGRITY_VERIFICATION_SCOPE_KERNEL_CORE_CONTAINER> <https://w3id.org/idsa/code/INTEGRITY_VERIFICATION_SCOPE_KERNEL_CORE_CONTAINER_APPLICATION> <https://w3id.org/idsa/code/INTEGRITY_VERIFICATION_SCOPE_NONE> )
                             ] .

core:IntervalUsageAgreement
        rdf:type         owl:Class;
        rdfs:comment     "The ContractAgreement class representing the 'Interval-restricted Data Usage' policy class."@en;
        rdfs:label       "Interval Usage Agreement"@en;
        rdfs:subClassOf  core:ContractAgreement .

core:IntervalUsageOffer
        rdf:type         owl:Class;
        rdfs:comment     "The ContractOffer class representing the 'Interval-restricted Data Usage' policy class."@en;
        rdfs:label       "Sales Offer"@en;
        rdfs:subClassOf  core:ContractOffer .

core:IntervalUsageRequest
        rdf:type         owl:Class;
        rdfs:comment     "The ContractRequest class representing the 'Interval-restricted Data Usage' policy class."@en;
        rdfs:label       "Sales Request"@en;
        rdfs:subClassOf  core:ContractRequest .

core:InvokeOperationMessage
        rdf:type         owl:Class;
        rdfs:comment     "Message requesting the recipient to invoke a specific operation."@en;
        rdfs:label       "Invoke Operation Message"@en;
        rdfs:subClassOf  core:RequestMessage .

core:JwtPayload  rdf:type  owl:Class;
        rdfs:comment  "The payload of an JSON Web Token as a RDF class. Is used as the common parent of e.g., DatPayload and DatRequestPayload."@en;
        rdfs:label    "JWT Payload"@en .

core:KeyType  rdf:type  owl:Class;
        rdfs:comment  "Cryptographic Key Type."@en;
        rdfs:label    "Key Type"@en .

core:Language  rdf:type  owl:Class;
        rdfs:comment  "The class of languages potentially being used by textual Data Assets."@en;
        rdfs:label    "Language"@en .

core:LocalDataConfidentialityGuarantee
        rdf:type             owl:Class;
        rdfs:comment         "Means by which local data is protected."@en;
        rdfs:label           "Local data confidentiality"@en;
        rdfs:subClassOf      core:SecurityGuarantee;
        owl:equivalentClass  [ rdf:type   owl:Class;
                               owl:oneOf  ( <https://w3id.org/idsa/code/LOCAL_DATA_CONFIDENTIALITY_FULL_ENCRYPTION> <https://w3id.org/idsa/code/LOCAL_DATA_CONFIDENTIALITY_NONE> <https://w3id.org/idsa/code/LOCAL_DATA_CONFIDENTIALITY_SECURE_ERASURE> )
                             ] .

core:Location  rdf:type  owl:Class;
        rdfs:comment     "Class of all locations."@en;
        rdfs:label       "Location"@en;
        rdfs:subClassOf  wgs84_pos:SpatialThing , terms:Location .

core:LogLevel  rdf:type  owl:Class;
        rdfs:comment  "Instances of ids:LogLevel can be used to specify a log level. Currently this is only used by the Configuration Model."@en;
        rdfs:label    "Log Level"@en .

core:LogMessage  rdf:type  owl:Class;
        rdfs:comment     "Log Message which can be used to transfer logs e.g., to the clearing house."@en;
        rdfs:label       "Log Message"@en;
        rdfs:subClassOf  core:NotificationMessage .

core:LoggingAgreement
        rdf:type         owl:Class;
        rdfs:comment     "The ContractAgreement class representing the 'Local Logging' policy class."@en;
        rdfs:label       "Logging Agreement"@en;
        rdfs:subClassOf  core:ContractAgreement .

core:LoggingOffer  rdf:type  owl:Class;
        rdfs:comment     "The ContractOffer class representing the 'Local Logging' policy class."@en;
        rdfs:label       "Sales Offer"@en;
        rdfs:subClassOf  core:ContractOffer .

core:LoggingRequest  rdf:type  owl:Class;
        rdfs:comment     "The ContractRequest class representing the 'Local Logging' policy class."@en;
        rdfs:label       "Sales Request"@en;
        rdfs:subClassOf  core:ContractRequest .

core:ManagedEntity  rdf:type  owl:Class;
        rdfs:comment     "The class of mutable individuals."@en;
        rdfs:label       "Managed entity"@en;
        rdfs:subClassOf  core:Described .

core:Message  rdf:type  owl:Class;
        rdfs:comment  "Metadata describing payload exchanged by interacting Connectors."@en;
        rdfs:label    "Message"@en .

core:MessageProcessedNotificationMessage
        rdf:type         owl:Class;
        rdfs:comment     "Notification that a message has been successfully processed (i.e. not ignored or rejected)."@en;
        rdfs:label       "Message Processed Notification Message"@en;
        rdfs:subClassOf  core:NotificationMessage .

core:Named  rdf:type         owl:Class;
        rdfs:comment         "Entity that is identifiable within a context by means of a name."@en;
        rdfs:label           "Named"@en;
        owl:equivalentClass  [ rdf:type         owl:Restriction;
                               owl:cardinality  "1"^^xsd:nonNegativeInteger;
                               owl:onProperty   core:name
                             ] .

core:NotMoreThanNAgreement
        rdf:type         owl:Class;
        rdfs:comment     "The ContractAgreement class representing the 'Restricted Number of Usages' policy class."@en;
        rdfs:label       "Use Not More Than N Times Agreement"@en;
        rdfs:subClassOf  core:ContractAgreement .

core:NotMoreThanNOffer
        rdf:type         owl:Class;
        rdfs:comment     "The ContractOffer class representing the 'Restricted Number of Usages' policy class."@en;
        rdfs:label       "Sales Offer"@en;
        rdfs:subClassOf  core:ContractOffer .

core:NotMoreThanNRequest
        rdf:type         owl:Class;
        rdfs:comment     "The ContractRequest class representing the 'Restricted Number of Usages' policy class."@en;
        rdfs:label       "Sales Request"@en;
        rdfs:subClassOf  core:ContractRequest .

core:NotificationAgreement
        rdf:type         owl:Class;
        rdfs:comment     "The ContractAgreement class representing the 'Remote Notifications' policy class."@en;
        rdfs:label       "Notification Agreement"@en;
        rdfs:subClassOf  core:ContractAgreement .

core:NotificationMessage
        rdf:type         owl:Class;
        rdfs:comment     "Event messages are informative and no response is expected by the sender."@en;
        rdfs:label       "Notification Message"@en;
        rdfs:subClassOf  core:Message .

core:NotificationOffer
        rdf:type         owl:Class;
        rdfs:comment     "The ContractOffer class representing the 'Remote Notifications' policy class."@en;
        rdfs:label       "Sales Offer"@en;
        rdfs:subClassOf  core:ContractOffer .

core:NotificationRequest
        rdf:type         owl:Class;
        rdfs:comment     "The ContractRequest class representing the 'Remote Notifications' policy class."@en;
        rdfs:label       "Sales Request"@en;
        rdfs:subClassOf  core:ContractRequest .

core:OperationResultMessage
        rdf:type         owl:Class;
        rdfs:comment     "Message indicating that the result of a former InvokeOperation message is available. May transfer the result data in its associated payload section."@en;
        rdfs:label       "Operation Result Message"@en;
        rdfs:subClassOf  core:ResponseMessage .

core:OrchestrationApp
        rdf:type         owl:Class;
        rdfs:comment     "Apps for orchestrating System Adapter Apps or Smart Data Apps, inside a Connector."@en;
        rdfs:label       "Orchestration App"@en;
        rdfs:subClassOf  core:DataApp .

core:PIP  rdf:type       owl:Class;
        rdfs:comment     "Refers to the PIP that provides a specific piece of information (URI/reference to an associated PIP interface). "@en;
        rdfs:label       "policy information point"@en;
        rdfs:subClassOf  core:UsageControlComponent .

core:PXP  rdf:type       owl:Class;
        rdfs:comment     "The reference to the PXP that operates a specific action, URI or reference to an associated PXP interface."@en;
        rdfs:label       "policy execution point"@en;
        rdfs:subClassOf  core:UsageControlComponent .

core:ParIS  rdf:type     owl:Class;
        rdfs:comment     "The Participant Information Service (ParIS) provides metadata and relevant information about participants (humans and organizations) in the International Data Spaces."@en;
        rdfs:label       "Participant Information Service"@en;
        rdfs:subClassOf  core:Connector .

core:Participant  rdf:type  owl:Class;
        rdfs:comment     "Stakeholder in the International Data Spaces, assuming one or more of the predefined roles; every participant is given a unique identity by the Identity Provider."@en;
        rdfs:label       "Participant"@en;
        rdfs:subClassOf  core:ManagedEntity , foaf:Agent , org:Organization , odrl:Party .

core:ParticipantCatalog
        rdf:type         owl:Class;
        rdfs:comment     "Class that aggregates Participants from a (distributable) Catalog."@en;
        rdfs:label       "Participant Catalog"@en;
        rdfs:subClassOf  core:Described , odrl:AssetCollection , <http://www.w3.org/ns/dcat#Catalog> .

core:ParticipantCertificateGrantedMessage
        rdf:type         owl:Class;
        rdfs:comment     "Whenever a Participant has been successfully certified by the Certification Body, the Identity Provider can use this message to notify Infrastructure Components."@en;
        rdfs:label       "Participant Certificate Granted Message"@en;
        rdfs:subClassOf  core:ParticipantNotificationMessage .

core:ParticipantCertificateRevokedMessage
        rdf:type         owl:Class;
        rdfs:comment     "Indicates that a (previously certified) Participant is no more certified. This could happen, for instance, if the Certification Body revokes a granted certificate or if the certificate just expires."@en;
        rdfs:label       "Participant Certificate Revoked Message"@en;
        rdfs:subClassOf  core:ParticipantNotificationMessage .

core:ParticipantCertification
        rdf:type         owl:Class;
        rdfs:comment     "Process and result of certifying an interested party in order to become a certified member of the International Data Space."@en;
        rdfs:label       "Participant Certification"@en;
        rdfs:subClassOf  core:Certification;
        rdfs:subClassOf  [ rdf:type           owl:Restriction;
                           owl:allValuesFrom  core:ParticipantCertificationLevel;
                           owl:onProperty     core:certificationLevel
                         ] .

core:ParticipantCertificationLevel
        rdf:type         owl:Class;
        rdfs:comment     "Level of a Participant Certification"@en;
        rdfs:label       "Participant Certification Level"@en;
        rdfs:subClassOf  core:CertificationLevel .

core:ParticipantNotificationMessage
        rdf:type         owl:Class;
        rdfs:comment     "Superclass of all messages, indicating a change of a particpants's conditions."@en;
        rdfs:label       "Participant Notification Message"@en;
        rdfs:subClassOf  core:NotificationMessage .

core:ParticipantRequestMessage
        rdf:type         owl:Class;
        rdfs:comment     "This class is deprecated. Use ids:DescriptionRequestMessage instead. Message asking for retrieving the specified Participants information as the payload of an ids:ParticipantResponse message."@en;
        rdfs:label       "Participant Request Message (Deprecated)"@en;
        rdfs:subClassOf  core:RequestMessage;
        owl:deprecated   true .

core:ParticipantResponseMessage
        rdf:type         owl:Class;
        rdfs:comment     "This class is deprecated. Use ids:DescriptionResponseMessage instead. ParticipantResponseMessage follows up a ParticipantRequestMessage and contains the Participant's information in the payload section."@en;
        rdfs:label       "Participant Response Message (Deprecated)"@en;
        rdfs:subClassOf  core:ResponseMessage;
        owl:deprecated   true .

core:ParticipantUnavailableMessage
        rdf:type         owl:Class;
        rdfs:comment     "Event notifying the recipient(s) that a participant will be unavailable. The same participant may be available again in the future."@en;
        rdfs:label       "Participant Unavailable Message"@en;
        rdfs:subClassOf  core:ParticipantNotificationMessage .

core:ParticipantUpdateMessage
        rdf:type         owl:Class;
        rdfs:comment     "Event notifying the recipient(s) about the availability and current description of a participant. The payload of the message must contain the participant's self-description."@en;
        rdfs:label       "Participant Available Message"@en;
        rdfs:subClassOf  core:ParticipantNotificationMessage .

core:PaymentModality  rdf:type  owl:Class;
        rdfs:comment  "Various pricing modalities such as idsc:FREE, idsc:FIXED_PRICE and idsc:NEGOTIATION_BASIS can be used as a pre-selection to annotate the terms of the contract. Depending on the requirements, additional free text information can be attached."@en;
        rdfs:label    "Payment Modality"@en .

core:PolicyTemplate  rdf:type  owl:Class .

core:Proxy  rdf:type     owl:Class;
        rdfs:comment     "Holds Proxy information."@en;
        rdfs:label       "Proxy"@en;
        rdfs:seeAlso     <https://tools.ietf.org/html/rfc2068>;
        rdfs:subClassOf  core:Endpoint .

core:PublicKey  rdf:type  owl:Class;
        rdfs:comment  "Public key as used in asymmetric cryptography."@en;
        rdfs:label    "Public Key"@en .

core:PurposeAgreement
        rdf:type         owl:Class;
        rdfs:comment     "The ContractAgreement class representing the 'Purpose-restricted Data Usage' policy class."@en;
        rdfs:label       "Purpose Agreement"@en;
        rdfs:subClassOf  core:ContractAgreement .

core:PurposeOffer  rdf:type  owl:Class;
        rdfs:comment     "The ContractOffer class representing the 'Purpose-restricted Data Usage' policy class."@en;
        rdfs:label       "Sales Offer"@en;
        rdfs:subClassOf  core:ContractOffer .

core:PurposeRequest  rdf:type  owl:Class;
        rdfs:comment     "The ContractRequest class representing the 'Purpose-restricted Data Usage' policy class."@en;
        rdfs:label       "Sales Request"@en;
        rdfs:subClassOf  core:ContractRequest .

core:QueryLanguage  rdf:type  owl:Class;
        rdfs:comment  "Class of query languages in which query strings may be formalized."@en;
        rdfs:label    "QueryLanguage"@en .

core:QueryMessage  rdf:type  owl:Class;
        rdfs:comment     "Query message intended to be consumed by a component."@en;
        rdfs:label       "Query Message"@en;
        rdfs:subClassOf  core:RequestMessage .

core:QueryTarget  rdf:type  owl:Class;
        rdfs:comment  "Class of recipients of a query message, e.g., BROKER, APPSTORE, ANY."@en;
        rdfs:label    "Query Target"@en .

core:RejectionMessage
        rdf:type         owl:Class;
        rdfs:comment     "Rejection messages are specialized response messages that notify the sender of a message that processing of this message has failed."@en;
        rdfs:label       "Rejection Message"@en;
        rdfs:subClassOf  core:ResponseMessage .

core:RejectionReason  rdf:type  owl:Class;
        rdfs:comment  "Class of reasons that might lead to issuing a Rejection message."@en;
        rdfs:label    "RejectionReason"@en .

core:RentalAgreement  rdf:type  owl:Class;
        rdfs:comment     "The ContractAgreement class representing the 'Data Rental' policy class."@en;
        rdfs:label       "Rental Agreement"@en;
        rdfs:subClassOf  core:ContractAgreement .

core:RentalOffer  rdf:type  owl:Class;
        rdfs:comment     "The ContractOffer class representing the 'Data Rental' policy class."@en;
        rdfs:label       "Sales Offer"@en;
        rdfs:subClassOf  core:ContractOffer .

core:RentalRequest  rdf:type  owl:Class;
        rdfs:comment     "The ContractRequest class representing the 'Data Rental' policy class."@en;
        rdfs:label       "Sales Request"@en;
        rdfs:subClassOf  core:ContractRequest .

core:RepresentationInstance
        rdf:type      owl:Class;
        rdfs:comment  "A particular instance of given representation."@en;
        rdfs:label    "Representation instance"@en .

core:RequestInProcessMessage
        rdf:type         owl:Class;
        rdfs:comment     "Notification that a request has been accepted and is being processed."@en;
        rdfs:label       "Request In Process Message"@en;
        rdfs:subClassOf  core:NotificationMessage .

core:RequestMessage  rdf:type  owl:Class;
        rdfs:comment     "Client-generated message initiating a communication, motivated by a certain reason and with an answer expected."@en;
        rdfs:label       "Request Message"@en;
        rdfs:subClassOf  core:Message .

core:Resource  rdf:type  owl:Class;
        rdfs:comment     "Resource is a single digital content or a coherent set of digital contents. Resource content is formalized in Representations and optionally materialized as Artifacts. The Resource's content is exposed via defined Interfaces at various protocol Endpoints."@en;
        rdfs:label       "Resource"@en;
        rdfs:seeAlso     <https://www.w3.org/TR/vocab-dcat/#class-dataset>;
        rdfs:subClassOf  core:ManagedEntity , core:DigitalContent , core:DescribedSemantically , odrl:Asset .

core:ResourceCatalog  rdf:type  owl:Class;
        rdfs:comment     "Class that aggregates Resources from a (distributable) Catalog."@en;
        rdfs:label       "Resource Catalog"@en;
        rdfs:subClassOf  core:Described , odrl:AssetCollection , <http://www.w3.org/ns/dcat#Catalog> .

core:ResourceNotificationMessage
        rdf:type         owl:Class;
        rdfs:comment     "Superclass of all messages, indicating a change of a resource."@en;
        rdfs:label       "Resource Notification Message"@en;
        rdfs:subClassOf  core:NotificationMessage .

core:ResourceUnavailableMessage
        rdf:type         owl:Class;
        rdfs:comment     "Message indicating that a specific resource is unavailable. The same resource may be available again in the future."@en;
        rdfs:label       "Resource Unavailable Message"@en;
        rdfs:subClassOf  core:ResourceNotificationMessage .

core:ResourceUpdateMessage
        rdf:type         owl:Class;
        rdfs:comment     "Message indicating the availability and current description of a specific resource. The resource must be present in the payload of this message."@en;
        rdfs:label       "Resource Update Message"@en;
        rdfs:subClassOf  core:ResourceNotificationMessage .

core:ResponseMessage  rdf:type  owl:Class;
        rdfs:comment     "Response messages hold information about the reaction of a recipient to a formerly sent command or event. They must be correlated to this message."@en;
        rdfs:label       "Response Message"@en;
        rdfs:subClassOf  core:Message .

core:ResultMessage  rdf:type  owl:Class;
        rdfs:comment     "Result messages are intended to annotate the results of a query command. "@en;
        rdfs:label       "Result Message"@en;
        rdfs:subClassOf  core:ResponseMessage .

core:RolebasedAgreement
        rdf:type         owl:Class;
        rdfs:comment     "The ContractAgreement class representing the 'Role-restricted Data Usage' policy class."@en;
        rdfs:label       "Role-restricted Data Usage Agreement"@en;
        rdfs:subClassOf  core:ContractAgreement .

core:RolebasedOffer  rdf:type  owl:Class;
        rdfs:comment     "The ContractOffer class representing the 'Role-restricted Data Usage' policy class."@en;
        rdfs:label       "Role-restricted Data Usage Offer"@en;
        rdfs:subClassOf  core:ContractOffer .

core:RolebasedRequest
        rdf:type         owl:Class;
        rdfs:comment     "The ContractRequest class representing the 'Role-restricted Data Usage' policy class."@en;
        rdfs:label       "Role-restricted Data Usage Request"@en;
        rdfs:subClassOf  core:ContractRequest .

core:RouteStep  rdf:type  owl:Class;
        rdfs:comment     "RouteSteps hold information about a communication pipelines between apps. A RouteStep should hold\n    one value for the ids:appRouteStart and/or ids:appRouteEnd properties, so that communication between app endpoints remain distinguishable.\n    "@en;
        rdfs:label       "Route step"@en;
        rdfs:subClassOf  core:AppRoute .

core:SalesAgreement  rdf:type  owl:Class;
        rdfs:comment     "The ContractAgreement class representing the Perpetual Data Sale policy class."@en;
        rdfs:label       "Sales Agreement"@en;
        rdfs:subClassOf  core:ContractAgreement .

core:SalesOffer  rdf:type  owl:Class;
        rdfs:comment     "The ContractOffer class representing the 'Perpetual Data Sale' policy class."@en;
        rdfs:label       "Sales Offer"@en;
        rdfs:subClassOf  core:ContractOffer .

core:SalesRequest  rdf:type  owl:Class;
        rdfs:comment     "The ContractRequest class representing the 'Perpetual Data Sale' policy class."@en;
        rdfs:label       "Sales Request"@en;
        rdfs:subClassOf  core:ContractRequest .

core:SecurityAgreement
        rdf:type         owl:Class;
        rdfs:comment     "The ContractAgreement class representing the 'Security Level Restricted Policy' policy class."@en;
        rdfs:label       "Security Agreement"@en;
        rdfs:subClassOf  core:ContractAgreement .

core:SecurityGuarantee
        rdf:type      owl:Class;
        rdfs:comment  "Security guarantee claimed by a security profile."@en;
        rdfs:label    "Security guarantee"@en .

core:SecurityOffer  rdf:type  owl:Class;
        rdfs:comment     "The ContractOffer class representing the 'Security Level Restricted Policy' policy class."@en;
        rdfs:label       "Security Offer"@en;
        rdfs:subClassOf  core:ContractOffer .

core:SecurityProfile  rdf:type  owl:Class;
        rdfs:comment  "Set of security guarantees claimed by a Connector. Connectors may asses their mutual technical reliability and trustworthiness by evaluating each other’s security profile."@en;
        rdfs:label    "SecurityProfile"@en .

core:SecurityRequest  rdf:type  owl:Class;
        rdfs:comment     "The ContractRequest class representing the 'Security Level Restricted Policy' policy class."@en;
        rdfs:label       "Security Request"@en;
        rdfs:subClassOf  core:ContractRequest .

core:ServiceIsolationGuarantee
        rdf:type             owl:Class;
        rdfs:comment         "Service isolation mechanism supported by the Connector. Examples are process group (Docker) or by least privilege with clear separation and support for additional security modules as done by trustme."@en;
        rdfs:label           "Service isolation"@en;
        rdfs:subClassOf      core:SecurityGuarantee;
        owl:equivalentClass  [ rdf:type   owl:Class;
                               owl:oneOf  ( <https://w3id.org/idsa/code/SERVICE_ISOLATION_LEAST_PRIVILEGE> <https://w3id.org/idsa/code/SERVICE_ISOLATION_NONE> <https://w3id.org/idsa/code/SERVICE_ISOLATION_PROCESS_GROUP> )
                             ] .

core:SmartDataApp  rdf:type  owl:Class;
        rdfs:comment     "Smart DataApps are executing any kind of necessary data processing or transformation."@en;
        rdfs:label       "Smart DataApp"@en;
        rdfs:subClassOf  core:DataApp .

core:SoftwareRepresentation
        rdf:type         owl:Class;
        rdfs:comment     "Software representation"@en;
        rdfs:label       "Software Representation"@en;
        rdfs:subClassOf  core:Described , <http://www.w3.org/ns/dcat#Distribution> .

core:SoftwareResource
        rdf:type         owl:Class;
        rdfs:comment     "Resource (at least partially) comprising Software."@en;
        rdfs:label       "Software Resource"@en;
        rdfs:subClassOf  core:Resource .

core:SpatialAgreement
        rdf:type         owl:Class;
        rdfs:comment     "The ContractAgreement class representing the 'Location Restricted Usage' policy class."@en;
        rdfs:label       "Spatial Usage Agreement"@en;
        rdfs:subClassOf  core:ContractAgreement .

core:SpatialOffer  rdf:type  owl:Class;
        rdfs:comment     "The ContractOffer class representing the 'Location Restricted Usage' policy class."@en;
        rdfs:label       "Spatial Usage Offer"@en;
        rdfs:subClassOf  core:ContractOffer .

core:SpatialRequest  rdf:type  owl:Class;
        rdfs:comment     "The ContractRequest class representing the 'Location Restricted Usage' policy class."@en;
        rdfs:label       "Spatial Usage Request"@en;
        rdfs:subClassOf  core:ContractRequest .

core:SwapAgreement  rdf:type  owl:Class;
        rdfs:comment     "The ContractAgreement class representing the 'Data Swap' policy class."@en;
        rdfs:label       "Swap Agreement"@en;
        rdfs:subClassOf  core:ContractAgreement .

core:SwapOffer  rdf:type  owl:Class;
        rdfs:comment     "The ContractOffer class representing the 'Data Swap' policy class."@en;
        rdfs:label       "Sales Offer"@en;
        rdfs:subClassOf  core:ContractOffer .

core:SwapRequest  rdf:type  owl:Class;
        rdfs:comment     "The ContractRequest class representing the 'Data Swap' policy class."@en;
        rdfs:label       "Sales Request"@en;
        rdfs:subClassOf  core:ContractRequest .

core:SystemAdapter  rdf:type  owl:Class;
        rdfs:comment     "Data Apps that integrate sources and sinks of digital content maintained internally on Participant's premises with a Connector."@en;
        rdfs:label       "System Adapter"@en;
        rdfs:subClassOf  core:DataApp .

core:TextRepresentation
        rdf:type         owl:Class;
        rdfs:comment     "Representation of a textual content."@en;
        rdfs:label       "Text representation"@en;
        rdfs:subClassOf  core:Described , <http://www.w3.org/ns/dcat#Distribution> .

core:TextResource  rdf:type  owl:Class;
        rdfs:comment     "Resource (at least partially) comprising textual content."@en;
        rdfs:label       "Text Resource"@en;
        rdfs:subClassOf  core:Resource .

core:Token  rdf:type  owl:Class;
        rdfs:comment  "A token (e.g., for authorization) mediated as part of the message."@en;
        rdfs:label    "Token."@en .

core:TokenFormat  rdf:type  owl:Class;
        rdfs:comment  "Possible formats for (security-related) tokens."@en;
        rdfs:label    "Token format"@en .

core:TrustedConnector
        rdf:type         owl:Class;
        rdfs:comment     "Hardened implementation of the Connector specification providing enhanced security capabilities."@en;
        rdfs:label       "Trusted Connector"@en;
        rdfs:subClassOf  core:Connector .

core:UploadMessage  rdf:type  owl:Class;
        rdfs:comment     "Message used to upload a data to a recipient. Payload contains data."@en;
        rdfs:label       "Upload Message"@en;
        rdfs:subClassOf  core:RequestMessage .

core:UploadResponseMessage
        rdf:type         owl:Class;
        rdfs:comment     "Message that follows up a UploadMessage and contains the upload confirmation."@en;
        rdfs:label       "Upload Response Message"@en;
        rdfs:subClassOf  core:ResponseMessage .

core:UsageControlComponent
        rdf:type      owl:Class;
        rdfs:comment  "Defined usage control component (i.e. PIP, PXP, etc.) in the IDS."@en;
        rdfs:label    "Usage Control Component"@en .

core:UsageControlGuarantee
        rdf:type             owl:Class;
        rdfs:comment         "Extent of supporting usage control."@en;
        rdfs:label           "Usage control"@en;
        rdfs:subClassOf      core:SecurityGuarantee;
        owl:equivalentClass  [ rdf:type   owl:Class;
                               owl:oneOf  ( <https://w3id.org/idsa/code/USAGE_CONTROL_NONE> <https://w3id.org/idsa/code/USAGE_CONTROL_POLICY_ENFORCEMENT> <https://w3id.org/idsa/code/USAGE_CONTROL_REMOTE_COMPLIANCE_VERIFICATION> )
                             ] .

core:UsageControlObject
        rdf:type      owl:Class;
        rdfs:comment  "A data element containing all relevant information for usage control engines."@en;
        rdfs:label    "Usage Control Object"@en .

core:UsagePolicyClass
        rdf:type      owl:Class;
        rdfs:comment  "Defined usage policy classes in the IDS."@en;
        rdfs:label    "Usage policy class"@en .

core:UserAuthentication
        rdf:type      owl:Class;
        rdfs:comment  "Holds User authentication information. Differs from ids:AuthInfo. This class refers to user authentication methods that are not intended for direct data exchange with a connector."@en;
        rdfs:label    "User Authentication"@en .

core:Value  rdf:type     owl:Class;
        rdfs:comment     "Literal, inline value instantiation of a representation."@en;
        rdfs:label       "Value"@en;
        rdfs:subClassOf  core:RepresentationInstance .

core:VideoRepresentation
        rdf:type         owl:Class;
        rdfs:comment     "Video representation"@en;
        rdfs:label       "Video Representation"@en;
        rdfs:subClassOf  core:Described , <http://www.w3.org/ns/dcat#Distribution> .

core:VideoResource  rdf:type  owl:Class;
        rdfs:comment     "Resource (at least partially) comprising video content."@en;
        rdfs:label       "Video Resource"@en;
        rdfs:subClassOf  core:Resource .

core:accessURL  rdf:type  owl:DatatypeProperty;
        rdfs:comment  "Access URL of an endpoint."@en;
        rdfs:domain   core:Endpoint;
        rdfs:label    "access URL"@en;
        rdfs:range    xsd:anyURI;
        rdfs:seeAlso  <https://tools.ietf.org/html/rfc3986#section-3> .

core:accessed  rdf:type  owl:DatatypeProperty , owl:ObjectProperty;
        rdfs:comment  "Last read or write access."@en;
        rdfs:domain   core:UsageControlObject;
        rdfs:label    "last accessed"@en;
        rdfs:range    xsd:dateTimeStamp .

core:actionRefinement
        rdf:type      owl:ObjectProperty;
        rdfs:comment  "Constraint that refines an Action."@en;
        rdfs:domain   odrl:Action;
        rdfs:label    "action refinement"@en;
        rdfs:range    odrl:Constraint .

core:affectedConnector
        rdf:type      owl:ObjectProperty;
        rdfs:comment  "References the connector that is affected by the runtime condition change."@en;
        rdfs:domain   core:ConnectorNotificationMessage;
        rdfs:label    "affected Connector"@en;
        rdfs:range    core:Connector .

core:affectedDataApp  rdf:type  owl:ObjectProperty;
        rdfs:comment  "The affected data app that is referenced in the App-related messages. "@en;
        rdfs:domain   core:AppRegistrationRequestMessage;
        rdfs:label    "affected AppResource"@en;
        rdfs:range    core:AppResource .

core:affectedParticipant
        rdf:type      owl:ObjectProperty;
        rdfs:comment  "References the participant that is referenced in the participant-related notification messages."@en;
        rdfs:domain   core:ParticipantNotificationMessage;
        rdfs:label    "affected Participant"@en;
        rdfs:range    core:Participant .

core:affectedResource
        rdf:type      owl:ObjectProperty;
        rdfs:comment  "The affected resource that is referenced in the resource-related notification messages. "@en;
        rdfs:domain   core:ResourceNotificationMessage;
        rdfs:label    "affected Resource"@en;
        rdfs:range    core:Resource .

core:apiSpecifiation  rdf:type  owl:ObjectProperty;
        rdfs:comment  "Declares which endpoint specification is supported by this IDS endpoint.";
        rdfs:domain   core:Endpoint;
        rdfs:label    "follows API specification";
        rdfs:range    core:IdsProtocolSpecification .

core:appArtifactReference
        rdf:type      owl:ObjectProperty;
        rdfs:comment  "IRI reference to the ids:Artifact, whose corresponding data is transfered as payload of the AppUploadMessage. The Artifact IRI reference must match the IRI of the instance IRI for the corresponding ids:AppRepresentation."@en;
        rdfs:domain   core:AppUploadMessage;
        rdfs:label    "app artifact reference"@en;
        rdfs:range    core:Artifact .

core:appDocumentation
        rdf:type      owl:DatatypeProperty;
        rdfs:comment  "text documentation of the data app"@en;
        rdfs:domain   core:DataApp;
        rdfs:label    "app documentation"@en;
        rdfs:range    xsd:string .

core:appEndpoint  rdf:type  owl:ObjectProperty;
        rdfs:comment  "Endpoints of a data app"@en;
        rdfs:domain   core:DataApp;
        rdfs:label    "app endpoint"@en;
        rdfs:range    core:AppEndpoint .

core:appEndpointMediaType
        rdf:type      owl:ObjectProperty;
        rdfs:comment  "Mediatype, such as IANA types, of the data an endpoint expects or returns ."@en;
        rdfs:domain   core:AppEndpoint;
        rdfs:label    "app endpoint media type"@en;
        rdfs:range    terms:MediaType .

core:appEndpointPort  rdf:type  owl:DatatypeProperty;
        rdfs:comment  "Port used to access the endpoint."@en;
        rdfs:domain   core:AppEndpoint;
        rdfs:label    "app endpoint port"@en;
        rdfs:range    xsd:integer .

core:appEndpointProtocol
        rdf:type      owl:DatatypeProperty;
        rdfs:comment  "Protocol used to communicate with the app endpoint."@en;
        rdfs:domain   core:AppEndpoint;
        rdfs:label    "app endpoint protocol"@en;
        rdfs:range    xsd:string .

core:appEndpointType  rdf:type  owl:ObjectProperty;
        rdfs:comment  "Type of an app endpoint. Data apps have different endpoint types, e.g., for input, output or health status."@en;
        rdfs:domain   core:AppEndpoint;
        rdfs:label    "App endpoint type"@en;
        rdfs:range    core:AppEndpointType .

core:appEnvironmentVariables
        rdf:type      owl:DatatypeProperty;
        rdfs:comment  "Necessary or optional environment variables of a data app."@en;
        rdfs:domain   core:DataApp;
        rdfs:label    "app environment variables"@en;
        rdfs:range    xsd:string .

core:appRoute  rdf:type  owl:ObjectProperty;
        rdfs:domain  core:ConfigurationModel;
        rdfs:label   "app route";
        rdfs:range   core:AppRoute .

core:appRouteBroker  rdf:type  owl:ObjectProperty;
        rdfs:comment  "One or more ids:Broker(s) to which changes/updates of this route's ids:appRouteOutput ids:Resource are announced.\nThis should be a subset of those Brokers that have been configured as ids:configuredBrokers in the ids:ConfigurationModel of which this is an ids:appRoute.\n"@en;
        rdfs:domain   core:AppRoute;
        rdfs:label    "app route broker"@en;
        rdfs:range    core:Broker .

core:appRouteClearingHouse
        rdf:type      owl:ObjectProperty;
        rdfs:comment  "One or more ids:ClearingHouse(s) to which information of this route's data exchange are notified.\nThis should be a subset of clearing houses listed in the corresponding ids:ClearingHouseCatalog for a given configuration model. The Configuration Model ids:configuredClearingHouse in the ids:ConfigurationModel of which this is an ids:appRoute.\n"@en;
        rdfs:domain   core:AppRoute;
        rdfs:label    "app route broker"@en;
        rdfs:range    core:ClearingHouse .

core:appRouteEnd  rdf:type  owl:ObjectProperty;
        rdfs:comment  "End of a route."@en;
        rdfs:domain   core:AppRoute;
        rdfs:label    "app route end"@en;
        rdfs:range    core:Endpoint .

core:appRouteOutput  rdf:type  owl:ObjectProperty;
        rdfs:comment  "ids:Resource that corresponds to the output of an app route.\nRationale: whereas an ids:Endpoint can have an ids:endpointArtifact, it is additionally important that the data flow inside the ids:Connector / ids:ConfigurationModel is aware of the ids:ContractOffer (a property of ids:Resource!) associated with the data coming into the Connector or going out of the Connector.\nUse: Whenever properties of this Resource change, it may make sense to notify the ids:broker(s) configured for this AppRoute.\nNote: In an ids:AppRoute that is the sequence of multiple ids:RouteSteps, the output resource of one step serves immediately as the input that is processed by the subsequent step(s).  An ids:SystemAdapter typically does not change the ids:Resource, but might rather make it available in a different dcat:Distribution.  An ids:SmartDataApp might replate its input(s) by an entirely different (e.g., fused) resource.\n"@en;
        rdfs:domain   core:AppRoute;
        rdfs:label    "app route output"@en;
        rdfs:range    core:Resource .

core:appRouteStart  rdf:type  owl:ObjectProperty;
        rdfs:comment  "Start of a route."@en;
        rdfs:domain   core:AppRoute;
        rdfs:label    "app route start"@en;
        rdfs:range    core:Endpoint .

core:appStorageConfiguration
        rdf:type      owl:DatatypeProperty;
        rdfs:comment  "Storage configuration of a data app. Value may differ based on the app ecosystem, e.g., a writeable path in the file system or a volume name (e.g., for containerized apps)"@en;
        rdfs:domain   core:DataApp;
        rdfs:label    "app storage configuration"@en;
        rdfs:range    xsd:string .

core:assetSource  rdf:type  owl:DatatypeProperty , owl:ObjectProperty;
        rdfs:comment        "A remote link to the location (PIP) where this AssetCollection and its members are maintained."@en;
        rdfs:domain         odrl:AssetCollection;
        rdfs:label          "asset source"@en;
        rdfs:range          xsd:anyURI;
        rdfs:subPropertyOf  odrl:source .

core:aud  rdf:type    owl:ObjectProperty;
        rdfs:comment  "The 'aud' (audience) claim identifies the recipients that the JWT is intended for."@en;
        rdfs:domain   core:JwtPayload;
        rdfs:label    "aud"@en;
        rdfs:range    core:Audience;
        rdfs:seeAlso  <https://tools.ietf.org/html/rfc7519#section-4.1.3> .

core:authInfo  rdf:type  owl:ObjectProperty;
        rdfs:comment  "Information of the authentication service used by the Connector."@en;
        rdfs:domain   core:Connector;
        rdfs:label    "authInfo"@en;
        rdfs:range    core:AuthInfo .

core:authPassword  rdf:type  owl:DatatypeProperty;
        rdfs:comment  "Username / ID used for authentication.";
        rdfs:domain   core:BasicAuthentication;
        rdfs:label    "auth password";
        rdfs:range    xsd:string .

core:authService  rdf:type  owl:DatatypeProperty , owl:ObjectProperty;
        rdfs:comment  "The URL of the authentication service that is provided by the Connector."@en;
        rdfs:domain   core:AuthInfo;
        rdfs:label    "authService"@en;
        rdfs:range    xsd:anyURI .

core:authStandard  rdf:type  owl:ObjectProperty;
        rdfs:comment  "The standard used by the authentication service that is provided by the Connector."@en;
        rdfs:domain   core:AuthInfo;
        rdfs:label    "authStandard"@en;
        rdfs:range    core:AuthStandard .

core:authUsername  rdf:type  owl:DatatypeProperty;
        rdfs:comment  "Username / ID used for authentication."@en;
        rdfs:domain   core:UserAuthentication;
        rdfs:label    "auth username"@en;
        rdfs:range    xsd:string .

core:authorizationToken
        rdf:type      owl:ObjectProperty;
        rdfs:comment  "An authorization token like JSON Web Token."@en;
        rdfs:domain   core:Message;
        rdfs:label    "Authorization token"@en;
        rdfs:range    core:Token .

core:broader  rdf:type  owl:ObjectProperty;
        rdfs:comment  "This LeftOperand is transitively included in the object LeftOperand."@en;
        rdfs:domain   odrl:LeftOperand;
        rdfs:label    "broader LeftOperand"@en;
        rdfs:range    odrl:LeftOperand;
        rdfs:seeAlso  skos:broader;
        skos:broader  odrl:includedIn .

core:businessIdentifier
        rdf:type      owl:ObjectProperty;
        rdfs:comment  "Company identifiers, described via ids:BusinessIdentifier."@en;
        rdfs:domain   core:Participant;
        rdfs:label    "has business identifier"@en;
        rdfs:range    core:BusinessIdentifier .

core:byteSize  rdf:type     owl:DatatypeProperty;
        rdfs:comment        "Size of the Artifact in bytes."@en;
        rdfs:domain         core:Artifact;
        rdfs:label          "byte size"@en;
        rdfs:range          xsd:integer;
        rdfs:subPropertyOf  <http://www.w3.org/ns/dcat#byteSize> .

core:callbackAddress  rdf:type  owl:DatatypeProperty;
        rdfs:comment  "A callback address must be provided in a request message and a notification message. "@en;
        rdfs:domain   [ rdf:type     owl:Class;
                        owl:unionOf  ( core:NotificationMessage core:RequestMessage )
                      ];
        rdfs:label    "callback address"@en;
        rdfs:range    xsd:anyURI .

core:certificationLevel
        rdf:type      owl:ObjectProperty;
        rdfs:comment  "Level of certification (based on a combination of requierements, evaluation method etc.)"@en;
        rdfs:domain   core:Certification;
        rdfs:label    "certification level"@en;
        rdfs:range    core:CertificationLevel .

core:checkSum  rdf:type  owl:DatatypeProperty;
        rdfs:comment  "Checksum of the artifact"@en;
        rdfs:domain   core:Artifact;
        rdfs:label    "checksum"@en;
        rdfs:range    xsd:string .

core:componentCertification
        rdf:type      owl:ObjectProperty;
        rdfs:comment  "Certification issued for the given Infrastructure Component."@en;
        rdfs:domain   core:InfrastructureComponent;
        rdfs:label    "component certification"@en;
        rdfs:range    core:ComponentCertification .

core:configurationModelLogLevel
        rdf:type      owl:ObjectProperty;
        rdfs:comment  "Log level configuration for a Connector which is deployed using the Configuration Model"@en;
        rdfs:domain   core:ConfigurationModel;
        rdfs:label    "configuration model log level"@en;
        rdfs:range    core:LogLevel .

core:configuredAppResource
        rdf:type      owl:ObjectProperty;
        rdfs:comment  "Catalog of app resources for a given Configuration Model. Used to persist configured / installed apps."@en;
        rdfs:domain   core:ConfigurationModel;
        rdfs:label    "configured app resources"@en;
        rdfs:range    core:AppResourceCatalog .

core:configuredAppStore
        rdf:type      owl:ObjectProperty;
        rdfs:comment  "One or more app stores to which the ids:Connector that we are configuring (cf. ids:connectorDescription) may want to talk, e.g., to retrieve apps from them."@en;
        rdfs:domain   core:ConfigurationModel;
        rdfs:label    "configured appstore"@en;
        rdfs:range    core:AppStoreCatalog .

core:configuredBroker
        rdf:type      owl:ObjectProperty;
        rdfs:comment  "Catalog of Brokers to which the ids:Connector that we are configuring (cf. ids:connectorDescription) may want to talk."@en;
        rdfs:domain   core:ConfigurationModel;
        rdfs:label    "configured broker"@en;
        rdfs:range    core:BrokerCatalog .

core:configuredClearingHouse
        rdf:type      owl:ObjectProperty;
        rdfs:comment  "Catalog of clearing houses for a given Configuration Model."@en;
        rdfs:domain   core:ConfigurationModel;
        rdfs:label    "configured clearing house"@en;
        rdfs:range    core:ClearingHouseCatalog .

core:connectorCatalog
        rdf:type      owl:ObjectProperty;
        rdfs:comment  "Reference to catalog of Connectors, which are listed in the Broker."@en;
        rdfs:domain   core:Broker;
        rdfs:label    "connector Catalog"@en;
        rdfs:range    core:ConnectorCatalog .

core:connectorDeployMode
        rdf:type      owl:ObjectProperty;
        rdfs:comment  "Deply mode of a Connector in the Configuration Model"@en;
        rdfs:domain   core:ConfigurationModel;
        rdfs:label    "connector deploy mode"@en;
        rdfs:range    core:ConnectorDeployMode .

core:connectorDescription
        rdf:type      owl:ObjectProperty;
        rdfs:comment  "References to Connector which is deployed / maintained in the Configuration Model"@en;
        rdfs:domain   core:ConfigurationModel;
        rdfs:label    "Connector description"@en;
        rdfs:range    core:Connector .

core:connectorProxy  rdf:type  owl:ObjectProperty;
        rdfs:comment  "Proxies for a Connector which is deployed using the Configuration Model"@en;
        rdfs:domain   core:ConfigurationModel;
        rdfs:label    "Connector proxy"@en;
        rdfs:range    core:Proxy .

core:connectorStatus  rdf:type  owl:ObjectProperty;
        rdfs:comment  "Status of a Connector deployed by the Configuration Model"@en;
        rdfs:domain   core:ConfigurationModel;
        rdfs:label    "Connector Status"@en;
        rdfs:range    core:ConnectorStatus .

core:consumer  rdf:type  owl:ObjectProperty;
        rdfs:comment  "Consumer of a Resource or Service that is the subject matter of the Contract. This party may differ from the Assignee specified by the Contract rules."@en;
        rdfs:domain   core:Contract;
        rdfs:label    "Consumer"@en;
        rdfs:range    core:Participant .

core:contentPart  rdf:type  owl:ObjectProperty;
        rdfs:comment  "Reference to a Digital Content (physically or logically) included, definition of part-whole hierarchies."@en;
        rdfs:domain   core:DigitalContent;
        rdfs:label    "content part"@en;
        rdfs:range    core:DigitalContent .

core:contentStandard  rdf:type  owl:DatatypeProperty;
        rdfs:comment        "IRI containing document, which defines the standard for the given Digital Content. The content is assumed to conform to that Standard."@en;
        rdfs:domain         core:DigitalContent;
        rdfs:label          "content standard"@en;
        rdfs:range          xsd:anyURI;
        rdfs:subPropertyOf  terms:conformsTo .

core:contentType  rdf:type  owl:ObjectProperty;
        rdfs:comment        "Detailed type, genre or interpretation of the Digital Content."@en;
        rdfs:domain         core:DigitalContent;
        rdfs:label          "content type"@en;
        rdfs:range          terms:DCMIType;
        rdfs:subPropertyOf  terms:type .

core:contentVersion  rdf:type  owl:DatatypeProperty;
        rdfs:comment  "Version of the content in the payload. Use digits and semantic versioning pattern like MAJOR.MINOR.PATCH."@en;
        rdfs:domain   core:Message;
        rdfs:label    "contentVersion"@en;
        rdfs:range    xsd:string .

core:contract  rdf:type  owl:ObjectProperty;
        rdfs:comment  "The target contract defining the usage of the data object."@en;
        rdfs:domain   core:UsageControlObject;
        rdfs:label    "has contract"@en;
        rdfs:range    core:ContractAgreement .

core:contractAnnex  rdf:type  owl:ObjectProperty;
        rdfs:comment  "Any type of resource related to the Contract."@en;
        rdfs:domain   core:Contract;
        rdfs:label    "Annex to contract"@en;
        rdfs:range    core:Resource .

core:contractDate  rdf:type  owl:DatatypeProperty;
        rdfs:comment  "Absolute datetime of signing the Contract."@en;
        rdfs:domain   core:Contract;
        rdfs:label    "Contract date"@en;
        rdfs:range    xsd:dateTimeStamp .

core:contractDocument
        rdf:type      owl:ObjectProperty;
        rdfs:comment  "Equivalent human-readable encoding of this machine-interpretable Contract."@en;
        rdfs:domain   core:Contract;
        rdfs:label    "Contract document"@en;
        rdfs:range    core:TextResource .

core:contractEnd  rdf:type  owl:DatatypeProperty;
        rdfs:comment  "Absolute datetime the Contract is requested, offered or expected to end. If omitted, the contract has to be explicitly terminated by any of the parties."@en;
        rdfs:domain   core:Contract;
        rdfs:label    "Contract end"@en;
        rdfs:range    xsd:dateTimeStamp .

core:contractOffer  rdf:type  owl:ObjectProperty;
        rdfs:comment  "Reference to a Contract Offer defining the authorized use of the Resource."@en;
        rdfs:domain   core:Resource;
        rdfs:label    "contract offer"@en;
        rdfs:range    core:ContractOffer .

core:contractRejectionReason
        rdf:type      owl:DatatypeProperty;
        rdfs:comment  "Human-readable text describing the reason for contract rejection."@en;
        rdfs:domain   core:ContractRejectionMessage;
        rdfs:label    "Contract Rejection Reason"@en;
        rdfs:range    xsd:string .

core:contractStart  rdf:type  owl:DatatypeProperty;
        rdfs:comment  "Absolute datetime the Contract is requested, offered or expected to start, depending on the type of Contract."@en;
        rdfs:domain   core:Contract;
        rdfs:label    "Contract start"@en;
        rdfs:range    xsd:dateTimeStamp .

core:correlationMessage
        rdf:type      owl:ObjectProperty;
        rdfs:comment  "Correlated message, e.g., a response to a previous request."@en;
        rdfs:domain   core:Message;
        rdfs:label    "consumer connector"@en;
        rdfs:range    core:Message .

core:curator  rdf:type      owl:ObjectProperty;
        rdfs:comment        "Participant responsible for the correctness of the content offered by the InfrastructureComponent."@en;
        rdfs:domain         core:InfrastructureComponent;
        rdfs:label          "curator"@en;
        rdfs:range          core:Participant;
        rdfs:subPropertyOf  terms:publisher .

core:data  rdf:type   owl:DatatypeProperty , owl:ObjectProperty;
        rdfs:comment  "The related data or a pointer/reference to it."@en;
        rdfs:domain   core:UsageControlObject;
        rdfs:label    "has data"@en;
        rdfs:range    xsd:anyURI .

core:dataAppDistributionService
        rdf:type      owl:DatatypeProperty;
        rdfs:comment  "IRI reference to storage and distribution system for the corresponding data app. Unlike regular representations for IDS resources, a data app may not be retrieved directly from a connector but from a separate registry instead."@en;
        rdfs:domain   core:AppRepresentation;
        rdfs:label    "data app distribution service"@en;
        rdfs:range    xsd:anyURI .

core:dataAppInformation
        rdf:type      owl:ObjectProperty;
        rdfs:comment  "Information about the concrete data app implementation"@en;
        rdfs:domain   core:AppRepresentation;
        rdfs:label    "data app information"@en;
        rdfs:range    core:DataApp .

core:dataAppRuntimeEnvironment
        rdf:type      owl:DatatypeProperty;
        rdfs:comment  "Runtime environment of a data app, e.g., software (or hardware) required to run the app."@en;
        rdfs:domain   core:AppRepresentation;
        rdfs:label    "data app runtime environment"@en;
        rdfs:range    xsd:string .

core:dataType  rdf:type  owl:DatatypeProperty;
        rdfs:comment  "Indicates the data type of the Representation."@en;
        rdfs:domain   core:DataRepresentation;
        rdfs:label    "Data type"@en;
        rdfs:range    xsd:anyURI .

core:dataTypeSchema  rdf:type  owl:ObjectProperty;
        rdfs:comment  "Indicates the data type schema of the Representation."@en;
        rdfs:domain   core:DataRepresentation;
        rdfs:label    "Data Type Schema"@en;
        rdfs:range    core:Resource .

core:defaultRepresentation
        rdf:type            owl:ObjectProperty;
        rdfs:comment        "Default representation of the content."@en;
        rdfs:domain         core:DigitalContent;
        rdfs:label          "Default representation"@en;
        rdfs:range          <http://www.w3.org/ns/dcat#Distribution>;
        rdfs:subPropertyOf  core:representation .

core:duration  rdf:type  owl:DatatypeProperty;
        rdfs:comment  "Duration of the media resource in seconds."@en;
        rdfs:domain   core:Artifact;
        rdfs:label    "duration"@en;
        rdfs:range    xsd:decimal .

core:endpointArtifact
        rdf:type      owl:ObjectProperty;
        rdfs:comment  "Content instance mediated via this individual endpoint (1:1 mapping)."@en;
        rdfs:domain   core:ConnectorEndpoint;
        rdfs:label    "endpoint artifact"@en;
        rdfs:range    core:Artifact .

core:endpointDocumentation
        rdf:type      owl:DatatypeProperty;
        rdfs:comment  "IRI reference to a documentation of the endpoint, e.g., reference to an OpenAPI-based documentation."@en;
        rdfs:domain   core:Endpoint;
        rdfs:label    "endpoint documentation"@en;
        rdfs:range    xsd:anyURI .

core:endpointInformation
        rdf:type      owl:DatatypeProperty;
        rdfs:comment  "Human-readable information and description of the endpoint."@en;
        rdfs:domain   core:Endpoint;
        rdfs:label    "endpoint information"@en;
        rdfs:range    xsd:string .

core:endpointURI  rdf:type  owl:DatatypeProperty , owl:ObjectProperty;
        rdfs:comment  "The reference to a URI that expresses an exact endpoint of that usage control endpoint."@en;
        rdfs:domain   core:UsageControlComponent;
        rdfs:label    "endpoint URI"@en;
        rdfs:range    xsd:anyURI .

core:evaluationFacility
        rdf:type      owl:ObjectProperty;
        rdfs:comment  "Evaluation Facility that performed and issued given Certification"@en;
        rdfs:domain   core:Certification;
        rdfs:label    "evaluation facility"@en;
        rdfs:range    core:EvaluationFacility .

core:exp  rdf:type    owl:DatatypeProperty;
        rdfs:comment  "The 'exp' (expiration time) claim identifies the expiration time on or after which the JWT MUST NOT be accepted for processing."@en;
        rdfs:domain   core:JwtPayload;
        rdfs:label    "exp"@en;
        rdfs:range    xsd:integer;
        rdfs:seeAlso  <https://tools.ietf.org/html/rfc7519#section-4.1.4> .

core:extendedGuarantee
        rdf:type      owl:ObjectProperty;
        rdfs:comment  "Reference to a security guarantee that, if used in combination with a security profile instance, overrides the respective guarantee of the given predefined instance."@en;
        rdfs:domain   [ rdf:type     owl:Class;
                        owl:unionOf  ( core:Connector core:DatPayload )
                      ];
        rdfs:label    "extended guarantee"@en;
        rdfs:range    core:SecurityGuarantee .

core:fileName  rdf:type  owl:DatatypeProperty;
        rdfs:comment  "Name of the Artifcat file."@en;
        rdfs:domain   core:Artifact;
        rdfs:label    "file name"@en;
        rdfs:range    xsd:string .

core:filenameExtension
        rdf:type      owl:DatatypeProperty;
        rdfs:comment  "Suffix of a file name, typically separated by a period, indicating the nature and intended processing of the file."@en;
        rdfs:domain   terms:MediaType;
        rdfs:label    "filename extension"@en;
        rdfs:range    xsd:string;
        rdfs:seeAlso  <https://en.wikipedia.org/wiki/Filename_extension> .

core:frameRate  rdf:type  owl:DatatypeProperty;
        rdfs:comment  "Video frame rate, as frames/second."@en;
        rdfs:domain   core:VideoRepresentation;
        rdfs:label    "frame rate"@en;
        rdfs:range    xsd:decimal .

core:genericEndpointAuthentication
        rdf:type      owl:ObjectProperty;
        rdfs:comment  "Authentication credentials for generic endpoints. "@en;
        rdfs:domain   core:GenericEndpoint;
        rdfs:label    "generic endpoint authentication"@en;
        rdfs:range    core:BasicAuthentication .

core:genericEndpointConfiguration
        rdf:type      owl:DatatypeProperty;
        rdfs:comment  "Endpoint-specific configuration details (e.g., contents of a config file) used for the endpoint."@en;
        rdfs:domain   core:GenericEndpoint;
        rdfs:label    "generic endpoint configuration"@en;
        rdfs:range    xsd:string .

core:geoPoint  rdf:type  owl:ObjectProperty;
        rdfs:comment  "Refers to a GeoPoint that is member of a BoundingPolygon."@en;
        rdfs:domain   core:BoundingPolygon;
        rdfs:label    "geoPoint"@en;
        rdfs:range    core:GeoPoint .

core:hasAgent  rdf:type  owl:ObjectProperty;
        rdfs:comment  "The Agents for which this Connector may initiate and receive Messages."@en;
        rdfs:domain   core:Connector;
        rdfs:label    "has Agent"@en;
        rdfs:range    foaf:Agent .

core:hasDefaultEndpoint
        rdf:type      owl:ObjectProperty;
        rdfs:comment  "Indicates the default endpoint that should be used for basic infrastructure interactions, e.g., providing the self description."@en;
        rdfs:domain   core:Connector;
        rdfs:label    "has default endpoint"@en;
        rdfs:range    core:ConnectorEndpoint .

core:hasDuration  rdf:type  owl:DatatypeProperty;
        rdfs:comment  "Duration (relative time interval) of a temporal specification. Different to the TIME Ontology, durations are expressed using the xsd:duration datatype. In case it is used with a instance of time:Instant, the value must be 'P0Y0M0DT0H0M0S'^^xsd:duration."@en;
        rdfs:domain   <http://www.w3.org/2006/time#TemporalEntity>;
        rdfs:label    "has duration"@en;
        rdfs:range    xsd:duration;
        rdfs:seeAlso  <http://www.w3.org/2006/time#hasDuration> .

core:hasEndpoint  rdf:type  owl:ObjectProperty;
        rdfs:comment  "Reference to the Endpoints that serve the resource's content or let you exchange messages with an IDS Connector."@en;
        rdfs:domain   core:Connector;
        rdfs:label    "has endpoint"@en;
        rdfs:range    core:ConnectorEndpoint .

core:hasState  rdf:type  owl:ObjectProperty;
        rdfs:comment  "The list of combined current states of the data object."@en;
        rdfs:domain   core:UsageControlObject;
        rdfs:label    "has state"@en;
        rdfs:range    core:ArtifactState .

core:hasSubRoute  rdf:type  owl:ObjectProperty;
        rdfs:comment  "Route between two or more app endpoints inside a app routing pipeline."@en;
        rdfs:domain   core:AppRoute;
        rdfs:label    "sub route"@en;
        rdfs:range    core:RouteStep .

core:height  rdf:type  owl:DatatypeProperty;
        rdfs:comment  "Height of the visible frame."@en;
        rdfs:domain   core:ImageRepresentation;
        rdfs:label    "height"@en;
        rdfs:range    xsd:decimal .

core:httpAuthURI  rdf:type  owl:DatatypeProperty;
        rdfs:comment  "HTTP authentication URI."@en;
        rdfs:domain   core:HTTPAuthentication;
        rdfs:label    "http auth URI"@en;
        rdfs:range    xsd:anyURI;
        rdfs:seeAlso  <https://tools.ietf.org/html/rfc7235> .

core:iat  rdf:type    owl:DatatypeProperty;
        rdfs:comment  "The 'iat' (issued at) claim contains the point in time when the JWT was created."@en;
        rdfs:domain   core:JwtPayload;
        rdfs:label    "iat"@en;
        rdfs:range    xsd:integer .

core:identifierSystem
        rdf:type      owl:DatatypeProperty;
        rdfs:comment  "This property is used to define the system used as an business identifier. E.g., DUNS or SIRET."@en;
        rdfs:domain   core:BusinessIdentifier;
        rdfs:label    "identifier system"@en;
        rdfs:range    xsd:string .

core:inboundModelVersion
        rdf:type      owl:DatatypeProperty;
        rdfs:comment  "Information Model version that the InfrastructureComponent is capable of reading/processing."@en;
        rdfs:domain   core:InfrastructureComponent;
        rdfs:label    "inboundModelVersion"@en;
        rdfs:range    xsd:string .

core:inboundPath  rdf:type  owl:DatatypeProperty;
        rdfs:comment  "Relative path used for inbound communication via this endpoint, i.e., input messages and faults only."@en;
        rdfs:domain   core:Endpoint;
        rdfs:label    "inbound topic"@en;
        rdfs:range    xsd:string .

core:includedCertificationLevel
        rdf:type            owl:ObjectProperty;
        rdfs:comment        "Certification Level transitively implied by given Certification Level of same root type."@en;
        rdfs:domain         core:CertificationLevel;
        rdfs:label          "included certification level"@en;
        rdfs:range          core:CertificationLevel;
        rdfs:seeAlso        <https://www.w3.org/TR/odrl-vocab/#term-includedIn>;
        rdfs:subPropertyOf  terms:isPartOf .

core:instance  rdf:type  owl:ObjectProperty;
        rdfs:comment  "Reference to an instance of given representation, i.e. inline value or file placeholder."@en;
        rdfs:domain   <http://www.w3.org/ns/dcat#Distribution>;
        rdfs:label    "instance"@en;
        rdfs:range    core:RepresentationInstance .

core:interfaceDescription
        rdf:type      owl:DatatypeProperty , owl:ObjectProperty;
        rdfs:comment  "The reference to a URI that provides the interface description of a usage control endpoint."@en;
        rdfs:domain   core:UsageControlComponent;
        rdfs:label    "interface description"@en;
        rdfs:range    xsd:anyURI .

core:iss  rdf:type    owl:DatatypeProperty;
        rdfs:comment  "The 'iss' (issuer) claim identifies the principal that issued the JWT."@en;
        rdfs:domain   core:JwtPayload;
        rdfs:label    "iss"@en;
        rdfs:range    xsd:string;
        rdfs:seeAlso  <https://tools.ietf.org/html/rfc7519#section-4.1.1> .

core:issuerConnector  rdf:type  owl:DatatypeProperty , owl:ObjectProperty;
        rdfs:comment  "The Connector which is the origin of the message."@en;
        rdfs:domain   core:Message;
        rdfs:label    "issuer connector"@en;
        rdfs:range    core:Connector .

core:jurisdiction  rdf:type  owl:DatatypeProperty;
        rdfs:comment  "jurisdiction / court which is responsible for the entity. The use of existing standards such as ISO 3166-2 is recommended."@en;
        rdfs:domain   core:Participant;
        rdfs:label    "legal form"@en;
        rdfs:range    xsd:string .

core:keyStore  rdf:type  owl:DatatypeProperty;
        rdfs:comment  "URI of the key store server."@en;
        rdfs:domain   core:ConfigurationModel;
        rdfs:label    "key store"@en;
        rdfs:range    xsd:anyURI .

core:keyStoreAlias  rdf:type  owl:DatatypeProperty;
        rdfs:comment  "alias for the key store."@en;
        rdfs:domain   core:ConfigurationModel;
        rdfs:label    "key store alias"@en;
        rdfs:range    xsd:string .

core:keyStorePassword
        rdf:type      owl:DatatypeProperty;
        rdfs:comment  "Password of the key store server."@en;
        rdfs:domain   core:ConfigurationModel;
        rdfs:label    "key store password"@en;
        rdfs:range    xsd:string .

core:keyType  rdf:type  owl:ObjectProperty;
        rdfs:comment  "Type of the public key."@en;
        rdfs:domain   core:PublicKey;
        rdfs:label    "Key Type"@en;
        rdfs:range    core:KeyType .

core:keyValue  rdf:type  owl:DatatypeProperty;
        rdfs:comment  "Binary representation of the key."@en;
        rdfs:domain   core:PublicKey;
        rdfs:label    "Key Value"@en;
        rdfs:range    xsd:base64Binary .

core:lastValidDate  rdf:type  owl:DatatypeProperty;
        rdfs:comment  "Last date (as xsd:dateTimeStamp) the given Certification is considered valid."@en;
        rdfs:domain   core:Certification;
        rdfs:label    "last valid date"@en;
        rdfs:range    xsd:dateTimeStamp .

core:latitude  rdf:type     owl:DatatypeProperty , owl:AnnotationProperty;
        rdfs:comment        "Latitude of a GeoPoint (decimal degrees)."@en;
        rdfs:domain         core:GeoPoint;
        rdfs:label          "latitude"@en;
        rdfs:range          xsd:float;
        rdfs:subPropertyOf  wgs84_pos:lat .

core:legalForm  rdf:type  owl:DatatypeProperty;
        rdfs:comment  "Legal form of the participant. It is advisable to use an existing standard such as ISO-20275."@en;
        rdfs:domain   core:Participant;
        rdfs:label    "legal form"@en;
        rdfs:range    xsd:string;
        rdfs:seeAlso  <https://www.gleif.org/en/about-lei/code-lists/iso-20275-entity-legal-forms-code-list/> .

core:legalName  rdf:type  owl:DatatypeProperty;
        rdfs:comment  "The complete legal name of a Participant. Unlike the title property for the participant which refers to the commonly used name or term for the Participant, a legal name identifies a participant for legal, administrative and other official purposes."@en;
        rdfs:domain   core:Participant;
        rdfs:label    "legal name"@en;
        rdfs:range    xsd:string .

core:listedAppResource
        rdf:type            owl:ObjectProperty;
        rdfs:comment        "An AppResource that is part of an AppResourceCatalog."@en;
        rdfs:domain         core:AppResourceCatalog;
        rdfs:label          "listed AppResource"@en;
        rdfs:range          core:AppResource;
        rdfs:subPropertyOf  <http://www.w3.org/ns/dcat#dataset> .

core:listedClearingHouse
        rdf:type            owl:ObjectProperty;
        rdfs:comment        "A Clearing House that is part of a Clearing House catalog."@en;
        rdfs:domain         core:ClearingHouseCatalog;
        rdfs:label          "listed Clearing House"@en;
        rdfs:range          core:ClearingHouse;
        rdfs:subPropertyOf  <http://www.w3.org/ns/dcat#dataset> .

core:listedConnector  rdf:type  owl:ObjectProperty;
        rdfs:comment        "A Connector that is part of a Connector catalog."@en;
        rdfs:domain         core:ConnectorCatalog;
        rdfs:label          "listed Connector"@en;
        rdfs:range          core:Connector;
        rdfs:subPropertyOf  <http://www.w3.org/ns/dcat#dataset> .

core:longitude  rdf:type    owl:DatatypeProperty , owl:AnnotationProperty;
        rdfs:comment        "Longitude of a GeoPoint (decimal degrees)."@en;
        rdfs:domain         core:GeoPoint;
        rdfs:label          "longitude"@en;
        rdfs:range          xsd:float;
        rdfs:subPropertyOf  wgs84_pos:long .

core:maintainer  rdf:type  owl:ObjectProperty;
        rdfs:comment  "Participant responsible for technical maintenance of the InfrastructureComponent."@en;
        rdfs:domain   core:InfrastructureComponent;
        rdfs:label    "maintainer"@en;
        rdfs:range    core:Participant .

core:member  rdf:type       owl:ObjectProperty;
        rdfs:comment        "A Participant that is part of a participant catalog."@en;
        rdfs:domain         core:ParticipantCatalog;
        rdfs:label          "member"@en;
        rdfs:range          core:Participant;
        rdfs:subPropertyOf  <http://www.w3.org/ns/dcat#dataset> .

core:memberParticipant
        rdf:type            owl:ObjectProperty , owl:AnnotationProperty;
        rdfs:comment        "Indicates that a participant has a member which is again a participant. This is useful for defining hierarchical relations in a participant's organization as well as identifying groups of participants to capture, e.g., members of a collaboration."@en;
        rdfs:domain         core:Participant;
        rdfs:label          "member participant"@en;
        rdfs:range          core:Participant;
        rdfs:subPropertyOf  org:hasMember .

core:memberPerson  rdf:type  owl:ObjectProperty , owl:AnnotationProperty;
        rdfs:comment        "Indicates membership of a person to an organization."@en;
        rdfs:domain         core:Participant;
        rdfs:label          "memberPerson"@en;
        rdfs:range          foaf:Person;
        rdfs:subPropertyOf  org:hasMember .

core:membershipEnd  rdf:type  owl:DatatypeProperty;
        rdfs:comment  "End of the participant's IDS membership."@en;
        rdfs:domain   core:ParticipantCertification;
        rdfs:label    "membership end"@en;
        rdfs:range    xsd:dateTimeStamp .

core:modelVersion  rdf:type  owl:DatatypeProperty;
        rdfs:comment  "Version of the Information Model against which the Message should be interpreted."@en;
        rdfs:domain   core:Message;
        rdfs:label    "model version"@en;
        rdfs:range    xsd:string .

core:name  rdf:type   owl:FunctionalProperty , owl:DatatypeProperty;
        rdfs:comment  "Entity name unique within a specified context."@en;
        rdfs:domain   core:Named;
        rdfs:label    "name"@en;
        rdfs:range    xsd:string .

core:nbf  rdf:type    owl:DatatypeProperty;
        rdfs:comment  "The 'aud' (audience) claim identifies the recipients that the JWT is intended for."@en;
        rdfs:domain   core:JwtPayload;
        rdfs:label    "nbf"@en;
        rdfs:range    xsd:integer;
        rdfs:seeAlso  <https://tools.ietf.org/html/rfc7519#section-4.1.5> .

core:noProxy  rdf:type  owl:DatatypeProperty;
        rdfs:comment  "URLs that should be excluded from proxying.GNU emcs documentation contains a good explanation for the usage of noProxy."@en;
        rdfs:domain   core:Proxy;
        rdfs:label    "no proxy"@en;
        rdfs:range    xsd:anyURI;
        rdfs:seeAlso  <https://www.gnu.org/software/emacs/manual/html_node/url/Proxies.html> .

core:offeredResource  rdf:type  owl:ObjectProperty;
        rdfs:comment        "A Resource that is part of a resource catalog, indicating an offering (of, e.g., data)."@en;
        rdfs:domain         core:ResourceCatalog;
        rdfs:label          "offered resource"@en;
        rdfs:range          core:Resource;
        rdfs:subPropertyOf  <http://www.w3.org/ns/dcat#dataset> .

core:operationReference
        rdf:type      owl:DatatypeProperty;
        rdfs:comment  "References the operation to be invoked on the recipient's side by an URI."@en;
        rdfs:domain   core:InvokeOperationMessage;
        rdfs:label    "Operation Reference"@en;
        rdfs:range    xsd:anyURI .

core:outboundModelVersion
        rdf:type      owl:DatatypeProperty;
        rdfs:comment  "Information Model version being produced by the InfrastructureComponent."@en;
        rdfs:domain   core:InfrastructureComponent;
        rdfs:label    "outbound model version"@en;
        rdfs:range    xsd:string .

core:outboundPath  rdf:type  owl:DatatypeProperty;
        rdfs:comment  "Relative path used for outbound communication via this endpoint, i.e., output messages and faults only."@en;
        rdfs:domain   core:Endpoint;
        rdfs:label    "outbound topic"@en;
        rdfs:range    xsd:string .

core:participantCatalog
        rdf:type      owl:ObjectProperty;
        rdfs:comment  "List of participants a ParIS may expose."@en;
        rdfs:domain   core:ParIS;
        rdfs:label    "participant catalog"@en;
        rdfs:range    core:ParticipantCatalog .

core:participantCertification
        rdf:type      owl:ObjectProperty;
        rdfs:comment  "Certification issued for the given Participant."@en;
        rdfs:domain   core:Participant;
        rdfs:label    "participant certification"@en;
        rdfs:range    core:ParticipantCertification .

core:participantRefinement
        rdf:type      owl:ObjectProperty;
        rdfs:comment  "Conditions which needs to be satisfied that a single Participant can be seen as a member of the subject Participant. For instance, all Participants with their headquarter in Europe might be a potential consumer of GDPR-releated data."@en;
        rdfs:domain   core:Participant;
        rdfs:label    "participant refinement"@en;
        rdfs:range    odrl:Constraint .

core:path  rdf:type   owl:DatatypeProperty;
        rdfs:comment  "Relative path, topic or queue at which the content is published by the related host."@en;
        rdfs:domain   core:Endpoint;
        rdfs:label    "path"@en;
        rdfs:range    xsd:string .

core:paymentModality  rdf:type  owl:ObjectProperty;
        rdfs:comment  "Various pricing modalities such as idsc:FREE, idsc:FIXED_PRICE and idsc:NEGOTIATION_BASIS can be used as a pre-selection to annotate the terms of the contract. Depending on the requirements, additional free text information can be attached."@en;
        rdfs:domain   core:Resource;
        rdfs:label    "payment modality"@en;
        rdfs:range    core:PaymentModality .

core:physicalLocation
        rdf:type      owl:ObjectProperty;
        rdfs:comment  "The location where the Connector is physically deployed."@en;
        rdfs:domain   core:InfrastructureComponent;
        rdfs:label    "physicalLocation"@en;
        rdfs:range    core:Location .

core:pipEndpoint  rdf:type  owl:ObjectProperty;
        rdfs:comment  "The reference to the endpoint which provides the current state of the feature of interest (as referrenced by the leftOperand) can be retrieved."@en;
        rdfs:domain   odrl:Constraint;
        rdfs:label    "has PIP endpoint"@en;
        rdfs:range    core:PIP .

core:postDuty  rdf:type     owl:ObjectProperty , owl:AnnotationProperty;
        rdfs:comment        "A Duty imposed by the Rule, which must be executed after the Rule."@en;
        rdfs:domain         odrl:Permission;
        rdfs:label          "post-duty"@en;
        rdfs:range          odrl:Duty;
        rdfs:subPropertyOf  odrl:duty .

core:preDuty  rdf:type      owl:ObjectProperty , owl:AnnotationProperty;
        rdfs:comment        "A Duty imposed by the Rule, which must be executed before the Rule."@en;
        rdfs:domain         odrl:Permission;
        rdfs:label          "pre-duty"@en;
        rdfs:range          odrl:Duty;
        rdfs:subPropertyOf  odrl:duty .

core:provider  rdf:type  owl:ObjectProperty;
        rdfs:comment  "Provider of a Resource or Service that is the subject matter of the contract. This party may differ from the Assigner specified by the Contract rules."@en;
        rdfs:domain   core:Contract;
        rdfs:label    "Provider"@en;
        rdfs:range    core:Participant .

core:proxyAuthentication
        rdf:type      owl:DatatypeProperty , owl:ObjectProperty;
        rdfs:comment  "authentication information for the proxy"@en;
        rdfs:domain   core:Proxy;
        rdfs:label    "proxy Authentication"@en;
        rdfs:range    core:BasicAuthentication .

core:proxyURI  rdf:type  owl:DatatypeProperty;
        rdfs:comment  "URI of the proxy server."@en;
        rdfs:domain   core:Proxy;
        rdfs:label    "proxy URI"@en;
        rdfs:range    xsd:anyURI;
        rdfs:seeAlso  <https://www.gnu.org/software/emacs/manual/html_node/url/Proxies.html> .

core:publicKey  rdf:type  owl:ObjectProperty;
        rdfs:comment  "Public Key that has been created for the Component."@en;
        rdfs:domain   core:InfrastructureComponent;
        rdfs:label    "Public Key"@en;
        rdfs:range    core:PublicKey .

core:pxpEndpoint  rdf:type  owl:ObjectProperty;
        rdfs:comment  "The reference to the PXP which operates a specific action, URI or reference to an associated PXP interface."@en;
        rdfs:domain   odrl:Action;
        rdfs:label    "has PXP endpoint"@en;
        rdfs:range    core:PXP .

core:queryLanguage  rdf:type  owl:ObjectProperty;
        rdfs:comment  "This property specifies the language of the query."@en;
        rdfs:domain   core:QueryMessage;
        rdfs:label    "queryLanguage"@en;
        rdfs:range    core:QueryLanguage .

core:recipientAgent  rdf:type  owl:DatatypeProperty , owl:ObjectProperty;
        rdfs:comment  "The Agent for which the Mesaage is intended."@en;
        rdfs:domain   core:Message;
        rdfs:label    "recipient agent"@en;
        rdfs:range    foaf:Agent .

core:recipientConnector
        rdf:type      owl:ObjectProperty;
        rdfs:comment  "The Connector which is the recipient of the message."@en;
        rdfs:domain   core:Message;
        rdfs:label    "recipient connector"@en;
        rdfs:range    core:Connector .

core:recipientScope  rdf:type  owl:ObjectProperty;
        rdfs:comment  "Refers to the target property of a query message, see ids:QueryTarget."@en;
        rdfs:domain   core:QueryMessage;
        rdfs:label    "recipient scope"@en;
        rdfs:range    core:QueryTarget .

core:referringConnector
        rdf:type      owl:DatatypeProperty , owl:ObjectProperty;
        rdfs:comment  "The RDF connector entity as referred to by the DAT, with its URI included as the value. The value MUST be its accessible URI."@en;
        rdfs:domain   core:JwtPayload;
        rdfs:label    "referringConnector"@en;
        rdfs:range    core:Connector .

core:rejectionReason  rdf:type  owl:ObjectProperty;
        rdfs:comment  "Specifies the reason of the rejection."@en;
        rdfs:domain   core:RejectionMessage;
        rdfs:label    "rejectionReason"@en;
        rdfs:range    core:RejectionReason .

core:representation  rdf:type  owl:ObjectProperty;
        rdfs:comment  "Representation of the content."@en;
        rdfs:domain   core:DigitalContent;
        rdfs:label    "representation"@en;
        rdfs:range    <http://www.w3.org/ns/dcat#Distribution> .

core:representationStandard
        rdf:type            owl:DatatypeProperty;
        rdfs:comment        "Standards document defining the given Representation (in contrast to general Resource content). The Representation is assumed to conform to that Standard."@en;
        rdfs:domain         <http://www.w3.org/ns/dcat#Distribution>;
        rdfs:label          "representation standard"@en;
        rdfs:range          xsd:anyURI;
        rdfs:subPropertyOf  terms:conformsTo .

core:requestedArtifact
        rdf:type      owl:ObjectProperty;
        rdfs:comment  "References an artifact in the context of a request."@en;
        rdfs:domain   core:ArtifactRequestMessage;
        rdfs:label    "Requested Artifact"@en;
        rdfs:range    core:Artifact .

core:requestedElement
        rdf:type      owl:DatatypeProperty;
        rdfs:comment  "The element whose metadata is requested. "@en;
        rdfs:domain   core:DescriptionRequestMessage;
        rdfs:label    "requested Element"@en;
        rdfs:range    xsd:anyURI .

core:requestedParticipant
        rdf:type        owl:ObjectProperty;
        rdfs:comment    "This property is deprecated. Use ids:requestedElement along with ids:DescriptionRequestMessage instead. References a Participant in the context of a request."@en;
        rdfs:domain     core:ParticipantRequestMessage;
        rdfs:label      "Requested Participant (Deprecated)"@en;
        rdfs:range      core:Participant;
        owl:deprecated  true .

core:requestedResource
        rdf:type            owl:ObjectProperty;
        rdfs:comment        "A Resource that is part of a resource catalog, indicating a request (of, e.g., data, software, …)."@en;
        rdfs:domain         core:ResourceCatalog;
        rdfs:label          "requested resource"@en;
        rdfs:range          core:Resource;
        rdfs:subPropertyOf  <http://www.w3.org/ns/dcat#dataset> .

core:requester  rdf:type  owl:DatatypeProperty , owl:ObjectProperty;
        rdfs:comment  "\tThe target application requesting the usage. Should be some locally unique identifiers, preferably URIs."@en;
        rdfs:domain   core:UsageControlObject;
        rdfs:label    "requesting application"@en;
        rdfs:range    xsd:anyURI .

core:requiredDataApp  rdf:type  owl:ObjectProperty;
        rdfs:comment  "Refers to the concrete app representation (ids:AppRepresentation) for a data app (ids:DataApp) which is deployed in the Connector maintained by the Configuration Model and\n    whoose endpoint (ids:AppEndpoint) is used in this ids:RouteStep. The referred app representation should be part of the catalog of AppResources in the\n    corresponding Configuration Model (cf. ids:configuredAppResource property in class ids:ConfigurationModel).\n    "@en;
        rdfs:domain   core:RouteStep;
        rdfs:label    "requiredDataApp"@en;
        rdfs:range    core:AppRepresentation .

core:resourceCatalog  rdf:type  owl:ObjectProperty;
        rdfs:comment  "References the Catalog of published or requested resource by this Connector."@en;
        rdfs:domain   core:Connector;
        rdfs:label    "resource catalog"@en;
        rdfs:range    core:ResourceCatalog .

core:resourceEndpoint
        rdf:type      owl:ObjectProperty;
        rdfs:comment  "Reference to the Endpoints that serve the resource's content or let you exchange messages with an IDS Connector."@en;
        rdfs:domain   core:Resource;
        rdfs:label    "resource endpoint"@en;
        rdfs:range    core:ConnectorEndpoint .

core:resourcePart  rdf:type  owl:ObjectProperty;
        rdfs:comment        "Reference to a Resource (physically or logically) included, definition of part-whole hierarchies."@en;
        rdfs:domain         core:Resource;
        rdfs:label          "resource part"@en;
        rdfs:range          core:Resource;
        rdfs:subPropertyOf  core:contentPart .

core:revocationReason
        rdf:type      owl:DatatypeProperty;
        rdfs:comment  "Plain Text containing the reason for revoking an existing certificate of either a connector or participant."@en;
        rdfs:domain   [ rdf:type     owl:Class;
                        owl:unionOf  ( core:ConnectorCertificateRevokedMessage core:ParticipantCertificateRevokedMessage )
                      ];
        rdfs:label    "Revocation Reason"@en;
        rdfs:range    xsd:string .

core:routeConfiguration
        rdf:type      owl:DatatypeProperty;
        rdfs:comment  "Configuration details (e.g., contents of a config file) used to configure the route. Should be Base64 encoded."@en;
        rdfs:domain   core:AppRoute;
        rdfs:label    "route configuration"@en;
        rdfs:range    xsd:string .

core:routeDeployMethod
        rdf:type      owl:DatatypeProperty;
        rdfs:comment  "Supplementary information about, e.g., the technology used, for routes.";
        rdfs:domain   core:AppRoute;
        rdfs:label    "route deploy method"@en;
        rdfs:range    xsd:string .

core:routeDescription
        rdf:type      owl:DatatypeProperty;
        rdfs:comment  "Route description."@en;
        rdfs:domain   core:AppRoute;
        rdfs:label    "route description "@en;
        rdfs:range    xsd:string .

core:sample  rdf:type  owl:ObjectProperty;
        rdfs:comment  "Sample Resource instance."@en;
        rdfs:domain   core:Resource;
        rdfs:label    "sample"@en;
        rdfs:range    core:Resource .

core:samplingRate  rdf:type  owl:DatatypeProperty;
        rdfs:comment  "Audio sampling rate."@en;
        rdfs:domain   core:AudioRepresentation;
        rdfs:label    "sampling rate"@en;
        rdfs:range    xsd:decimal .

core:scope  rdf:type  owl:DatatypeProperty;
        rdfs:comment  "Currently, the scope is limited to 'Connector' but can be used for scoping purposes in the future. Scope is currently fixed to 'https://w3id.org/idsa/core/Connector'."@en;
        rdfs:domain   core:JwtPayload;
        rdfs:label    "scope"@en;
        rdfs:range    xsd:string;
        rdfs:seeAlso  <https://tools.ietf.org/html/rfc7519#section-4.1.2> .

core:securityGuarantee
        rdf:type      owl:ObjectProperty;
        rdfs:comment  "Reference to a security guarantee supported by given profile."@en;
        rdfs:domain   core:SecurityProfile;
        rdfs:label    "Security guarantee"@en;
        rdfs:range    core:SecurityGuarantee .

core:securityProfile  rdf:type  owl:ObjectProperty;
        rdfs:comment  "The SecurityProfile supported by the Connector."@en;
        rdfs:domain   [ rdf:type     owl:Class;
                        owl:unionOf  ( core:Connector core:JwtPayload )
                      ];
        rdfs:label    "securityProfile"@en;
        rdfs:range    core:SecurityProfile .

core:securityToken  rdf:type  owl:ObjectProperty;
        rdfs:comment  "A token representing a claim that the message sender supports a certain security profile."@en;
        rdfs:domain   core:Message;
        rdfs:label    "Security token"@en;
        rdfs:range    core:DynamicAttributeToken .

core:senderAgent  rdf:type  owl:DatatypeProperty , owl:ObjectProperty;
        rdfs:comment  "The Agent which initiated the Message."@en;
        rdfs:domain   core:Message;
        rdfs:label    "sender agent"@en;
        rdfs:range    foaf:Agent .

core:siteAddress  rdf:type  owl:DatatypeProperty;
        rdfs:comment  "Indicates an address for the site."@en;
        rdfs:domain   org:Site;
        rdfs:label    "site address"@en;
        rdfs:range    xsd:string .

core:source  rdf:type  owl:DatatypeProperty , owl:ObjectProperty;
        rdfs:comment  "The application which provided the data object. Should be a valid URI. Must be unique in the regarded environment."@en;
        rdfs:domain   core:UsageControlObject;
        rdfs:label    "source"@en;
        rdfs:range    xsd:anyURI .

core:sovereign  rdf:type  owl:ObjectProperty;
        rdfs:comment  "The 'owner', i.e. sovereign of the data."@en;
        rdfs:domain   core:Resource;
        rdfs:label    "sovereign"@en;
        rdfs:range    foaf:Agent .

core:sub  rdf:type    owl:DatatypeProperty;
        rdfs:comment  "The 'sub' (subject) claim identifies the principal that is the subject of the JWT."@en;
        rdfs:domain   core:JwtPayload;
        rdfs:label    "sub"@en;
        rdfs:range    xsd:string;
        rdfs:seeAlso  <https://tools.ietf.org/html/rfc7519#section-4.1.2> .

core:supportedUsagePolicies
        rdf:type      owl:ObjectProperty;
        rdfs:comment  "IDS Usage Policies a DataApp supports"@en;
        rdfs:domain   core:DataApp;
        rdfs:label    "supported usage policies"@en;
        rdfs:range    core:UsagePolicyClass .

core:target  rdf:type  owl:ObjectProperty;
        rdfs:comment  "The subject of the policy statement (odrl:Rule)."@en;
        rdfs:domain   odrl:Rule;
        rdfs:label    "target"@en;
        rdfs:range    odrl:Asset .

core:tokenFormat  rdf:type  owl:ObjectProperty;
        rdfs:comment  "Describes the format of the authentication token."@en;
        rdfs:domain   core:Token;
        rdfs:label    "tokenFormat"@en;
        rdfs:range    core:TokenFormat .

core:tokenValue  rdf:type  owl:DatatypeProperty;
        rdfs:comment  "An authentication token value like JSON Web Token."@en;
        rdfs:domain   core:Token;
        rdfs:label    "tokenValue"@en;
        rdfs:range    xsd:string .

core:transferContract
        rdf:type      owl:ObjectProperty;
        rdfs:comment  "The contract which is (or will be) the legal basis of the data transfer."@en;
        rdfs:domain   core:Message;
        rdfs:label    "transferContract"@en;
        rdfs:range    core:Contract .

core:transportCertsSha256
        rdf:type      owl:DatatypeProperty;
        rdfs:comment  "Separate certificates for IDS identification and transport encryption opens an attack vector for relay attacks. In order to prevent these attacks, a binding of this transport certificates to the connector is required. The inclusion of SHA256 fingerprints of currently valid transport certificates, mainly into the DAT, enables the client to relate the transport layer security with the IDS interactions."@en;
        rdfs:domain   core:JwtPayload;
        rdfs:label    "transportCertsSha256"@en;
        rdfs:range    xsd:string .

core:trustStore  rdf:type  owl:DatatypeProperty;
        rdfs:comment  "URI of the trust store server."@en;
        rdfs:domain   core:ConfigurationModel;
        rdfs:label    "trust store"@en;
        rdfs:range    xsd:anyURI .

core:trustStoreAlias  rdf:type  owl:DatatypeProperty;
        rdfs:comment  "alias for the trust store."@en;
        rdfs:domain   core:ConfigurationModel;
        rdfs:label    "trust store alias"@en;
        rdfs:range    xsd:string .

core:trustStorePassword
        rdf:type      owl:DatatypeProperty;
        rdfs:comment  "Password of the trust store server."@en;
        rdfs:domain   core:ConfigurationModel;
        rdfs:label    "trust store password"@en;
        rdfs:range    xsd:string .

core:usageDuration  rdf:type  owl:DatatypeProperty , owl:ObjectProperty;
        rdfs:comment  "Duration, which this asset is in use by now. Might be calculated on the fly when requested by a Usage Control Engine."@en;
        rdfs:domain   core:UsageControlObject;
        rdfs:label    "usage duration"@en;
        rdfs:range    xsd:duration .

core:user  rdf:type   owl:ObjectProperty;
        rdfs:comment  "The participant intending to use the data."@en;
        rdfs:domain   core:UsageControlObject;
        rdfs:label    "has user"@en;
        rdfs:range    core:Participant .

core:userAuthentication
        rdf:type      owl:ObjectProperty;
        rdfs:comment  "authentication methods allowed in a Configuration Model"@en;
        rdfs:domain   core:ConfigurationModel;
        rdfs:label    "user authentication"@en;
        rdfs:range    core:UserAuthentication .

core:variant  rdf:type  owl:ObjectProperty;
        rdfs:comment  "(Equivalent) variant of given Resource, e.g., a translation."@en;
        rdfs:domain   core:Resource;
        rdfs:label    "variant"@en;
        rdfs:range    core:Resource .

core:vatID  rdf:type  owl:DatatypeProperty;
        rdfs:comment  "The Value Added Tax ID (VAT ID) is used in the EU to clearly identify a company or entity which is liable for Value Added Tax."@en;
        rdfs:domain   core:Participant;
        rdfs:label    "VAT ID"@en;
        rdfs:range    xsd:string .

core:width  rdf:type  owl:DatatypeProperty;
        rdfs:comment  "Width of the visible frame."@en;
        rdfs:domain   core:ImageRepresentation;
        rdfs:label    "width"@en;
        rdfs:range    xsd:decimal .

dcam:memberOf  rdf:type  owl:AnnotationProperty .

dqv:Dimension  rdf:type  owl:Class .

dqv:Metric  rdf:type  owl:Class .

dqv:expectedDataType  rdf:type  owl:AnnotationProperty .

dqv:inDimension  rdf:type  owl:AnnotationProperty .

foaf:Agent  rdf:type  owl:Class .

foaf:Organization  rdf:type  owl:Class .

foaf:Person  rdf:type  owl:Class .

foaf:homepage  rdf:type  owl:AnnotationProperty .

foaf:name  rdf:type  owl:AnnotationProperty .

ns:license  rdf:type  owl:AnnotationProperty .

odrl:Action  rdf:type  owl:Class .

odrl:Agreement  rdf:type  owl:Class .

odrl:Asset  rdf:type  owl:Class .

odrl:AssetCollection  rdf:type  owl:Class .

odrl:Constraint  rdf:type  owl:Class .

odrl:Duty  rdf:type  owl:Class .

odrl:LeftOperand  rdf:type  owl:Class .

odrl:Offer  rdf:type  owl:Class .

odrl:Operator  rdf:type  owl:Class .

odrl:Party  rdf:type  owl:Class .

odrl:Permission  rdf:type  owl:Class .

odrl:Policy  rdf:type  owl:Class .

odrl:Request  rdf:type  owl:Class .

odrl:Rule  rdf:type  owl:Class .

odrl:duty  rdf:type  owl:AnnotationProperty .

odrl:includedIn  rdf:type  owl:AnnotationProperty .

odrl:source  rdf:type  owl:ObjectProperty .

org:Organization  rdf:type  owl:Class .

org:Site  rdf:type  owl:Class .

org:hasMember  rdf:type  owl:AnnotationProperty .

skos:Concept  rdf:type  owl:Class .

skos:broader  rdf:type  owl:AnnotationProperty .

skos:definition  rdf:type  owl:AnnotationProperty .

skos:inScheme  rdf:type  owl:AnnotationProperty .

skos:note  rdf:type  owl:AnnotationProperty .

skos:prefLabel  rdf:type  owl:AnnotationProperty .

terms:Agent  rdf:type  owl:Class .

terms:DCMIType  rdf:type  owl:Class .

terms:Frequency  rdf:type    owl:Class;
        owl:equivalentClass  core:Frequency .

terms:Location  rdf:type  owl:Class .

terms:MediaType  rdf:type  owl:Class .

terms:conformsTo  rdf:type  owl:DatatypeProperty .

terms:contributor  rdf:type  owl:AnnotationProperty .

terms:created  rdf:type  owl:AnnotationProperty .

terms:creator  rdf:type  owl:AnnotationProperty .

terms:isPartOf  rdf:type  owl:ObjectProperty .

terms:modified  rdf:type  owl:AnnotationProperty .

terms:publisher  rdf:type  owl:ObjectProperty .

terms:title  rdf:type  owl:AnnotationProperty .

terms:type  rdf:type  owl:ObjectProperty .

vann:preferredNamespacePrefix
        rdf:type  owl:AnnotationProperty .

vann:preferredNamespaceUri
        rdf:type  owl:AnnotationProperty .

void:vocabulary  rdf:type  owl:AnnotationProperty .

wgs84_pos:SpatialThing
        rdf:type  owl:Class .

wgs84_pos:lat  rdf:type  owl:AnnotationProperty .

wgs84_pos:long  rdf:type  owl:AnnotationProperty .

xsd:date  rdf:type  rdfs:Datatype .

xsd:duration  rdf:type  rdfs:Datatype .


<http://dbpedia.org/resource/ISO_639:aa>
        rdf:type    owl:NamedIndividual;
        owl:sameAs  <https://w3id.org/idsa/code/AA> .

<http://dbpedia.org/resource/ISO_639:ab>
        rdf:type    owl:NamedIndividual;
        owl:sameAs  <https://w3id.org/idsa/code/AB> .

<http://dbpedia.org/resource/ISO_639:ae>
        rdf:type    owl:NamedIndividual;
        owl:sameAs  <https://w3id.org/idsa/code/AE> .

<http://dbpedia.org/resource/ISO_639:af>
        rdf:type    owl:NamedIndividual;
        owl:sameAs  <https://w3id.org/idsa/code/AF> .

<http://dbpedia.org/resource/ISO_639:ak>
        rdf:type    owl:NamedIndividual;
        owl:sameAs  <https://w3id.org/idsa/code/AK> .

<http://dbpedia.org/resource/ISO_639:am>
        rdf:type    owl:NamedIndividual;
        owl:sameAs  <https://w3id.org/idsa/code/AM> .

<http://dbpedia.org/resource/ISO_639:an>
        rdf:type    owl:NamedIndividual;
        owl:sameAs  <https://w3id.org/idsa/code/AN> .

<http://dbpedia.org/resource/ISO_639:ar>
        rdf:type    owl:NamedIndividual;
        owl:sameAs  <https://w3id.org/idsa/code/AR> .

<http://dbpedia.org/resource/ISO_639:as>
        rdf:type    owl:NamedIndividual;
        owl:sameAs  <https://w3id.org/idsa/code/AS> .

<http://dbpedia.org/resource/ISO_639:av>
        rdf:type    owl:NamedIndividual;
        owl:sameAs  <https://w3id.org/idsa/code/AV> .

<http://dbpedia.org/resource/ISO_639:ay>
        rdf:type    owl:NamedIndividual;
        owl:sameAs  <https://w3id.org/idsa/code/AY> .

<http://dbpedia.org/resource/ISO_639:az>
        rdf:type    owl:NamedIndividual;
        owl:sameAs  <https://w3id.org/idsa/code/AZ> .

<http://dbpedia.org/resource/ISO_639:ba>
        rdf:type    owl:NamedIndividual;
        owl:sameAs  <https://w3id.org/idsa/code/BA> .

<http://dbpedia.org/resource/ISO_639:be>
        rdf:type    owl:NamedIndividual;
        owl:sameAs  <https://w3id.org/idsa/code/BE> .

<http://dbpedia.org/resource/ISO_639:bg>
        rdf:type    owl:NamedIndividual;
        owl:sameAs  <https://w3id.org/idsa/code/BG> .

<http://dbpedia.org/resource/ISO_639:bh>
        rdf:type    owl:NamedIndividual;
        owl:sameAs  <https://w3id.org/idsa/code/BH> .

<http://dbpedia.org/resource/ISO_639:bi>
        rdf:type    owl:NamedIndividual;
        owl:sameAs  <https://w3id.org/idsa/code/BI> .

<http://dbpedia.org/resource/ISO_639:bm>
        rdf:type    owl:NamedIndividual;
        owl:sameAs  <https://w3id.org/idsa/code/BM> .

<http://dbpedia.org/resource/ISO_639:bn>
        rdf:type    owl:NamedIndividual;
        owl:sameAs  <https://w3id.org/idsa/code/BN> .

<http://dbpedia.org/resource/ISO_639:bo>
        rdf:type    owl:NamedIndividual;
        owl:sameAs  <https://w3id.org/idsa/code/BO> .

<http://dbpedia.org/resource/ISO_639:br>
        rdf:type    owl:NamedIndividual;
        owl:sameAs  <https://w3id.org/idsa/code/BR> .

<http://dbpedia.org/resource/ISO_639:bs>
        rdf:type    owl:NamedIndividual;
        owl:sameAs  <https://w3id.org/idsa/code/BS> .

<http://dbpedia.org/resource/ISO_639:ca>
        rdf:type    owl:NamedIndividual;
        owl:sameAs  <https://w3id.org/idsa/code/CA> .

<http://dbpedia.org/resource/ISO_639:ce>
        rdf:type    owl:NamedIndividual;
        owl:sameAs  <https://w3id.org/idsa/code/CE> .

<http://dbpedia.org/resource/ISO_639:ch>
        rdf:type    owl:NamedIndividual;
        owl:sameAs  <https://w3id.org/idsa/code/CH> .

<http://dbpedia.org/resource/ISO_639:co>
        rdf:type    owl:NamedIndividual;
        owl:sameAs  <https://w3id.org/idsa/code/CO> .

<http://dbpedia.org/resource/ISO_639:cr>
        rdf:type    owl:NamedIndividual;
        owl:sameAs  <https://w3id.org/idsa/code/CR> .

<http://dbpedia.org/resource/ISO_639:cs>
        rdf:type    owl:NamedIndividual;
        owl:sameAs  <https://w3id.org/idsa/code/CS> .

<http://dbpedia.org/resource/ISO_639:cu>
        rdf:type    owl:NamedIndividual;
        owl:sameAs  <https://w3id.org/idsa/code/CU> .

<http://dbpedia.org/resource/ISO_639:cv>
        rdf:type    owl:NamedIndividual;
        owl:sameAs  <https://w3id.org/idsa/code/CV> .

<http://dbpedia.org/resource/ISO_639:cy>
        rdf:type    owl:NamedIndividual;
        owl:sameAs  <https://w3id.org/idsa/code/CY> .

<http://dbpedia.org/resource/ISO_639:da>
        rdf:type    owl:NamedIndividual;
        owl:sameAs  <https://w3id.org/idsa/code/DA> .

<http://dbpedia.org/resource/ISO_639:de>
        rdf:type    owl:NamedIndividual;
        owl:sameAs  <https://w3id.org/idsa/code/DE> .

<http://dbpedia.org/resource/ISO_639:dv>
        rdf:type    owl:NamedIndividual;
        owl:sameAs  <https://w3id.org/idsa/code/DV> .

<http://dbpedia.org/resource/ISO_639:dz>
        rdf:type    owl:NamedIndividual;
        owl:sameAs  <https://w3id.org/idsa/code/DZ> .

<http://dbpedia.org/resource/ISO_639:ee>
        rdf:type    owl:NamedIndividual;
        owl:sameAs  <https://w3id.org/idsa/code/EE> .

<http://dbpedia.org/resource/ISO_639:el>
        rdf:type    owl:NamedIndividual;
        owl:sameAs  <https://w3id.org/idsa/code/EL> .

<http://dbpedia.org/resource/ISO_639:en>
        rdf:type    owl:NamedIndividual;
        owl:sameAs  <https://w3id.org/idsa/code/EN> .

<http://dbpedia.org/resource/ISO_639:eo>
        rdf:type    owl:NamedIndividual;
        owl:sameAs  <https://w3id.org/idsa/code/EO> .

<http://dbpedia.org/resource/ISO_639:es>
        rdf:type    owl:NamedIndividual;
        owl:sameAs  <https://w3id.org/idsa/code/ES> .

<http://dbpedia.org/resource/ISO_639:et>
        rdf:type    owl:NamedIndividual;
        owl:sameAs  <https://w3id.org/idsa/code/ET> .

<http://dbpedia.org/resource/ISO_639:eu>
        rdf:type    owl:NamedIndividual;
        owl:sameAs  <https://w3id.org/idsa/code/EU> .

<http://dbpedia.org/resource/ISO_639:fa>
        rdf:type    owl:NamedIndividual;
        owl:sameAs  <https://w3id.org/idsa/code/FA> .

<http://dbpedia.org/resource/ISO_639:ff>
        rdf:type    owl:NamedIndividual;
        owl:sameAs  <https://w3id.org/idsa/code/FF> .

<http://dbpedia.org/resource/ISO_639:fi>
        rdf:type    owl:NamedIndividual;
        owl:sameAs  <https://w3id.org/idsa/code/FI> .

<http://dbpedia.org/resource/ISO_639:fj>
        rdf:type    owl:NamedIndividual;
        owl:sameAs  <https://w3id.org/idsa/code/FJ> .

<http://dbpedia.org/resource/ISO_639:fo>
        rdf:type    owl:NamedIndividual;
        owl:sameAs  <https://w3id.org/idsa/code/FO> .

<http://dbpedia.org/resource/ISO_639:fr>
        rdf:type    owl:NamedIndividual;
        owl:sameAs  <https://w3id.org/idsa/code/FR> .

<http://dbpedia.org/resource/ISO_639:fy>
        rdf:type    owl:NamedIndividual;
        owl:sameAs  <https://w3id.org/idsa/code/FY> .

<http://dbpedia.org/resource/ISO_639:ga>
        rdf:type    owl:NamedIndividual;
        owl:sameAs  <https://w3id.org/idsa/code/GA> .

<http://dbpedia.org/resource/ISO_639:gd>
        rdf:type    owl:NamedIndividual;
        owl:sameAs  <https://w3id.org/idsa/code/GD> .

<http://dbpedia.org/resource/ISO_639:gl>
        rdf:type    owl:NamedIndividual;
        owl:sameAs  <https://w3id.org/idsa/code/GL> .

<http://dbpedia.org/resource/ISO_639:gn>
        rdf:type    owl:NamedIndividual;
        owl:sameAs  <https://w3id.org/idsa/code/GN> .

<http://dbpedia.org/resource/ISO_639:gu>
        rdf:type    owl:NamedIndividual;
        owl:sameAs  <https://w3id.org/idsa/code/GU> .

<http://dbpedia.org/resource/ISO_639:gv>
        rdf:type    owl:NamedIndividual;
        owl:sameAs  <https://w3id.org/idsa/code/GV> .

<http://dbpedia.org/resource/ISO_639:ha>
        rdf:type    owl:NamedIndividual;
        owl:sameAs  <https://w3id.org/idsa/code/HA> .

<http://dbpedia.org/resource/ISO_639:he>
        rdf:type    owl:NamedIndividual;
        owl:sameAs  <https://w3id.org/idsa/code/HE> .

<http://dbpedia.org/resource/ISO_639:hi>
        rdf:type    owl:NamedIndividual;
        owl:sameAs  <https://w3id.org/idsa/code/HI> .

<http://dbpedia.org/resource/ISO_639:ho>
        rdf:type    owl:NamedIndividual;
        owl:sameAs  <https://w3id.org/idsa/code/HO> .

<http://dbpedia.org/resource/ISO_639:hr>
        rdf:type    owl:NamedIndividual;
        owl:sameAs  <https://w3id.org/idsa/code/HR> .

<http://dbpedia.org/resource/ISO_639:ht>
        rdf:type    owl:NamedIndividual;
        owl:sameAs  <https://w3id.org/idsa/code/HT> .

<http://dbpedia.org/resource/ISO_639:hu>
        rdf:type    owl:NamedIndividual;
        owl:sameAs  <https://w3id.org/idsa/code/HU> .

<http://dbpedia.org/resource/ISO_639:hy>
        rdf:type    owl:NamedIndividual;
        owl:sameAs  <https://w3id.org/idsa/code/HY> .

<http://dbpedia.org/resource/ISO_639:hz>
        rdf:type    owl:NamedIndividual;
        owl:sameAs  <https://w3id.org/idsa/code/HZ> .

<http://dbpedia.org/resource/ISO_639:ia>
        rdf:type    owl:NamedIndividual;
        owl:sameAs  <https://w3id.org/idsa/code/IA> .

<http://dbpedia.org/resource/ISO_639:id>
        rdf:type    owl:NamedIndividual;
        owl:sameAs  <https://w3id.org/idsa/code/ID> .

<http://dbpedia.org/resource/ISO_639:ie>
        rdf:type    owl:NamedIndividual;
        owl:sameAs  <https://w3id.org/idsa/code/IE> .

<http://dbpedia.org/resource/ISO_639:ig>
        rdf:type    owl:NamedIndividual;
        owl:sameAs  <https://w3id.org/idsa/code/IG> .

<http://dbpedia.org/resource/ISO_639:ii>
        rdf:type    owl:NamedIndividual;
        owl:sameAs  <https://w3id.org/idsa/code/II> .

<http://dbpedia.org/resource/ISO_639:ik>
        rdf:type    owl:NamedIndividual;
        owl:sameAs  <https://w3id.org/idsa/code/IK> .

<http://dbpedia.org/resource/ISO_639:io>
        rdf:type    owl:NamedIndividual;
        owl:sameAs  <https://w3id.org/idsa/code/IO> .

<http://dbpedia.org/resource/ISO_639:is>
        rdf:type    owl:NamedIndividual;
        owl:sameAs  <https://w3id.org/idsa/code/IS> .

<http://dbpedia.org/resource/ISO_639:it>
        rdf:type    owl:NamedIndividual;
        owl:sameAs  <https://w3id.org/idsa/code/IT> .

<http://dbpedia.org/resource/ISO_639:iu>
        rdf:type    owl:NamedIndividual;
        owl:sameAs  <https://w3id.org/idsa/code/IU> .

<http://dbpedia.org/resource/ISO_639:ja>
        rdf:type    owl:NamedIndividual;
        owl:sameAs  <https://w3id.org/idsa/code/JA> .

<http://dbpedia.org/resource/ISO_639:jv>
        rdf:type    owl:NamedIndividual;
        owl:sameAs  <https://w3id.org/idsa/code/JV> .

<http://dbpedia.org/resource/ISO_639:ka>
        rdf:type    owl:NamedIndividual;
        owl:sameAs  <https://w3id.org/idsa/code/KA> .

<http://dbpedia.org/resource/ISO_639:kg>
        rdf:type    owl:NamedIndividual;
        owl:sameAs  <https://w3id.org/idsa/code/KG> .

<http://dbpedia.org/resource/ISO_639:ki>
        rdf:type    owl:NamedIndividual;
        owl:sameAs  <https://w3id.org/idsa/code/KI> .

<http://dbpedia.org/resource/ISO_639:kj>
        rdf:type    owl:NamedIndividual;
        owl:sameAs  <https://w3id.org/idsa/code/KJ> .

<http://dbpedia.org/resource/ISO_639:kk>
        rdf:type    owl:NamedIndividual;
        owl:sameAs  <https://w3id.org/idsa/code/KK> .

<http://dbpedia.org/resource/ISO_639:kl>
        rdf:type    owl:NamedIndividual;
        owl:sameAs  <https://w3id.org/idsa/code/KL> .

<http://dbpedia.org/resource/ISO_639:km>
        rdf:type    owl:NamedIndividual;
        owl:sameAs  <https://w3id.org/idsa/code/KM> .

<http://dbpedia.org/resource/ISO_639:kn>
        rdf:type    owl:NamedIndividual;
        owl:sameAs  <https://w3id.org/idsa/code/KN> .

<http://dbpedia.org/resource/ISO_639:ko>
        rdf:type    owl:NamedIndividual;
        owl:sameAs  <https://w3id.org/idsa/code/KO> .

<http://dbpedia.org/resource/ISO_639:kr>
        rdf:type    owl:NamedIndividual;
        owl:sameAs  <https://w3id.org/idsa/code/KR> .

<http://dbpedia.org/resource/ISO_639:ks>
        rdf:type    owl:NamedIndividual;
        owl:sameAs  <https://w3id.org/idsa/code/KS> .

<http://dbpedia.org/resource/ISO_639:ku>
        rdf:type    owl:NamedIndividual;
        owl:sameAs  <https://w3id.org/idsa/code/KU> .

<http://dbpedia.org/resource/ISO_639:kv>
        rdf:type    owl:NamedIndividual;
        owl:sameAs  <https://w3id.org/idsa/code/KV> .

<http://dbpedia.org/resource/ISO_639:kw>
        rdf:type    owl:NamedIndividual;
        owl:sameAs  <https://w3id.org/idsa/code/KW> .

<http://dbpedia.org/resource/ISO_639:ky>
        rdf:type    owl:NamedIndividual;
        owl:sameAs  <https://w3id.org/idsa/code/KY> .

<http://dbpedia.org/resource/ISO_639:la>
        rdf:type    owl:NamedIndividual;
        owl:sameAs  <https://w3id.org/idsa/code/LA> .

<http://dbpedia.org/resource/ISO_639:lb>
        rdf:type    owl:NamedIndividual;
        owl:sameAs  <https://w3id.org/idsa/code/LB> .

<http://dbpedia.org/resource/ISO_639:lg>
        rdf:type    owl:NamedIndividual;
        owl:sameAs  <https://w3id.org/idsa/code/LG> .

<http://dbpedia.org/resource/ISO_639:li>
        rdf:type    owl:NamedIndividual;
        owl:sameAs  <https://w3id.org/idsa/code/LI> .

<http://dbpedia.org/resource/ISO_639:ln>
        rdf:type    owl:NamedIndividual;
        owl:sameAs  <https://w3id.org/idsa/code/LN> .

<http://dbpedia.org/resource/ISO_639:lo>
        rdf:type    owl:NamedIndividual;
        owl:sameAs  <https://w3id.org/idsa/code/LO> .

<http://dbpedia.org/resource/ISO_639:lt>
        rdf:type    owl:NamedIndividual;
        owl:sameAs  <https://w3id.org/idsa/code/LT> .

<http://dbpedia.org/resource/ISO_639:lu>
        rdf:type    owl:NamedIndividual;
        owl:sameAs  <https://w3id.org/idsa/code/LU> .

<http://dbpedia.org/resource/ISO_639:lv>
        rdf:type    owl:NamedIndividual;
        owl:sameAs  <https://w3id.org/idsa/code/LV> .

<http://dbpedia.org/resource/ISO_639:mg>
        rdf:type    owl:NamedIndividual;
        owl:sameAs  <https://w3id.org/idsa/code/MG> .

<http://dbpedia.org/resource/ISO_639:mh>
        rdf:type    owl:NamedIndividual;
        owl:sameAs  <https://w3id.org/idsa/code/MH> .

<http://dbpedia.org/resource/ISO_639:mi>
        rdf:type    owl:NamedIndividual;
        owl:sameAs  <https://w3id.org/idsa/code/MI> .

<http://dbpedia.org/resource/ISO_639:mk>
        rdf:type    owl:NamedIndividual;
        owl:sameAs  <https://w3id.org/idsa/code/MK> .

<http://dbpedia.org/resource/ISO_639:ml>
        rdf:type    owl:NamedIndividual;
        owl:sameAs  <https://w3id.org/idsa/code/ML> .

<http://dbpedia.org/resource/ISO_639:mn>
        rdf:type    owl:NamedIndividual;
        owl:sameAs  <https://w3id.org/idsa/code/MN> .

<http://dbpedia.org/resource/ISO_639:mr>
        rdf:type    owl:NamedIndividual;
        owl:sameAs  <https://w3id.org/idsa/code/MR> .

<http://dbpedia.org/resource/ISO_639:ms>
        rdf:type    owl:NamedIndividual;
        owl:sameAs  <https://w3id.org/idsa/code/MS> .

<http://dbpedia.org/resource/ISO_639:mt>
        rdf:type    owl:NamedIndividual;
        owl:sameAs  <https://w3id.org/idsa/code/MT> .

<http://dbpedia.org/resource/ISO_639:my>
        rdf:type    owl:NamedIndividual;
        owl:sameAs  <https://w3id.org/idsa/code/MY> .

<http://dbpedia.org/resource/ISO_639:na>
        rdf:type    owl:NamedIndividual;
        owl:sameAs  <https://w3id.org/idsa/code/NA> .

<http://dbpedia.org/resource/ISO_639:nb>
        rdf:type    owl:NamedIndividual;
        owl:sameAs  <https://w3id.org/idsa/code/NB> .

<http://dbpedia.org/resource/ISO_639:nd>
        rdf:type    owl:NamedIndividual;
        owl:sameAs  <https://w3id.org/idsa/code/ND> .

<http://dbpedia.org/resource/ISO_639:ne>
        rdf:type    owl:NamedIndividual;
        owl:sameAs  <https://w3id.org/idsa/code/NE> .

<http://dbpedia.org/resource/ISO_639:ng>
        rdf:type    owl:NamedIndividual;
        owl:sameAs  <https://w3id.org/idsa/code/NG> .

<http://dbpedia.org/resource/ISO_639:nl>
        rdf:type    owl:NamedIndividual;
        owl:sameAs  <https://w3id.org/idsa/code/NL> .

<http://dbpedia.org/resource/ISO_639:nn>
        rdf:type    owl:NamedIndividual;
        owl:sameAs  <https://w3id.org/idsa/code/NN> .

<http://dbpedia.org/resource/ISO_639:no>
        rdf:type    owl:NamedIndividual;
        owl:sameAs  <https://w3id.org/idsa/code/NO> .

<http://dbpedia.org/resource/ISO_639:nr>
        rdf:type    owl:NamedIndividual;
        owl:sameAs  <https://w3id.org/idsa/code/NR> .

<http://dbpedia.org/resource/ISO_639:nv>
        rdf:type    owl:NamedIndividual;
        owl:sameAs  <https://w3id.org/idsa/code/NV> .

<http://dbpedia.org/resource/ISO_639:ny>
        rdf:type    owl:NamedIndividual;
        owl:sameAs  <https://w3id.org/idsa/code/NY> .

<http://dbpedia.org/resource/ISO_639:oc>
        rdf:type    owl:NamedIndividual;
        owl:sameAs  <https://w3id.org/idsa/code/OC> .

<http://dbpedia.org/resource/ISO_639:oj>
        rdf:type    owl:NamedIndividual;
        owl:sameAs  <https://w3id.org/idsa/code/OJ> .

<http://dbpedia.org/resource/ISO_639:om>
        rdf:type    owl:NamedIndividual;
        owl:sameAs  <https://w3id.org/idsa/code/OM> .

<http://dbpedia.org/resource/ISO_639:or>
        rdf:type    owl:NamedIndividual;
        owl:sameAs  <https://w3id.org/idsa/code/OR> .

<http://dbpedia.org/resource/ISO_639:os>
        rdf:type    owl:NamedIndividual;
        owl:sameAs  <https://w3id.org/idsa/code/OS> .

<http://dbpedia.org/resource/ISO_639:pa>
        rdf:type    owl:NamedIndividual;
        owl:sameAs  <https://w3id.org/idsa/code/PA> .

<http://dbpedia.org/resource/ISO_639:pi>
        rdf:type    owl:NamedIndividual;
        owl:sameAs  <https://w3id.org/idsa/code/PI> .

<http://dbpedia.org/resource/ISO_639:pl>
        rdf:type    owl:NamedIndividual;
        owl:sameAs  <https://w3id.org/idsa/code/PL> .

<http://dbpedia.org/resource/ISO_639:ps>
        rdf:type    owl:NamedIndividual;
        owl:sameAs  <https://w3id.org/idsa/code/PS> .

<http://dbpedia.org/resource/ISO_639:pt>
        rdf:type    owl:NamedIndividual;
        owl:sameAs  <https://w3id.org/idsa/code/PT> .

<http://dbpedia.org/resource/ISO_639:qu>
        rdf:type    owl:NamedIndividual;
        owl:sameAs  <https://w3id.org/idsa/code/QU> .

<http://dbpedia.org/resource/ISO_639:rm>
        rdf:type    owl:NamedIndividual;
        owl:sameAs  <https://w3id.org/idsa/code/RM> .

<http://dbpedia.org/resource/ISO_639:rn>
        rdf:type    owl:NamedIndividual;
        owl:sameAs  <https://w3id.org/idsa/code/RN> .

<http://dbpedia.org/resource/ISO_639:ro>
        rdf:type    owl:NamedIndividual;
        owl:sameAs  <https://w3id.org/idsa/code/RO> .

<http://dbpedia.org/resource/ISO_639:ru>
        rdf:type    owl:NamedIndividual;
        owl:sameAs  <https://w3id.org/idsa/code/RU> .

<http://dbpedia.org/resource/ISO_639:rw>
        rdf:type    owl:NamedIndividual;
        owl:sameAs  <https://w3id.org/idsa/code/RW> .

<http://dbpedia.org/resource/ISO_639:sa>
        rdf:type    owl:NamedIndividual;
        owl:sameAs  <https://w3id.org/idsa/code/SA> .

<http://dbpedia.org/resource/ISO_639:sc>
        rdf:type    owl:NamedIndividual;
        owl:sameAs  <https://w3id.org/idsa/code/SC> .

<http://dbpedia.org/resource/ISO_639:sd>
        rdf:type    owl:NamedIndividual;
        owl:sameAs  <https://w3id.org/idsa/code/SD> .

<http://dbpedia.org/resource/ISO_639:se>
        rdf:type    owl:NamedIndividual;
        owl:sameAs  <https://w3id.org/idsa/code/SE> .

<http://dbpedia.org/resource/ISO_639:sg>
        rdf:type    owl:NamedIndividual;
        owl:sameAs  <https://w3id.org/idsa/code/SG> .

<http://dbpedia.org/resource/ISO_639:si>
        rdf:type    owl:NamedIndividual;
        owl:sameAs  <https://w3id.org/idsa/code/SI> .

<http://dbpedia.org/resource/ISO_639:sk>
        rdf:type    owl:NamedIndividual;
        owl:sameAs  <https://w3id.org/idsa/code/SK> .

<http://dbpedia.org/resource/ISO_639:sl>
        rdf:type    owl:NamedIndividual;
        owl:sameAs  <https://w3id.org/idsa/code/SL> .

<http://dbpedia.org/resource/ISO_639:sm>
        rdf:type    owl:NamedIndividual;
        owl:sameAs  <https://w3id.org/idsa/code/SM> .

<http://dbpedia.org/resource/ISO_639:sn>
        rdf:type    owl:NamedIndividual;
        owl:sameAs  <https://w3id.org/idsa/code/SN> .

<http://dbpedia.org/resource/ISO_639:so>
        rdf:type    owl:NamedIndividual;
        owl:sameAs  <https://w3id.org/idsa/code/SO> .

<http://dbpedia.org/resource/ISO_639:sq>
        rdf:type    owl:NamedIndividual;
        owl:sameAs  <https://w3id.org/idsa/code/SQ> .

<http://dbpedia.org/resource/ISO_639:sr>
        rdf:type    owl:NamedIndividual;
        owl:sameAs  <https://w3id.org/idsa/code/SR> .

<http://dbpedia.org/resource/ISO_639:ss>
        rdf:type    owl:NamedIndividual;
        owl:sameAs  <https://w3id.org/idsa/code/SS> .

<http://dbpedia.org/resource/ISO_639:st>
        rdf:type    owl:NamedIndividual;
        owl:sameAs  <https://w3id.org/idsa/code/ST> .

<http://dbpedia.org/resource/ISO_639:su>
        rdf:type    owl:NamedIndividual;
        owl:sameAs  <https://w3id.org/idsa/code/SU> .

<http://dbpedia.org/resource/ISO_639:sv>
        rdf:type    owl:NamedIndividual;
        owl:sameAs  <https://w3id.org/idsa/code/SV> .

<http://dbpedia.org/resource/ISO_639:sw>
        rdf:type    owl:NamedIndividual;
        owl:sameAs  <https://w3id.org/idsa/code/SW> .

<http://dbpedia.org/resource/ISO_639:ta>
        rdf:type    owl:NamedIndividual;
        owl:sameAs  <https://w3id.org/idsa/code/TA> .

<http://dbpedia.org/resource/ISO_639:te>
        rdf:type    owl:NamedIndividual;
        owl:sameAs  <https://w3id.org/idsa/code/TE> .

<http://dbpedia.org/resource/ISO_639:tg>
        rdf:type    owl:NamedIndividual;
        owl:sameAs  <https://w3id.org/idsa/code/TG> .

<http://dbpedia.org/resource/ISO_639:th>
        rdf:type    owl:NamedIndividual;
        owl:sameAs  <https://w3id.org/idsa/code/TH> .

<http://dbpedia.org/resource/ISO_639:ti>
        rdf:type    owl:NamedIndividual;
        owl:sameAs  <https://w3id.org/idsa/code/TI> .

<http://dbpedia.org/resource/ISO_639:tk>
        rdf:type    owl:NamedIndividual;
        owl:sameAs  <https://w3id.org/idsa/code/TK> .

<http://dbpedia.org/resource/ISO_639:tl>
        rdf:type    owl:NamedIndividual;
        owl:sameAs  <https://w3id.org/idsa/code/TL> .

<http://dbpedia.org/resource/ISO_639:tn>
        rdf:type    owl:NamedIndividual;
        owl:sameAs  <https://w3id.org/idsa/code/TN> .

<http://dbpedia.org/resource/ISO_639:to>
        rdf:type    owl:NamedIndividual;
        owl:sameAs  <https://w3id.org/idsa/code/TO> .

<http://dbpedia.org/resource/ISO_639:tr>
        rdf:type    owl:NamedIndividual;
        owl:sameAs  <https://w3id.org/idsa/code/TR> .

<http://dbpedia.org/resource/ISO_639:ts>
        rdf:type    owl:NamedIndividual;
        owl:sameAs  <https://w3id.org/idsa/code/TS> .

<http://dbpedia.org/resource/ISO_639:tt>
        rdf:type    owl:NamedIndividual;
        owl:sameAs  <https://w3id.org/idsa/code/TT> .

<http://dbpedia.org/resource/ISO_639:tw>
        rdf:type    owl:NamedIndividual;
        owl:sameAs  <https://w3id.org/idsa/code/TW> .

<http://dbpedia.org/resource/ISO_639:ty>
        rdf:type    owl:NamedIndividual;
        owl:sameAs  <https://w3id.org/idsa/code/TY> .

<http://dbpedia.org/resource/ISO_639:ug>
        rdf:type    owl:NamedIndividual;
        owl:sameAs  <https://w3id.org/idsa/code/UG> .

<http://dbpedia.org/resource/ISO_639:uk>
        rdf:type    owl:NamedIndividual;
        owl:sameAs  <https://w3id.org/idsa/code/UK> .

<http://dbpedia.org/resource/ISO_639:ur>
        rdf:type    owl:NamedIndividual;
        owl:sameAs  <https://w3id.org/idsa/code/UR> .

<http://dbpedia.org/resource/ISO_639:uz>
        rdf:type    owl:NamedIndividual;
        owl:sameAs  <https://w3id.org/idsa/code/UZ> .

<http://dbpedia.org/resource/ISO_639:ve>
        rdf:type    owl:NamedIndividual;
        owl:sameAs  <https://w3id.org/idsa/code/VE> .

<http://dbpedia.org/resource/ISO_639:vi>
        rdf:type    owl:NamedIndividual;
        owl:sameAs  <https://w3id.org/idsa/code/VI> .

<http://dbpedia.org/resource/ISO_639:vo>
        rdf:type    owl:NamedIndividual;
        owl:sameAs  <https://w3id.org/idsa/code/VO> .

<http://dbpedia.org/resource/ISO_639:wa>
        rdf:type    owl:NamedIndividual;
        owl:sameAs  <https://w3id.org/idsa/code/WA> .

<http://dbpedia.org/resource/ISO_639:wo>
        rdf:type    owl:NamedIndividual;
        owl:sameAs  <https://w3id.org/idsa/code/WO> .

<http://dbpedia.org/resource/ISO_639:xh>
        rdf:type    owl:NamedIndividual;
        owl:sameAs  <https://w3id.org/idsa/code/XH> .

<http://dbpedia.org/resource/ISO_639:yi>
        rdf:type    owl:NamedIndividual;
        owl:sameAs  <https://w3id.org/idsa/code/YI> .

<http://dbpedia.org/resource/ISO_639:yo>
        rdf:type    owl:NamedIndividual;
        owl:sameAs  <https://w3id.org/idsa/code/YO> .

<http://dbpedia.org/resource/ISO_639:za>
        rdf:type    owl:NamedIndividual;
        owl:sameAs  <https://w3id.org/idsa/code/ZA> .

<http://dbpedia.org/resource/ISO_639:zh>
        rdf:type    owl:NamedIndividual;
        owl:sameAs  <https://w3id.org/idsa/code/ZH> .

<http://dbpedia.org/resource/ISO_639:zu>
        rdf:type    owl:NamedIndividual;
        owl:sameAs  <https://w3id.org/idsa/code/ZU> .

<http://purl.org/cld/freq/annual>
        rdf:type    owl:NamedIndividual;
        owl:sameAs  <https://w3id.org/idsa/code/ANNUAL> .

<http://purl.org/cld/freq/biennial>
        rdf:type    owl:NamedIndividual;
        owl:sameAs  <https://w3id.org/idsa/code/BIENNIAL> .

<http://purl.org/cld/freq/bimonthly>
        rdf:type    owl:NamedIndividual;
        owl:sameAs  <https://w3id.org/idsa/code/BIMONTHLY> .

<http://purl.org/cld/freq/biweekly>
        rdf:type    owl:NamedIndividual;
        owl:sameAs  <https://w3id.org/idsa/code/BIWEEKLY> .

<http://purl.org/cld/freq/continuous>
        rdf:type    owl:NamedIndividual;
        owl:sameAs  <https://w3id.org/idsa/code/CONTINUOUS> .

<http://purl.org/cld/freq/daily>
        rdf:type    owl:NamedIndividual;
        owl:sameAs  <https://w3id.org/idsa/code/DAILY> .

<http://purl.org/cld/freq/irregular>
        rdf:type    owl:NamedIndividual;
        owl:sameAs  <https://w3id.org/idsa/code/IRREGULAR> .

<http://purl.org/cld/freq/monthly>
        rdf:type    owl:NamedIndividual;
        owl:sameAs  <https://w3id.org/idsa/code/MONTHLY> .

<http://purl.org/cld/freq/quarterly>
        rdf:type    owl:NamedIndividual;
        owl:sameAs  <https://w3id.org/idsa/code/QUARTERLY> .

<http://purl.org/cld/freq/semiannual>
        rdf:type    owl:NamedIndividual;
        owl:sameAs  <https://w3id.org/idsa/code/SEMIANNUAL> .

<http://purl.org/cld/freq/semimonthly>
        rdf:type    owl:NamedIndividual;
        owl:sameAs  <https://w3id.org/idsa/code/SEMIMONTHLY> .

<http://purl.org/cld/freq/semiweekly>
        rdf:type    owl:NamedIndividual;
        owl:sameAs  <https://w3id.org/idsa/code/SEMIWEEKLY> .

<http://purl.org/cld/freq/threeTimesAMonth>
        rdf:type    owl:NamedIndividual;
        owl:sameAs  <https://w3id.org/idsa/code/THREE_TIMES_A_MONTH> .

<http://purl.org/cld/freq/threeTimesAWeek>
        rdf:type    owl:NamedIndividual;
        owl:sameAs  <https://w3id.org/idsa/code/THREE_TIMES_A_WEEK> .

<http://purl.org/cld/freq/threeTimesAYear>
        rdf:type    owl:NamedIndividual;
        owl:sameAs  <https://w3id.org/idsa/code/THREE_TIMES_A_YEAR> .

<http://purl.org/cld/freq/triennial>
        rdf:type    owl:NamedIndividual;
        owl:sameAs  <https://w3id.org/idsa/code/TRIENNIAL> .

<http://purl.org/cld/freq/weekly>
        rdf:type    owl:NamedIndividual;
        owl:sameAs  <https://w3id.org/idsa/code/WEEKLY> .

<http://purl.org/vocommons/voaf#Vocabulary>
        rdf:type  owl:Class .

<http://sebastian.tramp.name>
        rdf:type   foaf:Person , terms:Agent , owl:NamedIndividual;
        foaf:name  "Sebastian Tramp" .

<http://www.apache.org/licenses/LICENSE-2.0>
        rdfs:label  "Apache License Version 2.0, January 2004" .

<http://www.geonames.org/ontology#Feature>
        rdf:type  owl:Class .

<http://www.w3.org/2006/time#TemporalEntity>
        rdf:type  owl:Class .

<http://www.w3.org/ns/dcat#Catalog>
        rdf:type  owl:Class .

<http://www.w3.org/ns/dcat#Dataset>
        rdf:type  owl:Class .

<http://www.w3.org/ns/dcat#Distribution>
        rdf:type  owl:Class .

<http://www.w3.org/ns/dcat#byteSize>
        rdf:type  owl:DatatypeProperty .

<http://www.w3.org/ns/dcat#dataset>
        rdf:type  owl:ObjectProperty .

<http://www.w3.org/ns/locn#Geometry>
        rdf:type  owl:Class .

<https://github.com/HaydarAk>
        rdf:type   foaf:Person , terms:Agent , owl:NamedIndividual;
        foaf:name  "Haydar Akyürek" .

<https://github.com/JohannesLipp>
        rdf:type   foaf:Person , terms:Agent , owl:NamedIndividual;
        foaf:name  "Johannes Lipp" .

<https://github.com/Maboeckmann>
        rdf:type   foaf:Person , terms:Agent , owl:NamedIndividual;
        foaf:name  "Matthias Böckmann" .

<https://github.com/clange>
        rdf:type   foaf:Person , terms:Agent , owl:NamedIndividual;
        foaf:name  "Christoph Lange" .

<https://github.com/cmader>
        rdf:type   foaf:Person , terms:Agent , owl:NamedIndividual;
        foaf:name  "Christian Mader" .

<https://github.com/jlangkau>
        rdf:type   foaf:Person , terms:Agent , owl:NamedIndividual;
        foaf:name  "Jörg Langkau" .

<https://github.com/jpullmann>
        rdf:type   foaf:Person , terms:Agent , owl:NamedIndividual;
        foaf:name  "Jaroslav Pullmann" .

<https://github.com/lcomet>
        rdf:type   foaf:Person , terms:Agent , owl:NamedIndividual;
        foaf:name  "Lina Molinas Comet" .

<https://github.com/mkollenstart>
        rdf:type   foaf:Person , terms:Agent , owl:NamedIndividual;
        foaf:name  "Maarten Kollenstart" .

<https://github.com/sebbader>
        rdf:type   foaf:Person , terms:Agent , owl:NamedIndividual;
        foaf:name  "Sebastian Bader" .
